@prefix : <https://saref.etsi.org/saref4bldgMerge/> .
@prefix owl: <http://www.w3.org/2002/07/owl#> .
@prefix rdf: <http://www.w3.org/1999/02/22-rdf-syntax-ns#> .
@prefix xml: <http://www.w3.org/XML/1998/namespace> .
@prefix xsd: <http://www.w3.org/2001/XMLSchema#> .
@prefix rdfs: <http://www.w3.org/2000/01/rdf-schema#> .
@base <https://saref.etsi.org/saref4bldgMerge/> .

<https://saref.etsi.org/saref4bldgMerge/> rdf:type owl:Ontology ;
                                           <http://purl.org/dc/terms/contributor> <http://www.maxime-lefrancois.info/> ,
                                                                                  <https://pdi.fbk.eu/people/profile/dragoni> ;
                                           <http://purl.org/dc/terms/creator> <http://maxime-lefrancois.info/me#> ,
                                                                              <http://purl.org/net/mpoveda> ,
                                                                              <http://www.garcia-castro.com/foaf.rdf#me> ,
                                                                              <https://w3id.org/people/mpoveda/> ,
                                                                              <https://www.linkedin.com/in/bouterca> ,
                                                                              <https://www.linkedin.com/in/giulia-biagioni> ,
                                                                              <https://www.linkedin.com/in/lauradaniele> ,
                                                                              <https://www.linkedin.com/in/david-gnabasik-0056a0ba/> ;
                                           <http://purl.org/dc/terms/description> "The Smart Applications REFerence ontology (SAREF) is intended to enable interoperability between solutions from different providers and among various activity sectors in the Internet of Things (IoT), thus contributing to the development of the global digital market."@en ,
                                                                                  "This ontology extends the SAREF ontology for the building domain by defining building devices and how they are located in a building. This extension is based on the ISO 16739:2013 Industry Foundation Classes (IFC) standard for data sharing in the construction and facility management industries. The descriptions of the classes and properties extracted from IFC have been taken from the IFC documentation."@en ;
                                           <http://purl.org/dc/terms/issued> "2024-10-31"^^xsd:date ,
                                                                             "2025-04-24"^^xsd:date ;
                                           <http://purl.org/dc/terms/license> <https://forge.etsi.org/etsi-software-license> ;
                                           <http://purl.org/dc/terms/modified> "2024-03-06"^^xsd:date ,
                                                                               "2025-04-24"^^xsd:date ;
                                           <http://purl.org/dc/terms/publisher> <https://www.etsi.org/> ;
                                           <http://purl.org/dc/terms/source> <https://saref.etsi.org/sources/saref-core/> ,
                                                                             <https://saref.etsi.org/sources/saref4bldg/> ;
                                           <http://purl.org/dc/terms/title> "SAREF4BLDG: an extension of SAREF for the building domain"@en ,
                                                                            "SAREF: the Smart Applications REFerence ontology"@en ;
                                           <http://purl.org/vocab/vann/preferredNamespacePrefix> "saref" ,
                                                                                                 "s4bldg" ;
                                           <http://purl.org/vocab/vann/preferredNamespaceUri> "https://saref.etsi.org/core/" ,
                                                                                              "https://saref.etsi.org/saref4bldg/" ;
                                           rdfs:comment """Information about changes compared to version 1.1.1: 
 - Updated namespaces for compatibility with SAREF v3."""@en ,
                                                        """Information about changes compared to version 1.1.2: 
 - see https://labs.etsi.org/rep/saref/saref4bldg/-/milestones/1."""@en ,
                                                        """Information about changes to version 2.1.1:

- The classes and properties related to how to represent devices in building spaces (such as the saref:BuildingSpace class,  saref:BuildingObject class and saref:isLocatedIn property) have been removed from SAREF and incorporated  into the SAREF4BLDG extension related to buildings, including the reuse of the W3C? WGS84 geo positioning vocabulary.
- The saref:DeviceCategory and saref:FunctionCategory classes have been removed. Instead, the hierarchy of device categories has been implemented directly as subclasses of the saref:Device class.
- The information specific for energy efficiency has been moved to the SAREF4ENER extension. For example, the saref:Profile class has been redefined to accommodate only the properties that are general enough for any type of profile, not only for energy and power. Details on how to specifically model a power profile can be found in the SAREF4ENER extension. 
- The subclasses of the saref:Energy class  have been removed (i.e., Average Energy, Maximum Energy, Minimum Energy, Total Energy, HVAC Energy, Hot Water Energy and Lighting Energy).
- The saref:Property class has been split into two classes (saref:Property and saref:Measurement), as it is done in the SAREF4ENVI extension, in order to properly accommodate the distinction between the concept of property (an observable quality of something) and the concept of measurement (a concrete value observed for a property).
- Too restrictive cardinality restrictions have been revised, sometimes making them optional rather than mandatory (better to make properties mandatory in the extensions that specialize SAREF for a specific purpose, rather than restricting SAREF, whose purpose is more general). For example, definitions of units of measurement using an enumeration (owl:oneOf) were too restrictive because they did not allow using other units than those enumerated. Therefore, the individuals of each class are still there, but the owl:oneOf enumeration has been removed.
- The saref:UnitOfMeasure subclasses use individuals from the OM ontology for unit of measures, but this is not the only solution. It has been clarified in the comments that the OM ontology is an example, but other ontologies can be used.
- The global restrictions (rdfs:domain and rdfs:range) in object properties have been completely removed not to hinder interoperability. Object properties are now only restricted locally in the classes. 
- The subclasses of saref:Task have been transormed in individuals.
- The saref:hasTask property has been removed from the saref:Profile class to resolve an ambiguity with the saref:Task class.""" ,
                                                        """Information about changes to version 3.1.1:

NOTE:	In some cases, references have been added to indicate the issue in the ETSI Forge (https://saref.etsi.org/sources/saref-core/issues) where the change was discussed and implemented.

- Added the saref:FeatureOfInterest class and the properties used to relate it to saref:Measurement (saref:hasMeasurement and saref:isMeasurementOf) and to saref:Property (saref:hasProperty and saref:isPropertyOf).
- Added the saref:measurementMadeBy property as inverse of saref:makesMeasurement.
- The saref:relatesToProperty and saref:relatesToMeasurement properties are now inverse of each other.
- The range of saref:hasValue, which was defined as xsd:float, has been removed to support other datatypes for measurements.
- The range of datatype properties, which was defined as xsd:string, has been removed in order to support strings with language tags (rdf:langString). This affects saref:hasDescription, saref:hasManufacturer, saref:hasModel and saref:hasName, which now have implicitly a range of rdfs:Literal.
- The saref:hasName property has been removed and the use of rdfs:label is recommended. 
- The saref:hasDescription property has been deprecated and the use of rdfs:comment is recommended. 
- Too restrictive restrictions have been removed and in some cases the ontology documentation has been updated to reflect this: a saref:Command having at most one saref:hasDescription; a saref:Task being accomplished by at least one saref:Device; a saref:Device having a typical consumption of only energy or power; a saref:Commodity being measured in units of measure; restrictions on the values of saref:accomplishes that only covered specific use cases; universal restrictions on the saref:actsUpon property have been changed to existential ones; restrictions on the commands that a saref:Function may have, since there could be others not included in the defined enumerations; restrictive documentation of saref:EventFunction and saref:SmokeSensor.
- Bugs have been fixed: some devices (saref:DoorSwitch, saref:EnergyMeter, saref:LigthSwitch, saref:SmokeSensor, and saref:TemperatureSensor) were defined as subclass of a device and at the same time as consisting of such device; a saref:LightSwitch controls light and does not measure light, since it is an actuator; incorrect documentation of saref:OnState and saref:OffState.
- The saref:BuildingRelated, saref:EnergyRelated and saref:FunctionRelated classes have been removed, since the different extensions already classify the device types.
- The instances of the subclasses of saref:Command have been removed, since they represent examples.
- The instances of saref:UnitOfMeasure have been moved to examples.
- The classes related to the SAREF4ENER extension have been removed: saref:Generator, saref:Storage, saref:Load and saref:EnergyMeter.
- Some instances of saref:Device have been moved to examples: saref:WashingMachine, saref:LightingDevice, saref:MicroRenewable, saref:Multimedia, and saref:Network.
- Added domain and range axioms wherever the definition of a property unambiguously identifies the domain or the range of the property.
- The OWL Time ontology is not imported anymore.
- The documentation of some ontology terms has been updated for clarification.
- Language tags have been added to all labels and comments.
""" ,
                                                        """Information about changes to version 3.2.1:

NOTE: Rationale and decisions for many of the changes in V3.2.1 are available in issues in project https://saref.etsi.org/sources/saref-core/issues.

- Definition of saref:FeatureOfInterest is clarified, not only properties are measured, but properties and states can be observed and controlled.
- Definition of saref:FeatureOfInterest: Clarify it is a specific real world entity.
- Definition of saref:FeatureOfInterest: allValuesFrom axioms are unnecessary and have been deleted.
- Introduced class saref:FeatureKind
- Use SKOS to organize generic classes in taxonomies.
- Introduce hasClassKind for Class is Feature, Device, Property, State, Function, Command.
- Add local restrictions on consistsOf on feature of interest
- Defined domain of saref:hasManufacturer to union of feature kind and feature of interest.
- Defined domain of saref:hasModel to union of feature kind and feature of interest.
- Most axioms on saref:Device were useless and have been deleted.
- definition of saref:Device clarifies it is a real world entity.
- saref:Device is explicitly a subclass of saref:FeatureOfInterest and s4syst:System.
- saref:actsUpon now holds not only between a command and a state. It generalizes actsUpon, observes, controls. Domain and range are unions of several classes.
- Introduced property saref:isActedUponBy.
- Introduced property saref:observes, as sub-property of saref:actsUpon. and generalization of measures.
- Introduced property saref:controls, as sub-property of saref:actsUpon. and generalization of saref:controlsProperty.
- Introduced property saref:isControlledBy.
- saref:measuresProperty is deprecated: will be deleted in the next release of SAREF
- saref:isMeasuredByDevice is deprecated: will be deleted in the next release of SAREF
- saref:isControlledByDevice is deprecated: will be deleted in the next release of SAREF
- saref:controlsProperty is deprecated: will be deleted in the next release of SAREF
- Definition of saref:Appliance is grounded on tasks and commodities.
- Definition of Sensor is simplified and grounded on saref:observes. Local restriction on saref:hasFunction is deleted.
- Definition of Actuator is simplified and grounded on saref:controls. Local restriction on saref:hasFunction is deleted.
- Definition of Meter is simplified and grounded on saref:observes. Local restriction on saref:hasFunction is deleted.
- Deprecated saref:HVAC for it is only an example.
- Deprecated saref:Switch for it is only an example.
- Deprecated saref:DoorSwitch for it is only an example.
- Deprecated saref:LightSwitch for it is only an example.
- Deprecated saref:SmokeSensor for it is only an example.
- Deprecated saref:TemperatureSensor for it is only an example.
- The following tasks are deprecated, and may be deleted in the next release of SAREF: saref:Cleaning, saref:Comfort, saref:Drying, saref:EnergyEfficiency, saref:Entertainment, saref:Lighting, saref:MeterReading, saref:Safety, saref:Washing, saref:WellBeing.
- Definition of saref:Commodity is simplified.
- saref:Electricity is deprecated: will be defined as an instance of saref:Commodity in the next release of SAREF
- saref:Gas is deprecated: will be defined as an instance of saref:Commodity in the next release of SAREF
- saref:Coal is deprecated: will be defined as an instance of saref:Commodity in the next release of SAREF
- saref:Water is deprecated: will be defined as an instance of saref:Commodity in the next release of SAREF
- New category of commodities saref:EnergyCommodity
- New category of commodities saref:NaturalResourceCommodity
- Introduced saref:consumes, saref:isConsumedBy, saref:produces, saref:isProducedBy, saref:stores, saref:isStoredBy.
- The definition and scope of usage for saref:Property is clarified. Axiomatization is simplified.
- applicability of saref:hasProperty is relaxed to also saref:FeatureKind
- Introduced saref:PropertyOfInterest to solved the ambiguity between generic vs specific properties.
- Introduced saref:hasPropertyOfInterest and saref:isPropertyOfInterestOf. Cannot use saref:hasProperty due to the combination of cardinality restrictions and sub-property chain axioms makes the ontology exist the OWL 2 DL prodile.
- Introduced saref:PropertyValue to simplify the association of a measure to a property, without always needing it to be a measurement made by a device.
- Clarified definition of saref:hasValue.
- Relaxed domain of saref:isMeasuredIn so it can apply to saref:PropertyValue as well as saref:Measurement. The new range will be enforced in the next release of SAREF.
- Introduced saref:hasPropertyValue.
- Introduced saref:isValueOfProperty.
- The following classes are deprecated and may be defined as instances of saref:Property in the next release of SAREF: saref:Energy, saref:Humidity, saref:Light, saref:Motion, saref:Occupancy, saref:Power, saref:Pressure, saref:Price, saref:Smoke, saref:Temperature
- saref:EnergyUnit is deprecated. Will be deleted in the next release of SAREF
- saref:IlluminanceUnit is deprecated. Will be deleted in the next release of SAREF
- saref:PowerUnit is deprecated. Will be deleted in the next release of SAREF
- saref:PressureUnit is deprecated. Will be deleted in the next release of SAREF
- saref:TemperatureUnit is deprecated. Will be deleted in the next release of SAREF
- Clarified and generalized definition of saref:State. Can now apply to all features of interest, not just devices.
- Relaxed domain of saref:hasState.
- Introduced saref:isStateOf.
- Introduced saref:StateOfInterest, parallel to saref:PropertyOfInterest.
- Introduced saref:hasStateOfInterest and saref:isStateOfInterestOf, parallel to saref:hasPropertyOfInterest and saref:isPropertyOfInterestOf.
- The following classes are deprecated and may be defined as instances of saref:State in the next release of SAREF: saref:CloseState, saref:MultiLevelState, saref:OffState, saref:OnOffState, saref:OnState, saref:OpenCloseState, saref:OpenState, saref:StartState, saref:StartStopState, saref:StopState.
- Simplified definition and axiomatization of saref:Function. Added examples.
- saref:SensingFunction is deprecated: may be defined as an instance of saref:Function in the next release of SAREF
- saref:hasSensingRange is deprecated together with saref:SensingFunction. And may be defined as an instance of saref:Property in the next release of SAREF
- saref:hasSensorType is deprecated together with saref:SensingFunction. Use saref:hasDeviceKind instead.
- saref:EventFunction is deprecated: may be defined as an instance of saref:Function in the next release of SAREF
- saref:hasThresholdMeasurement is deprecated together with saref:EventFunction. And may be defined as an instance of saref:Property in the next release of SAREF
- saref:MeteringFunction is deprecated: may be defined as an instance of saref:Function in the next release of SAREF
- deprecated saref:hasMeterReading together with saref:Measurement and saref:MeteringFunction
- deprecated saref:hasMeterReadingType together with saref:MeteringFunction
- saref:LevelControlFunction, saref:StartStopFunction, saref:OpenCloseFunction, saref:OnOffFunction,  
- saref:ActuatingFunction are deprecated: may be defined as an instance of saref:Function in the next release of SAREF.
- Domain of saref:hasFunction is relaxed.
- Introduced saref:isFunctionOf.
- Introduced saref:FunctionOfInterest, parallel to saref:PropertyOfInterest.
- Simplified definition and axiomatization of saref:Command. Added examples.
- Domain of saref:hasCommand is relaxed to saref:Function or saref:FunctionOfInterest.
- Introduced mandatory and optional commands.
- Introduced saref:hasInput and saref:hasOutput.
- Introduced saref:CommandOfInterest, parallel to saref:PropertyOfInterest.
- The following classes are deprecated and may be defined as instances of saref:Command in the next release of SAREF: saref:ToggleCommand, saref:GetCommand, saref:NotifyCommand, saref:GetSensingDataCommand, saref:GetCurrentMeterValueCommand, saref:GetMeterDataCommand, saref:GetMeterHistoryCommand, saref:SetAbsoluteLevelCommand, saref:SetRelativeLevelCommand, saref:SetLevelCommand, saref:StepDownCommand, saref:StepUpCommand, saref:PauseCommand, saref:StartCommand, saref:StopCommand, saref:CloseCommand, saref:OpenCommand, saref:OnCommand, saref:OffCommand.
- Simplified definition of saref:Service. Added examples.
- Relaxed domain and range of saref:represents.
- Clarified definition of saref:offers.
- Clarified definition of saref:isOfferedBy.
- saref:SwitchOnService is deprecated for it is just an example. It may be deleted in the next release of SAREF
- Introduced saref:Operation and associated properties from oneM2M base ontology.
- Introduced saref:ProcedureExecution.
- Introduce saref:madeBy (resp. saref:madeExecution) as generalization of saref:measurementMadeBy (resp. saref:makesMeasurement).
- saref:makesMeasurement is deprecated as one of the properties related to saref:Measurement. It may be deleted in the next release of SAREF
- saref:makesMeasurement is deprecated as one of the properties related to saref:Measurement. It may be deleted in the next release of SAREF
- Introduced saref:hasResult as part of general will to make SAREF and SOSA/SSN converge.
- Introduced saref:hasResultTime as part of general will to make SAREF and SOSA/SSN converge.
- Introduced saref:hasPhenomenonTime as part of general will to make SAREF and SOSA/SSN converge.
- Tried to clarify definition of saref:hasTimestamp. Still unclear.
- Deprecated saref:Measurement in favour of saref:Observation, to generalize to observation of states and convergence with SOSA/SSN.
- Deprecated saref:isMeasurementOf together with saref:Measurement.
- Deprecated saref:isMeasurementOf together with saref:Measurement.
- Deprecated saref:isMeasurementOf together with saref:Measurement.
- Deprecated saref:isMeasurementOf together with saref:Measurement.
- Class saref:Profile has been re-specified, to take into account findings from SAREF4ENER V1.2.1.
- Relaxed domain of saref:hasProfile to saref:FeatureKind or saref:Device
- Deprecated saref:hasTime and use OWL Time instead whenever possible.
- Deprecated saref:Time and use OWL Time instead whenever possible.
- Deprecated saref:hasTypicalConsumption. May be defined as an instance of saref:Property in the next release of SAREF.
""" ,
                                                        """Information about changes to version 4.1.1:

NOTE: Rationale and decisions for many of the changes in V4.1.1 are available in issues in project https://labs.etsi.org/rep/saref/saref-core/-/milestones/3#tab-issues

- Deprecated classes and properties have been deleted
- Reworded definition of saref:Sensor and saref:Meter
- saref:hasValue is now optional on saref:PropertyValue
- improved parallel between Property and State descriptions
- introduced saref:StateValue
- Removed examples of commodity categories
- Added notes and examples in multiple sections
- Added clause 5.14 about composite properties
- Reworked figures throughout the document
- Added migration guide from V3.1.1 to V4.1.1
- Updated the oneM2M base ontology to SAREF mapping
- Added principle on generic versus specific entities distinction
- Added references to EN 303 760
""" ;
                                           rdfs:seeAlso <https://www.etsi.org/deliver/etsi_ts/103200_103299/103264/04.01.01_60/ts_103264v040101p.pdf> ,
                                                        <https://www.etsi.org/deliver/etsi_ts/103400_103499/10341003/02.01.01_60/ts_10341003v020101p.pdf> ;
                                           owl:priorVersion <https://saref.etsi.org/core/v3.2.1/> ,
                                                            <https://saref.etsi.org/saref4bldg/v1.1.2/> ;
                                           owl:versionInfo "v4.1.1" ,
                                                           "v2.1.1" .

#################################################################
#    Annotation properties
#################################################################

###  http://purl.org/dc/terms/contributor
<http://purl.org/dc/terms/contributor> rdf:type owl:AnnotationProperty .


###  http://purl.org/dc/terms/creator
<http://purl.org/dc/terms/creator> rdf:type owl:AnnotationProperty .


###  http://purl.org/dc/terms/dateCopyrighted
<http://purl.org/dc/terms/dateCopyrighted> rdf:type owl:AnnotationProperty .


###  http://purl.org/dc/terms/description
<http://purl.org/dc/terms/description> rdf:type owl:AnnotationProperty .


###  http://purl.org/dc/terms/issued
<http://purl.org/dc/terms/issued> rdf:type owl:AnnotationProperty .


###  http://purl.org/dc/terms/license
<http://purl.org/dc/terms/license> rdf:type owl:AnnotationProperty .


###  http://purl.org/dc/terms/modified
<http://purl.org/dc/terms/modified> rdf:type owl:AnnotationProperty .


###  http://purl.org/dc/terms/publisher
<http://purl.org/dc/terms/publisher> rdf:type owl:AnnotationProperty .


###  http://purl.org/dc/terms/rightsHolder
<http://purl.org/dc/terms/rightsHolder> rdf:type owl:AnnotationProperty .


###  http://purl.org/dc/terms/source
<http://purl.org/dc/terms/source> rdf:type owl:AnnotationProperty .


###  http://purl.org/dc/terms/title
<http://purl.org/dc/terms/title> rdf:type owl:AnnotationProperty .


###  http://purl.org/vocab/vann/preferredNamespacePrefix
<http://purl.org/vocab/vann/preferredNamespacePrefix> rdf:type owl:AnnotationProperty .


###  http://purl.org/vocab/vann/preferredNamespaceUri
<http://purl.org/vocab/vann/preferredNamespaceUri> rdf:type owl:AnnotationProperty .


###  http://www.w3.org/2004/02/skos/core#example
<http://www.w3.org/2004/02/skos/core#example> rdf:type owl:AnnotationProperty .


###  http://www.w3.org/2004/02/skos/core#historyNote
<http://www.w3.org/2004/02/skos/core#historyNote> rdf:type owl:AnnotationProperty .


###  http://www.w3.org/2004/02/skos/core#note
<http://www.w3.org/2004/02/skos/core#note> rdf:type owl:AnnotationProperty .


###  http://www.w3.org/2004/02/skos/core#scopeNote
<http://www.w3.org/2004/02/skos/core#scopeNote> rdf:type owl:AnnotationProperty .


#################################################################
#    Datatypes
#################################################################

###  http://www.w3.org/2001/XMLSchema#date
xsd:date rdf:type rdfs:Datatype .


###  http://www.w3.org/2001/XMLSchema#duration
xsd:duration rdf:type rdfs:Datatype .


#################################################################
#    Object Properties
#################################################################

###  http://www.w3.org/2004/02/skos/core#broader
<http://www.w3.org/2004/02/skos/core#broader> rdf:type owl:ObjectProperty ;
                                              owl:inverseOf <http://www.w3.org/2004/02/skos/core#narrower> .


###  http://www.w3.org/2004/02/skos/core#narrower
<http://www.w3.org/2004/02/skos/core#narrower> rdf:type owl:ObjectProperty .


###  https://saref.etsi.org/core/accomplishes
<https://saref.etsi.org/core/accomplishes> rdf:type owl:ObjectProperty ;
                                           owl:inverseOf <https://saref.etsi.org/core/isAccomplishedBy> ;
                                           rdfs:range <https://saref.etsi.org/core/Task> ;
                                           rdfs:comment "Links a certain entity (e.g., a device) to the task it accomplishes."@en ;
                                           rdfs:label "accomplishes"@en .


###  https://saref.etsi.org/core/consistsOf
<https://saref.etsi.org/core/consistsOf> rdf:type owl:ObjectProperty ;
                                         owl:propertyChainAxiom ( <https://saref.etsi.org/core/consistsOf>
                                                                  <https://saref.etsi.org/core/hasFeatureKind>
                                                                ) ,
                                                                ( <https://saref.etsi.org/core/consistsOf>
                                                                  <https://saref.etsi.org/core/hasPropertyKind>
                                                                ) ,
                                                                ( <https://saref.etsi.org/core/consistsOf>
                                                                  <https://saref.etsi.org/core/hasStateKind>
                                                                ) ,
                                                                ( <https://saref.etsi.org/core/consistsOf>
                                                                  <https://saref.etsi.org/core/isValueOfProperty>
                                                                ) ,
                                                                ( <https://saref.etsi.org/core/consistsOf>
                                                                  <https://saref.etsi.org/core/isValueOfState>
                                                                ) ;
                                         rdfs:comment "A relationship indicating a composite entity that consists of other entities (e.g., a temperature/humidity sensor that consists of a temperature sensor and a humidity sensor)"@en ;
                                         rdfs:label "consists of"@en ;
                                         <http://www.w3.org/2004/02/skos/core#historyNote> "V3.2.1: Add local restrictions on consistsOf on feature of interest"@en ;
                                         <http://www.w3.org/2004/02/skos/core#note> "A feature kind (respectively a feature of interest) may consist of (OP saref:consistsOf) other feature kinds (respectively feature kinds or features of interest)."@en ,
                                                                                    "The OP saref:consistsOf can link a composite property, property of interest, or property value to its individual components."@en .


###  https://saref.etsi.org/core/consumes
<https://saref.etsi.org/core/consumes> rdf:type owl:ObjectProperty ;
                                       owl:inverseOf <https://saref.etsi.org/core/isConsumedBy> ;
                                       rdfs:domain [ rdf:type owl:Class ;
                                                     owl:unionOf ( <https://saref.etsi.org/core/Device>
                                                                   <https://saref.etsi.org/core/DeviceKind>
                                                                   <https://saref.etsi.org/core/FeatureKind>
                                                                   <https://saref.etsi.org/core/FeatureOfInterest>
                                                                 )
                                                   ] ;
                                       rdfs:range <https://saref.etsi.org/core/Commodity> ;
                                       rdfs:comment "Links a feature kind, feature of interest, or device, to the commodity it consumes"@en ;
                                       rdfs:label "consumes"@en ;
                                       <http://www.w3.org/2004/02/skos/core#historyNote> "V3.2.1: Introduced saref:consumes, saref:isConsumedBy, saref:produces, saref:isProducedBy, saref:stores, saref:isStoredBy."@en .


###  https://saref.etsi.org/core/controls
<https://saref.etsi.org/core/controls> rdf:type owl:ObjectProperty ;
                                       rdfs:subPropertyOf <https://saref.etsi.org/core/targets> ;
                                       owl:inverseOf <https://saref.etsi.org/core/isControlledBy> ;
                                       rdfs:domain [ rdf:type owl:Class ;
                                                     owl:unionOf ( <https://saref.etsi.org/core/Actuation>
                                                                   <https://saref.etsi.org/core/Actuator>
                                                                   <https://saref.etsi.org/core/Command>
                                                                   <https://saref.etsi.org/core/CommandOfInterest>
                                                                   <https://saref.etsi.org/core/DeviceKind>
                                                                   <https://saref.etsi.org/core/Function>
                                                                   <https://saref.etsi.org/core/FunctionOfInterest>
                                                                 )
                                                   ] ;
                                       rdfs:comment "Links a device, function, command, or procedure execution, to the feature, property, or state, it controls."@en ;
                                       rdfs:label "controls"@en ;
                                       <http://www.w3.org/2004/02/skos/core#historyNote> "V3.2.1: Introduced property saref:controls, as sub-property of saref:targets. and generalization of saref:controlsProperty."@en .


###  https://saref.etsi.org/core/hasApplicableTime
<https://saref.etsi.org/core/hasApplicableTime> rdf:type owl:ObjectProperty ;
                                                rdfs:range [ rdf:type owl:Class ;
                                                             owl:unionOf ( <http://www.w3.org/2006/time#TemporalEntity>
                                                                           <http://www.w3.org/2006/time#TemporalPosition>
                                                                         )
                                                           ] ;
                                                rdfs:comment "Links an entity (e.g., a profile) to an instant or interval or other compound temporal entity expressed using OWL Time, which bounds temporally the applicable context of that entity."@en ;
                                                rdfs:label "has applicable time"@en .


###  https://saref.etsi.org/core/hasCommand
<https://saref.etsi.org/core/hasCommand> rdf:type owl:ObjectProperty ;
                                         owl:inverseOf <https://saref.etsi.org/core/isCommandOf> ;
                                         rdfs:domain [ rdf:type owl:Class ;
                                                       owl:unionOf ( <https://saref.etsi.org/core/Function>
                                                                     <https://saref.etsi.org/core/FunctionOfInterest>
                                                                   )
                                                     ] ;
                                         rdfs:range <https://saref.etsi.org/core/Command> ;
                                         owl:propertyChainAxiom ( <https://saref.etsi.org/core/hasCommandOfInterest>
                                                                  <https://saref.etsi.org/core/hasCommandKind>
                                                                ) ,
                                                                ( <https://saref.etsi.org/core/hasFeatureKind>
                                                                  <https://saref.etsi.org/core/hasMandatoryCommand>
                                                                ) ;
                                         rdfs:comment "Links a function or function of interest and the command it supports."@en ;
                                         rdfs:label "has command"@en ;
                                         <http://www.w3.org/2004/02/skos/core#historyNote> "V3.2.1: Domain of saref:hasCommand is relaxed to saref:Function or saref:FunctionOfInterest."@en .


###  https://saref.etsi.org/core/hasCommandKind
<https://saref.etsi.org/core/hasCommandKind> rdf:type owl:ObjectProperty ;
                                             rdfs:domain <https://saref.etsi.org/core/CommandOfInterest> ;
                                             rdfs:range <https://saref.etsi.org/core/Command> ;
                                             owl:propertyChainAxiom ( <https://saref.etsi.org/core/hasCommandKind>
                                                                      <http://www.w3.org/2004/02/skos/core#broader>
                                                                    ) ;
                                             rdfs:comment "links a command of interest to its kind, a command."@en ;
                                             rdfs:label "has command kind"@en .


###  https://saref.etsi.org/core/hasCommandOfInterest
<https://saref.etsi.org/core/hasCommandOfInterest> rdf:type owl:ObjectProperty ;
                                                   owl:inverseOf <https://saref.etsi.org/core/isCommandOfInterestOf> ;
                                                   rdfs:domain <https://saref.etsi.org/core/FunctionOfInterest> ;
                                                   rdfs:range <https://saref.etsi.org/core/CommandOfInterest> ;
                                                   rdfs:comment "Links a function of interest to one of its commands of interest."@en ;
                                                   rdfs:label "has command of interest"@en .


###  https://saref.etsi.org/core/hasDeviceKind
<https://saref.etsi.org/core/hasDeviceKind> rdf:type owl:ObjectProperty ;
                                            rdfs:subPropertyOf <https://saref.etsi.org/core/hasFeatureKind> ;
                                            rdfs:domain <https://saref.etsi.org/core/Device> ;
                                            rdfs:range <https://saref.etsi.org/core/DeviceKind> ;
                                            rdfs:comment "Links a device to its kind, a device kind. Kinds of devices describe models of devices, with common properties and common states having the same value, targeting the same properties and states, common functions, and common services."@en ;
                                            rdfs:label "has device kind"@en .


###  https://saref.etsi.org/core/hasFeatureKind
<https://saref.etsi.org/core/hasFeatureKind> rdf:type owl:ObjectProperty ;
                                             rdfs:domain <https://saref.etsi.org/core/FeatureOfInterest> ;
                                             rdfs:range <https://saref.etsi.org/core/FeatureKind> ;
                                             owl:propertyChainAxiom ( <https://saref.etsi.org/core/hasFeatureKind>
                                                                      <http://www.w3.org/2004/02/skos/core#broader>
                                                                    ) ;
                                             rdfs:comment "links a feature of interest to its kind, a feature kind"@en ;
                                             rdfs:label "has feature kind"@en ;
                                             <http://www.w3.org/2004/02/skos/core#historyNote> "V3.2.1: Introduce hasClassKind for Class is Feature, Device, Property, State, Function, Command."@en .


###  https://saref.etsi.org/core/hasFunction
<https://saref.etsi.org/core/hasFunction> rdf:type owl:ObjectProperty ;
                                          owl:inverseOf <https://saref.etsi.org/core/isFunctionOf> ;
                                          rdfs:domain [ rdf:type owl:Class ;
                                                        owl:unionOf ( <https://saref.etsi.org/core/FeatureKind>
                                                                      <https://saref.etsi.org/core/FeatureOfInterest>
                                                                    )
                                                      ] ;
                                          rdfs:range <https://saref.etsi.org/core/Function> ;
                                          owl:propertyChainAxiom ( <http://www.w3.org/2004/02/skos/core#broader>
                                                                   <https://saref.etsi.org/core/hasFunction>
                                                                 ) ,
                                                                 ( <https://saref.etsi.org/core/hasDeviceKind>
                                                                   <https://saref.etsi.org/core/hasFunction>
                                                                 ) ,
                                                                 ( <https://saref.etsi.org/core/hasFunctionOfInterest>
                                                                   <https://saref.etsi.org/core/hasFunctionKind>
                                                                 ) ;
                                          rdfs:comment "Links a feature kind or a device to one of its functions."@en ;
                                          rdfs:label "has function"@en ;
                                          <http://www.w3.org/2004/02/skos/core#historyNote> "V3.2.1: Domain of saref:hasFunction is relaxed."@en .


###  https://saref.etsi.org/core/hasFunctionKind
<https://saref.etsi.org/core/hasFunctionKind> rdf:type owl:ObjectProperty ;
                                              rdfs:domain <https://saref.etsi.org/core/FunctionOfInterest> ;
                                              rdfs:range <https://saref.etsi.org/core/Function> ;
                                              owl:propertyChainAxiom ( <https://saref.etsi.org/core/hasFunctionKind>
                                                                       <http://www.w3.org/2004/02/skos/core#broader>
                                                                     ) ;
                                              rdfs:comment "links a function of interest to its kind, a function"@en ;
                                              rdfs:label "has function kind"@en .


###  https://saref.etsi.org/core/hasFunctionOfInterest
<https://saref.etsi.org/core/hasFunctionOfInterest> rdf:type owl:ObjectProperty ;
                                                    owl:inverseOf <https://saref.etsi.org/core/isFunctionOfInterestOf> ;
                                                    rdfs:domain <https://saref.etsi.org/core/Device> ;
                                                    rdfs:range <https://saref.etsi.org/core/FunctionOfInterest> ;
                                                    rdfs:comment "Links a device to one of its functions of interest."@en ;
                                                    rdfs:label "has function of interest"@en .


###  https://saref.etsi.org/core/hasInput
<https://saref.etsi.org/core/hasInput> rdf:type owl:ObjectProperty ;
                                       rdfs:domain [ rdf:type owl:Class ;
                                                     owl:unionOf ( <https://saref.etsi.org/core/Command>
                                                                   <https://saref.etsi.org/core/CommandOfInterest>
                                                                   <https://saref.etsi.org/core/Operation>
                                                                   <https://saref.etsi.org/core/ProcedureExecution>
                                                                 )
                                                   ] ;
                                       rdfs:comment "Links a command, operation, or procedure execution, to its inputs."@en ;
                                       rdfs:label "has input"@en ;
                                       <http://www.w3.org/2004/02/skos/core#example> "Different complementary commands can be defined for controlling a light. Turn on or off the light based on a desired state, toggle the light status of a specific light, set the luminosity level with a transition time, set the default transition time, start comfort."@en ;
                                       <http://www.w3.org/2004/02/skos/core#historyNote> "V3.2.1: Introduced saref:hasInput and saref:hasOutput."@en .


###  https://saref.etsi.org/core/hasMandatoryCommand
<https://saref.etsi.org/core/hasMandatoryCommand> rdf:type owl:ObjectProperty ;
                                                  rdfs:subPropertyOf <https://saref.etsi.org/core/hasCommand> ;
                                                  rdfs:domain <https://saref.etsi.org/core/Function> ;
                                                  owl:propertyChainAxiom ( <http://www.w3.org/2004/02/skos/core#broader>
                                                                           <https://saref.etsi.org/core/hasMandatoryCommand>
                                                                         ) ;
                                                  rdfs:comment "Links a function and one of its mandatory commands"@en ;
                                                  rdfs:label "has mandatory command"@en ;
                                                  <http://www.w3.org/2004/02/skos/core#historyNote> "V3.2.1: Introduced mandatory and optional commands."@en .


###  https://saref.etsi.org/core/hasOperation
<https://saref.etsi.org/core/hasOperation> rdf:type owl:ObjectProperty ;
                                           owl:inverseOf <https://saref.etsi.org/core/isOperationOf> ;
                                           rdfs:domain <https://saref.etsi.org/core/Service> ;
                                           rdfs:range <https://saref.etsi.org/core/Operation> ;
                                           rdfs:comment "Links a service to one of its operations."@en ;
                                           rdfs:label "has operation"@en .


###  https://saref.etsi.org/core/hasOptionalCommand
<https://saref.etsi.org/core/hasOptionalCommand> rdf:type owl:ObjectProperty ;
                                                 rdfs:subPropertyOf <https://saref.etsi.org/core/hasCommand> ;
                                                 rdfs:domain <https://saref.etsi.org/core/Function> ;
                                                 rdfs:comment "Links a function and one of its optional commands"@en ;
                                                 rdfs:label "has optional command"@en .


###  https://saref.etsi.org/core/hasOutput
<https://saref.etsi.org/core/hasOutput> rdf:type owl:ObjectProperty ;
                                        rdfs:domain [ rdf:type owl:Class ;
                                                      owl:unionOf ( <https://saref.etsi.org/core/Command>
                                                                    <https://saref.etsi.org/core/CommandOfInterest>
                                                                    <https://saref.etsi.org/core/Operation>
                                                                  )
                                                    ] ;
                                        rdfs:comment "Links a command or operation to its outputs."@en ;
                                        rdfs:label "has output"@en ;
                                        <http://www.w3.org/2004/02/skos/core#example> "Different complementary commands can be defined for observing a smart home. Observe the temperature once will output the indoor temperature property; observe status of the entry door will output an open/close state."@en .


###  https://saref.etsi.org/core/hasPhenomenonTime
<https://saref.etsi.org/core/hasPhenomenonTime> rdf:type owl:ObjectProperty ;
                                                rdfs:range <http://www.w3.org/2006/time#TemporalEntity> ;
                                                rdfs:comment "Links a procedure execution to the time that the result applies. It may be an interval or an instant, or some other compound temporal entity expressed using OWL Time."@en ;
                                                rdfs:label "has phenomenon time"@en ;
                                                <http://www.w3.org/2004/02/skos/core#historyNote> "V3.2.1: Introduced saref:hasPhenomenonTime as part of general will to make SAREF and SOSA/SSN converge."@en .


###  https://saref.etsi.org/core/hasProfile
<https://saref.etsi.org/core/hasProfile> rdf:type owl:ObjectProperty ;
                                         owl:inverseOf <https://saref.etsi.org/core/isProfileOf> ;
                                         rdfs:domain [ rdf:type owl:Class ;
                                                       owl:unionOf ( <https://saref.etsi.org/core/Device>
                                                                     <https://saref.etsi.org/core/DeviceKind>
                                                                   )
                                                     ] ;
                                         rdfs:range <https://saref.etsi.org/core/Profile> ;
                                         rdfs:comment "Links a device to its profile. Its inverse is saref:isProfileOf. The device should be linked to a certain commodity using OP saref:consumes, saref:produces, or saref:stores, and optionally to some property or state using OP saref:targets or its sub-properties."@en ;
                                         rdfs:label "has profile"@en ;
                                         <http://www.w3.org/2004/02/skos/core#historyNote> "V3.2.1: Relaxed domain of saref:hasProfile to saref:FeatureKind or saref:Device"@en .


###  https://saref.etsi.org/core/hasProperty
<https://saref.etsi.org/core/hasProperty> rdf:type owl:ObjectProperty ;
                                          owl:inverseOf <https://saref.etsi.org/core/isPropertyOf> ;
                                          rdfs:domain [ rdf:type owl:Class ;
                                                        owl:unionOf ( <https://saref.etsi.org/core/FeatureKind>
                                                                      <https://saref.etsi.org/core/FeatureOfInterest>
                                                                    )
                                                      ] ;
                                          rdfs:range <https://saref.etsi.org/core/Property> ;
                                          owl:propertyChainAxiom ( <http://www.w3.org/2004/02/skos/core#broader>
                                                                   <https://saref.etsi.org/core/hasProperty>
                                                                 ) ,
                                                                 ( <https://saref.etsi.org/core/hasFeatureKind>
                                                                   <https://saref.etsi.org/core/hasProperty>
                                                                 ) ,
                                                                 ( <https://saref.etsi.org/core/hasProperty>
                                                                   <https://saref.etsi.org/core/consistsOf>
                                                                 ) ,
                                                                 ( <https://saref.etsi.org/core/hasPropertyOfInterest>
                                                                   <https://saref.etsi.org/core/hasPropertyKind>
                                                                 ) ;
                                          rdfs:comment "Links a feature kind or a feature of interest to one of its properties."@en ;
                                          rdfs:label "has property"@en ;
                                          <http://www.w3.org/2004/02/skos/core#historyNote> "V3.2.1: applicability of saref:hasProperty is relaxed to also saref:FeatureKind"@en .


###  https://saref.etsi.org/core/hasPropertyKind
<https://saref.etsi.org/core/hasPropertyKind> rdf:type owl:ObjectProperty ;
                                              rdfs:domain <https://saref.etsi.org/core/PropertyOfInterest> ;
                                              rdfs:range <https://saref.etsi.org/core/Property> ;
                                              owl:propertyChainAxiom ( <https://saref.etsi.org/core/hasPropertyKind>
                                                                       <http://www.w3.org/2004/02/skos/core#broader>
                                                                     ) ;
                                              rdfs:comment "links a property of interest to its kind, a property."@en ;
                                              rdfs:label "has property kind"@en .


###  https://saref.etsi.org/core/hasPropertyOfInterest
<https://saref.etsi.org/core/hasPropertyOfInterest> rdf:type owl:ObjectProperty ;
                                                    owl:inverseOf <https://saref.etsi.org/core/isPropertyOfInterestOf> ;
                                                    rdfs:domain <https://saref.etsi.org/core/FeatureOfInterest> ;
                                                    rdfs:range <https://saref.etsi.org/core/PropertyOfInterest> ;
                                                    rdfs:comment "Links a feature of interest to one of its properties of interest."@en ;
                                                    rdfs:label "has property of interest"@en ;
                                                    <http://www.w3.org/2004/02/skos/core#historyNote> "V3.2.1: Introduced saref:hasPropertyOfInterest and saref:isPropertyOfInterestOf. Cannot use saref:hasProperty due to the combination of cardinality restrictions and sub-property chain axioms makes the ontology exist the OWL 2 DL prodile."@en .


###  https://saref.etsi.org/core/hasPropertyValue
<https://saref.etsi.org/core/hasPropertyValue> rdf:type owl:ObjectProperty ;
                                               rdfs:domain [ rdf:type owl:Class ;
                                                             owl:unionOf ( <https://saref.etsi.org/core/FeatureKind>
                                                                           <https://saref.etsi.org/core/FeatureOfInterest>
                                                                           <https://saref.etsi.org/core/PropertyOfInterest>
                                                                         )
                                                           ] ;
                                               rdfs:range <https://saref.etsi.org/core/PropertyValue> ;
                                               owl:propertyChainAxiom ( <http://www.w3.org/2004/02/skos/core#broader>
                                                                        <https://saref.etsi.org/core/hasPropertyValue>
                                                                      ) ;
                                               rdfs:comment "Links a feature kind, a feature of interest, or a property of interest, to a property value."@en ;
                                               rdfs:label "has property value"@en ;
                                               <http://www.w3.org/2004/02/skos/core#historyNote> "V3.2.1: Introduced saref:hasPropertyValue."@en .


###  https://saref.etsi.org/core/hasResult
<https://saref.etsi.org/core/hasResult> rdf:type owl:ObjectProperty ;
                                        rdfs:domain <https://saref.etsi.org/core/ProcedureExecution> ;
                                        rdfs:comment "Links a procedure execution (e.g., an observation) to its result (e.g., a property value)."@en ;
                                        rdfs:label "has result"@en ;
                                        <http://www.w3.org/2004/02/skos/core#historyNote> "V3.2.1: Introduced saref:hasResult as part of general will to make SAREF and SOSA/SSN converge."@en .


###  https://saref.etsi.org/core/hasState
<https://saref.etsi.org/core/hasState> rdf:type owl:ObjectProperty ;
                                       owl:inverseOf <https://saref.etsi.org/core/isStateOf> ;
                                       rdfs:domain [ rdf:type owl:Class ;
                                                     owl:unionOf ( <https://saref.etsi.org/core/FeatureKind>
                                                                   <https://saref.etsi.org/core/FeatureOfInterest>
                                                                   <https://saref.etsi.org/core/StateOfInterest>
                                                                 )
                                                   ] ;
                                       rdfs:range <https://saref.etsi.org/core/State> ;
                                       owl:propertyChainAxiom ( <http://www.w3.org/2004/02/skos/core#broader>
                                                                <https://saref.etsi.org/core/hasState>
                                                              ) ,
                                                              ( <https://saref.etsi.org/core/hasFeatureKind>
                                                                <https://saref.etsi.org/core/hasState>
                                                              ) ,
                                                              ( <https://saref.etsi.org/core/hasStateOfInterest>
                                                                <https://saref.etsi.org/core/hasStateKind>
                                                              ) ;
                                       rdfs:comment "Links a feature kind or a feature of interest to one of its states."@en ;
                                       rdfs:label "has state"@en ;
                                       <http://www.w3.org/2004/02/skos/core#historyNote> "V3.2.1: Relaxed domain of saref:hasState."@en .


###  https://saref.etsi.org/core/hasStateKind
<https://saref.etsi.org/core/hasStateKind> rdf:type owl:ObjectProperty ;
                                           rdfs:domain <https://saref.etsi.org/core/StateOfInterest> ;
                                           rdfs:range <https://saref.etsi.org/core/State> ;
                                           owl:propertyChainAxiom ( <https://saref.etsi.org/core/hasStateKind>
                                                                    <http://www.w3.org/2004/02/skos/core#broader>
                                                                  ) ;
                                           rdfs:comment "links a state of interest to its kind, a state"@en ;
                                           rdfs:label "has state kind"@en .


###  https://saref.etsi.org/core/hasStateOfInterest
<https://saref.etsi.org/core/hasStateOfInterest> rdf:type owl:ObjectProperty ;
                                                 owl:inverseOf <https://saref.etsi.org/core/isStateOfInterestOf> ;
                                                 rdfs:domain <https://saref.etsi.org/core/FeatureOfInterest> ;
                                                 rdfs:range <https://saref.etsi.org/core/StateOfInterest> ;
                                                 rdfs:comment "Links a feature of interest to one of its states of interest."@en ;
                                                 rdfs:label "has state of interest"@en ;
                                                 <http://www.w3.org/2004/02/skos/core#historyNote> "V3.2.1: Introduced saref:hasStateOfInterest and saref:isStateOfInterestOf, parallel to saref:hasPropertyOfInterest and saref:isPropertyOfInterestOf."@en .


###  https://saref.etsi.org/core/hasStateValue
<https://saref.etsi.org/core/hasStateValue> rdf:type owl:ObjectProperty ;
                                            rdfs:domain [ rdf:type owl:Class ;
                                                          owl:unionOf ( <https://saref.etsi.org/core/FeatureKind>
                                                                        <https://saref.etsi.org/core/FeatureOfInterest>
                                                                        <https://saref.etsi.org/core/StateOfInterest>
                                                                      )
                                                        ] ;
                                            rdfs:range <https://saref.etsi.org/core/StateValue> ;
                                            owl:propertyChainAxiom ( <http://www.w3.org/2004/02/skos/core#broader>
                                                                     <https://saref.etsi.org/core/hasStateValue>
                                                                   ) ;
                                            rdfs:comment "Links a feature kind, a feature of interest, or a state of interest, to a state value."@en ;
                                            rdfs:label "has state value"@en ;
                                            <http://www.w3.org/2004/02/skos/core#historyNote> "V4.1.1: Introduced saref:hasStateValue."@en .


###  https://saref.etsi.org/core/isAccomplishedBy
<https://saref.etsi.org/core/isAccomplishedBy> rdf:type owl:ObjectProperty ;
                                               rdfs:domain <https://saref.etsi.org/core/Task> ;
                                               rdfs:comment "A relationship identifying an entity (e.g., a device) that can accomplish a task."@en ;
                                               rdfs:label "is accomplished by"@en .


###  https://saref.etsi.org/core/isCommandOf
<https://saref.etsi.org/core/isCommandOf> rdf:type owl:ObjectProperty ;
                                          rdfs:domain <https://saref.etsi.org/core/Command> ;
                                          rdfs:range [ rdf:type owl:Class ;
                                                       owl:unionOf ( <https://saref.etsi.org/core/Function>
                                                                     <https://saref.etsi.org/core/FunctionOfInterest>
                                                                   )
                                                     ] ;
                                          rdfs:comment "Links a command and a function or function of interest that supports it."@en ;
                                          rdfs:label "is command of"@en .


###  https://saref.etsi.org/core/isCommandOfInterestOf
<https://saref.etsi.org/core/isCommandOfInterestOf> rdf:type owl:ObjectProperty ,
                                                             owl:FunctionalProperty ;
                                                    rdfs:domain <https://saref.etsi.org/core/CommandOfInterest> ;
                                                    rdfs:range <https://saref.etsi.org/core/FunctionOfInterest> ;
                                                    rdfs:comment "Links a command of interest to the function of interest it is a command of."@en ;
                                                    rdfs:label "is command of interest of"@en .


###  https://saref.etsi.org/core/isConsumedBy
<https://saref.etsi.org/core/isConsumedBy> rdf:type owl:ObjectProperty ;
                                           rdfs:domain <https://saref.etsi.org/core/Commodity> ;
                                           rdfs:range [ rdf:type owl:Class ;
                                                        owl:unionOf ( <https://saref.etsi.org/core/Device>
                                                                      <https://saref.etsi.org/core/DeviceKind>
                                                                      <https://saref.etsi.org/core/FeatureKind>
                                                                      <https://saref.etsi.org/core/FeatureOfInterest>
                                                                    )
                                                      ] ;
                                           rdfs:comment "Links a commodity to the feature kind, feature of interest, or device, that consumes it"@en ;
                                           rdfs:label "is consumed by"@en .


###  https://saref.etsi.org/core/isControlledBy
<https://saref.etsi.org/core/isControlledBy> rdf:type owl:ObjectProperty ;
                                             rdfs:subPropertyOf <https://saref.etsi.org/core/isTargetOf> ;
                                             rdfs:comment "Links a feature, property, or state, to the device, function, command, or procedure execution, that controls it."@en ;
                                             rdfs:label "is controlled by"@en ;
                                             <http://www.w3.org/2004/02/skos/core#historyNote> "V3.2.1: Introduced property saref:isControlledBy."@en .


###  https://saref.etsi.org/core/isExecutionOf
<https://saref.etsi.org/core/isExecutionOf> rdf:type owl:ObjectProperty ;
                                            rdfs:domain <https://saref.etsi.org/core/ProcedureExecution> ;
                                            rdfs:range [ rdf:type owl:Class ;
                                                         owl:unionOf ( <https://saref.etsi.org/core/Command>
                                                                       <https://saref.etsi.org/core/CommandOfInterest>
                                                                       <https://saref.etsi.org/core/Operation>
                                                                     )
                                                       ] ;
                                            owl:propertyChainAxiom ( <https://saref.etsi.org/core/isExecutionOf>
                                                                     <http://www.w3.org/2004/02/skos/core#broader>
                                                                   ) ,
                                                                   ( <https://saref.etsi.org/core/isExecutionOf>
                                                                     <https://saref.etsi.org/core/hasCommandKind>
                                                                   ) ;
                                            rdfs:comment "Links a command execution to the command or command of interest that was executed. Also liks an operation execution to the operation that was executed"@en ;
                                            rdfs:label "is execution of"@en .


###  https://saref.etsi.org/core/isFunctionOf
<https://saref.etsi.org/core/isFunctionOf> rdf:type owl:ObjectProperty ;
                                           rdfs:domain <https://saref.etsi.org/core/Function> ;
                                           rdfs:range [ rdf:type owl:Class ;
                                                        owl:unionOf ( <https://saref.etsi.org/core/FeatureKind>
                                                                      <https://saref.etsi.org/core/FeatureOfInterest>
                                                                    )
                                                      ] ;
                                           rdfs:comment "Links a function to the feature kind or device it is a function of."@en ;
                                           rdfs:label "is function of"@en ;
                                           <http://www.w3.org/2004/02/skos/core#historyNote> "V3.2.1: Introduced saref:isFunctionOf."@en .


###  https://saref.etsi.org/core/isFunctionOfInterestOf
<https://saref.etsi.org/core/isFunctionOfInterestOf> rdf:type owl:ObjectProperty ,
                                                              owl:FunctionalProperty ;
                                                     rdfs:domain <https://saref.etsi.org/core/FunctionOfInterest> ;
                                                     rdfs:range <https://saref.etsi.org/core/Device> ;
                                                     rdfs:comment "Links a function of interest to the device it is a function of."@en ;
                                                     rdfs:label "is function of interest of"@en .


###  https://saref.etsi.org/core/isMeasuredIn
<https://saref.etsi.org/core/isMeasuredIn> rdf:type owl:ObjectProperty ;
                                           rdfs:range <https://saref.etsi.org/core/UnitOfMeasure> ;
                                           rdfs:comment "A relationship identifying the unit of measure used for a certain entity."@en ;
                                           rdfs:label "is measured in"@en ;
                                           <http://www.w3.org/2004/02/skos/core#historyNote> "V3.2.1: Relaxed domain of saref:isMeasuredIn so it can apply to saref:PropertyValue as well as saref:Measurement. The new range will be enforced in the next major revision of SAREF."@en .


###  https://saref.etsi.org/core/isObservedBy
<https://saref.etsi.org/core/isObservedBy> rdf:type owl:ObjectProperty ;
                                           rdfs:subPropertyOf <https://saref.etsi.org/core/isTargetOf> ;
                                           owl:inverseOf <https://saref.etsi.org/core/observes> ;
                                           rdfs:comment "Links a feature, property, or state, to the device, function, command, or procedure execution, that observes it."@en ;
                                           rdfs:label "is observed by"@en .


###  https://saref.etsi.org/core/isOfferedBy
<https://saref.etsi.org/core/isOfferedBy> rdf:type owl:ObjectProperty ;
                                          owl:inverseOf <https://saref.etsi.org/core/offers> ;
                                          rdf:type owl:FunctionalProperty ;
                                          rdfs:domain <https://saref.etsi.org/core/Service> ;
                                          rdfs:range <https://saref.etsi.org/core/Device> ;
                                          rdfs:comment "Links a service to the device that exposes it to a network"@en ;
                                          rdfs:label "is offered by"@en ;
                                          <http://www.w3.org/2004/02/skos/core#historyNote> "V3.2.1: Clarified definition of saref:isOfferedBy."@en .


###  https://saref.etsi.org/core/isOperationOf
<https://saref.etsi.org/core/isOperationOf> rdf:type owl:ObjectProperty ,
                                                     owl:FunctionalProperty ;
                                            rdfs:domain <https://saref.etsi.org/core/Operation> ;
                                            rdfs:range <https://saref.etsi.org/core/Service> ;
                                            rdfs:comment "Links an operation to the service it belongs to."@en ;
                                            rdfs:label "is operation of"@en .


###  https://saref.etsi.org/core/isProducedBy
<https://saref.etsi.org/core/isProducedBy> rdf:type owl:ObjectProperty ;
                                           owl:inverseOf <https://saref.etsi.org/core/produces> ;
                                           rdfs:domain <https://saref.etsi.org/core/Commodity> ;
                                           rdfs:range [ rdf:type owl:Class ;
                                                        owl:unionOf ( <https://saref.etsi.org/core/Device>
                                                                      <https://saref.etsi.org/core/DeviceKind>
                                                                      <https://saref.etsi.org/core/FeatureKind>
                                                                      <https://saref.etsi.org/core/FeatureOfInterest>
                                                                    )
                                                      ] ;
                                           rdfs:comment "Links a commodity to the feature kind, feature of interest, or device, that produces it"@en ;
                                           rdfs:label "is produced by"@en .


###  https://saref.etsi.org/core/isProfileOf
<https://saref.etsi.org/core/isProfileOf> rdf:type owl:ObjectProperty ;
                                          rdfs:domain <https://saref.etsi.org/core/Profile> ;
                                          rdfs:range [ rdf:type owl:Class ;
                                                       owl:unionOf ( <https://saref.etsi.org/core/Device>
                                                                     <https://saref.etsi.org/core/DeviceKind>
                                                                   )
                                                     ] ;
                                          rdfs:comment "Links a profile to the device it describes. The device should be linked to a certain commodity using OP saref:consumes, saref:produces, or saref:stores, and optionally to some property or state using OP saref:targets or its sub-properties."@en ;
                                          rdfs:label "is profile of"@en .


###  https://saref.etsi.org/core/isPropertyOf
<https://saref.etsi.org/core/isPropertyOf> rdf:type owl:ObjectProperty ;
                                           rdfs:domain <https://saref.etsi.org/core/Property> ;
                                           rdfs:range [ rdf:type owl:Class ;
                                                        owl:unionOf ( <https://saref.etsi.org/core/FeatureKind>
                                                                      <https://saref.etsi.org/core/FeatureOfInterest>
                                                                    )
                                                      ] ;
                                           rdfs:comment "Links a property to the feature kind or feature of interest it is a property of."@en ;
                                           rdfs:label "is property of"@en .


###  https://saref.etsi.org/core/isPropertyOfInterestOf
<https://saref.etsi.org/core/isPropertyOfInterestOf> rdf:type owl:ObjectProperty ,
                                                              owl:FunctionalProperty ;
                                                     rdfs:domain <https://saref.etsi.org/core/PropertyOfInterest> ;
                                                     rdfs:range <https://saref.etsi.org/core/FeatureOfInterest> ;
                                                     rdfs:comment "Links a property of interest to the feature of interest it is a property of."@en ;
                                                     rdfs:label "is property of interest of"@en .


###  https://saref.etsi.org/core/isStateOf
<https://saref.etsi.org/core/isStateOf> rdf:type owl:ObjectProperty ;
                                        rdfs:domain <https://saref.etsi.org/core/State> ;
                                        rdfs:range [ rdf:type owl:Class ;
                                                     owl:unionOf ( <https://saref.etsi.org/core/FeatureKind>
                                                                   <https://saref.etsi.org/core/FeatureOfInterest>
                                                                 )
                                                   ] ;
                                        rdfs:comment "Links a state to the feature kind or feature of interest it is a state of."@en ;
                                        rdfs:label "is state of"@en ;
                                        <http://www.w3.org/2004/02/skos/core#historyNote> "V3.2.1: Introduced saref:isStateOf."@en .


###  https://saref.etsi.org/core/isStateOfInterestOf
<https://saref.etsi.org/core/isStateOfInterestOf> rdf:type owl:ObjectProperty ,
                                                           owl:FunctionalProperty ;
                                                  rdfs:domain <https://saref.etsi.org/core/StateOfInterest> ;
                                                  rdfs:range <https://saref.etsi.org/core/FeatureOfInterest> ;
                                                  rdfs:comment "Links a state of interest to the feature of interest it is a state of."@en ;
                                                  rdfs:label "is state of interest of"@en .


###  https://saref.etsi.org/core/isStoredBy
<https://saref.etsi.org/core/isStoredBy> rdf:type owl:ObjectProperty ;
                                         owl:inverseOf <https://saref.etsi.org/core/stores> ;
                                         rdfs:domain <https://saref.etsi.org/core/Commodity> ;
                                         rdfs:range [ rdf:type owl:Class ;
                                                      owl:unionOf ( <https://saref.etsi.org/core/Device>
                                                                    <https://saref.etsi.org/core/DeviceKind>
                                                                    <https://saref.etsi.org/core/FeatureKind>
                                                                    <https://saref.etsi.org/core/FeatureOfInterest>
                                                                  )
                                                    ] ;
                                         rdfs:comment "Links a commodity to the feature kind, feature of interest, or device, that stores it"@en ;
                                         rdfs:label "is stored by"@en .


###  https://saref.etsi.org/core/isTargetOf
<https://saref.etsi.org/core/isTargetOf> rdf:type owl:ObjectProperty ;
                                         owl:inverseOf <https://saref.etsi.org/core/targets> ;
                                         rdfs:domain [ rdf:type owl:Class ;
                                                       owl:unionOf ( <https://saref.etsi.org/core/FeatureKind>
                                                                     <https://saref.etsi.org/core/FeatureOfInterest>
                                                                     <https://saref.etsi.org/core/Property>
                                                                     <https://saref.etsi.org/core/PropertyOfInterest>
                                                                     <https://saref.etsi.org/core/State>
                                                                     <https://saref.etsi.org/core/StateOfInterest>
                                                                   )
                                                     ] ;
                                         rdfs:range [ rdf:type owl:Class ;
                                                      owl:unionOf ( <https://saref.etsi.org/core/Command>
                                                                    <https://saref.etsi.org/core/CommandOfInterest>
                                                                    <https://saref.etsi.org/core/Device>
                                                                    <https://saref.etsi.org/core/DeviceKind>
                                                                    <https://saref.etsi.org/core/Function>
                                                                    <https://saref.etsi.org/core/FunctionOfInterest>
                                                                    <https://saref.etsi.org/core/ProcedureExecution>
                                                                  )
                                                    ] ;
                                         rdfs:comment "Links a feature, property, or state, to the device, function, command, or procedure execution, that targets it."@en ;
                                         rdfs:label "is target of"@en ;
                                         <http://www.w3.org/2004/02/skos/core#historyNote> "V3.2.1: Introduced property saref:isActedUponBy."@en ,
                                                                                           "V4.1.1: Renamed property saref:isActedUponBy into saref:isTargetOf."@en .


###  https://saref.etsi.org/core/isValueOfProperty
<https://saref.etsi.org/core/isValueOfProperty> rdf:type owl:ObjectProperty ;
                                                rdfs:domain <https://saref.etsi.org/core/PropertyValue> ;
                                                rdfs:range [ rdf:type owl:Class ;
                                                             owl:unionOf ( <https://saref.etsi.org/core/FeatureKind>
                                                                           <https://saref.etsi.org/core/FeatureOfInterest>
                                                                           <https://saref.etsi.org/core/Property>
                                                                           <https://saref.etsi.org/core/PropertyOfInterest>
                                                                         )
                                                           ] ;
                                                owl:propertyChainAxiom ( <https://saref.etsi.org/core/isValueOfProperty>
                                                                         <https://saref.etsi.org/core/hasPropertyKind>
                                                                       ) ;
                                                rdfs:comment "Links a property value to the property or property of interest it is a value of."@en ;
                                                rdfs:label "is value of property"@en ;
                                                <http://www.w3.org/2004/02/skos/core#historyNote> "V3.2.1: Introduced saref:isValueOfProperty."@en .


###  https://saref.etsi.org/core/isValueOfState
<https://saref.etsi.org/core/isValueOfState> rdf:type owl:ObjectProperty ;
                                             rdfs:domain <https://saref.etsi.org/core/StateValue> ;
                                             rdfs:range [ rdf:type owl:Class ;
                                                          owl:unionOf ( <https://saref.etsi.org/core/FeatureKind>
                                                                        <https://saref.etsi.org/core/FeatureOfInterest>
                                                                        <https://saref.etsi.org/core/StateOfInterest>
                                                                      )
                                                        ] ;
                                             owl:propertyChainAxiom ( <https://saref.etsi.org/core/isValueOfState>
                                                                      <https://saref.etsi.org/core/hasStateKind>
                                                                    ) ;
                                             rdfs:comment "Links a state value to the state or state of interest it is a value of."@en ;
                                             rdfs:label "is value of state"@en ;
                                             <http://www.w3.org/2004/02/skos/core#historyNote> "V4.1.1: Introduced saref:isValueOfState."@en .


###  https://saref.etsi.org/core/madeBy
<https://saref.etsi.org/core/madeBy> rdf:type owl:ObjectProperty ;
                                     owl:inverseOf <https://saref.etsi.org/core/madeExecution> ;
                                     rdfs:domain <https://saref.etsi.org/core/ProcedureExecution> ;
                                     rdfs:range <https://saref.etsi.org/core/FeatureOfInterest> ;
                                     rdfs:comment "Links a procedure execution to the entity (e.g., device) that made it."@en ;
                                     rdfs:label "made by"@en ;
                                     <http://www.w3.org/2004/02/skos/core#historyNote> "V3.2.1: Introduce saref:madeBy (resp. saref:madeExecution) as generalization of saref:measurementMadeBy (resp. saref:makesMeasurement)."@en .


###  https://saref.etsi.org/core/madeExecution
<https://saref.etsi.org/core/madeExecution> rdf:type owl:ObjectProperty ;
                                            rdfs:domain <https://saref.etsi.org/core/FeatureOfInterest> ;
                                            rdfs:range <https://saref.etsi.org/core/ProcedureExecution> ;
                                            rdfs:comment "Links an entity (e.g., device) to the procedure execution it made."@en ;
                                            rdfs:label "made execution"@en .


###  https://saref.etsi.org/core/observes
<https://saref.etsi.org/core/observes> rdf:type owl:ObjectProperty ;
                                       rdfs:subPropertyOf <https://saref.etsi.org/core/targets> ;
                                       rdfs:domain [ rdf:type owl:Class ;
                                                     owl:unionOf ( <https://saref.etsi.org/core/Command>
                                                                   <https://saref.etsi.org/core/CommandOfInterest>
                                                                   <https://saref.etsi.org/core/DeviceKind>
                                                                   <https://saref.etsi.org/core/Function>
                                                                   <https://saref.etsi.org/core/FunctionOfInterest>
                                                                   <https://saref.etsi.org/core/Observation>
                                                                   <https://saref.etsi.org/core/Sensor>
                                                                 )
                                                   ] ;
                                       rdfs:comment "Links a device, function, command, or procedure execution, to the feature, property, or state, it observes."@en ;
                                       rdfs:label "observes"@en ;
                                       <http://www.w3.org/2004/02/skos/core#historyNote> "V3.2.1: Introduced property saref:observes, as sub-property of saref:targets. and generalization of measures."@en .


###  https://saref.etsi.org/core/offers
<https://saref.etsi.org/core/offers> rdf:type owl:ObjectProperty ;
                                     rdfs:domain <https://saref.etsi.org/core/Device> ;
                                     rdfs:range <https://saref.etsi.org/core/Service> ;
                                     rdfs:comment "Links a device to a service it exposes to a network."@en ;
                                     rdfs:label "offers"@en ;
                                     <http://www.w3.org/2004/02/skos/core#historyNote> "V3.2.1: Clarified definition of saref:offers."@en .


###  https://saref.etsi.org/core/produces
<https://saref.etsi.org/core/produces> rdf:type owl:ObjectProperty ;
                                       rdfs:domain [ rdf:type owl:Class ;
                                                     owl:unionOf ( <https://saref.etsi.org/core/Device>
                                                                   <https://saref.etsi.org/core/DeviceKind>
                                                                   <https://saref.etsi.org/core/FeatureKind>
                                                                   <https://saref.etsi.org/core/FeatureOfInterest>
                                                                 )
                                                   ] ;
                                       rdfs:range <https://saref.etsi.org/core/Commodity> ;
                                       rdfs:comment "Links a feature kind, feature of interest, or device, to the commodity it produces"@en ;
                                       rdfs:label "produces"@en .


###  https://saref.etsi.org/core/profileHasPrice
<https://saref.etsi.org/core/profileHasPrice> rdf:type owl:ObjectProperty ;
                                              rdfs:domain <https://saref.etsi.org/core/Profile> ;
                                              rdfs:range <https://saref.etsi.org/core/PropertyValue> ;
                                              rdfs:comment "Links a profile to the money earned (negative values) or paid (positive values) for the use (production or consumption) of the commodity by the device"@en ;
                                              rdfs:label "has price"@en .


###  https://saref.etsi.org/core/represents
<https://saref.etsi.org/core/represents> rdf:type owl:ObjectProperty ;
                                         rdfs:domain [ rdf:type owl:Class ;
                                                       owl:unionOf ( <https://saref.etsi.org/core/Operation>
                                                                     <https://saref.etsi.org/core/Service>
                                                                   )
                                                     ] ;
                                         rdfs:range [ rdf:type owl:Class ;
                                                      owl:unionOf ( <https://saref.etsi.org/core/Command>
                                                                    <https://saref.etsi.org/core/CommandOfInterest>
                                                                    <https://saref.etsi.org/core/Function>
                                                                    <https://saref.etsi.org/core/FunctionOfInterest>
                                                                  )
                                                    ] ;
                                         rdfs:comment "Links a service to some function or function of interest it exposes to the network. Also links an operation to some command or command of interest it exposes to the network."@en ;
                                         rdfs:label "represents"@en ;
                                         <http://www.w3.org/2004/02/skos/core#historyNote> "V3.2.1: Relaxed domain and range of saref:represents."@en .


###  https://saref.etsi.org/core/stores
<https://saref.etsi.org/core/stores> rdf:type owl:ObjectProperty ;
                                     rdfs:domain [ rdf:type owl:Class ;
                                                   owl:unionOf ( <https://saref.etsi.org/core/Device>
                                                                 <https://saref.etsi.org/core/DeviceKind>
                                                                 <https://saref.etsi.org/core/FeatureKind>
                                                                 <https://saref.etsi.org/core/FeatureOfInterest>
                                                               )
                                                 ] ;
                                     rdfs:range <https://saref.etsi.org/core/Commodity> ;
                                     rdfs:comment "Links a feature kind, feature of interest, or device, to the commodity it stores"@en ;
                                     rdfs:label "stores"@en .


###  https://saref.etsi.org/core/targets
<https://saref.etsi.org/core/targets> rdf:type owl:ObjectProperty ;
                                      rdfs:domain [ rdf:type owl:Class ;
                                                    owl:unionOf ( <https://saref.etsi.org/core/Command>
                                                                  <https://saref.etsi.org/core/CommandOfInterest>
                                                                  <https://saref.etsi.org/core/Device>
                                                                  <https://saref.etsi.org/core/DeviceKind>
                                                                  <https://saref.etsi.org/core/Function>
                                                                  <https://saref.etsi.org/core/FunctionOfInterest>
                                                                  <https://saref.etsi.org/core/ProcedureExecution>
                                                                )
                                                  ] ;
                                      rdfs:range [ rdf:type owl:Class ;
                                                   owl:unionOf ( <https://saref.etsi.org/core/FeatureKind>
                                                                 <https://saref.etsi.org/core/FeatureOfInterest>
                                                                 <https://saref.etsi.org/core/Property>
                                                                 <https://saref.etsi.org/core/PropertyOfInterest>
                                                                 <https://saref.etsi.org/core/State>
                                                                 <https://saref.etsi.org/core/StateOfInterest>
                                                               )
                                                 ] ;
                                      rdfs:comment "Links a device, function, command, or procedure execution, to the feature, property, or state, it targets."@en ;
                                      rdfs:label "targets"@en ;
                                      <http://www.w3.org/2004/02/skos/core#historyNote> "V3.2.1: saref:actsUpon now holds not only between a command and a state. It generalizes observes, observes, controls. Domain and range are unions of several classes."@en ,
                                                                                        "V4.1.1: saref:actsUpon is renamed saref:targets."@en .


###  https://saref.etsi.org/core/whenPropertyValue
<https://saref.etsi.org/core/whenPropertyValue> rdf:type owl:ObjectProperty ;
                                                rdfs:domain <https://saref.etsi.org/core/Profile> ;
                                                rdfs:range <https://saref.etsi.org/core/PropertyValue> ;
                                                rdfs:comment "Links a profile to a property value that contributes to restricting its applicable context."@en ;
                                                rdfs:label "when property value"@en .


###  https://saref.etsi.org/core/whenState
<https://saref.etsi.org/core/whenState> rdf:type owl:ObjectProperty ;
                                        rdfs:domain <https://saref.etsi.org/core/Profile> ;
                                        rdfs:range <https://saref.etsi.org/core/State> ;
                                        rdfs:comment "Links a profile to a state that contributes to restricting its applicable context."@en ;
                                        rdfs:label "when state"@en .


###  https://saref.etsi.org/saref4bldg/contains
<https://saref.etsi.org/saref4bldg/contains> rdf:type owl:ObjectProperty ;
                                             owl:inverseOf <https://saref.etsi.org/saref4bldg/isContainedIn> ;
                                             rdf:type owl:TransitiveProperty ;
                                             rdfs:domain <https://saref.etsi.org/saref4bldg/PhysicalObject> ;
                                             rdfs:range <https://saref.etsi.org/saref4bldg/PhysicalObject> ;
                                             rdfs:comment "A relation between a physical object and another physical object it contains."@en ;
                                             rdfs:label "contains"@en .


###  https://saref.etsi.org/saref4bldg/hasSpace
<https://saref.etsi.org/saref4bldg/hasSpace> rdf:type owl:ObjectProperty ;
                                             owl:inverseOf <https://saref.etsi.org/saref4bldg/isSpaceOf> ;
                                             rdf:type owl:TransitiveProperty ;
                                             rdfs:comment "Relation between a building or a building space and the spaces it can be divided into."@en ;
                                             rdfs:label "has space"@en .


###  https://saref.etsi.org/saref4bldg/isContainedIn
<https://saref.etsi.org/saref4bldg/isContainedIn> rdf:type owl:ObjectProperty ,
                                                           owl:TransitiveProperty ;
                                                  rdfs:domain <https://saref.etsi.org/saref4bldg/PhysicalObject> ;
                                                  rdfs:range <https://saref.etsi.org/saref4bldg/PhysicalObject> ;
                                                  rdfs:comment "A relation between a physical object and the physical space in which it is contained."@en ;
                                                  rdfs:label "is contained in"@en .


###  https://saref.etsi.org/saref4bldg/isSpaceOf
<https://saref.etsi.org/saref4bldg/isSpaceOf> rdf:type owl:ObjectProperty ,
                                                       owl:TransitiveProperty ;
                                              rdfs:comment "Relation between a building space and the building or building space it belongs to."@en ;
                                              rdfs:label "isSpaceOf"@en .


###  https://saref.etsi.org/saref4bldg/nominalSupplyVoltageMax
<https://saref.etsi.org/saref4bldg/nominalSupplyVoltageMax> rdf:type owl:ObjectProperty ;
                                                            rdfs:comment "The maximum and minimum allowed voltage of the supply e.g. boundaries of 380V/440V may be applied for a nominal voltage of 400V."@en ;
                                                            rdfs:label "nominal supply voltage offset"@en .


###  https://saref.etsi.org/saref4bldg/shortCircuitVoltage
<https://saref.etsi.org/saref4bldg/shortCircuitVoltage> rdf:type owl:ObjectProperty ;
                                                        rdfs:comment "A complex number that specifies the real and imaginary parts of the short-circuit voltage at rated current of a transformer given in %."@en ;
                                                        rdfs:label "short circuit voltage"@en .


#################################################################
#    Data properties
#################################################################

###  https://saref.etsi.org/core/hasIdentifier
<https://saref.etsi.org/core/hasIdentifier> rdf:type owl:DatatypeProperty ;
                                            rdfs:comment "Links some entity to its identifier. Extensions of SAREF may define sub-properties such as s4abcd:hasUUID, s4abcd:hasGTIN12, etc."@en ;
                                            rdfs:label "has identifier"@en ;
                                            rdfs:seeAlso <https://labs.etsi.org/rep/saref/saref-portal/-/issues/2> .


###  https://saref.etsi.org/core/hasManufacturer
<https://saref.etsi.org/core/hasManufacturer> rdf:type owl:DatatypeProperty ;
                                              rdfs:domain [ rdf:type owl:Class ;
                                                            owl:unionOf ( <https://saref.etsi.org/core/FeatureKind>
                                                                          <https://saref.etsi.org/core/FeatureOfInterest>
                                                                        )
                                                          ] ;
                                              rdfs:comment "A relationship identifying the manufacturer of an entity (e.g., device). The value is expected to be a string or a string with language tag."@en ;
                                              rdfs:label "has manufacturer"@en ;
                                              <http://www.w3.org/2004/02/skos/core#historyNote> "V3.2.1: Defined domain of saref:hasManufacturer to union of feature kind and feature of interest."@en .


###  https://saref.etsi.org/core/hasModel
<https://saref.etsi.org/core/hasModel> rdf:type owl:DatatypeProperty ;
                                       rdfs:domain [ rdf:type owl:Class ;
                                                     owl:unionOf ( <https://saref.etsi.org/core/FeatureKind>
                                                                   <https://saref.etsi.org/core/FeatureOfInterest>
                                                                 )
                                                   ] ;
                                       rdfs:comment "A relationship identifying the model of an entity (e.g., device). The value is expected to be a string or a string with language tag."@en ;
                                       rdfs:label "has model"@en ;
                                       <http://www.w3.org/2004/02/skos/core#historyNote> "V3.2.1: Defined domain of saref:hasModel to union of feature kind and feature of interest."@en .


###  https://saref.etsi.org/core/hasResultTime
<https://saref.etsi.org/core/hasResultTime> rdf:type owl:DatatypeProperty ;
                                            rdfs:domain <https://saref.etsi.org/core/ProcedureExecution> ;
                                            rdfs:range xsd:dateTime ;
                                            rdfs:comment "Links a procedure execution to the instant of time when the activity was completed, expressed as an xsd:dateTime literal."@en ;
                                            rdfs:label "has result time"@en ;
                                            <http://www.w3.org/2004/02/skos/core#historyNote> "V3.2.1: Introduced saref:hasResultTime as part of general will to make SAREF and SOSA/SSN converge."@en .


###  https://saref.etsi.org/core/hasRevisionNumber
<https://saref.etsi.org/core/hasRevisionNumber> rdf:type owl:DatatypeProperty ;
                                                rdfs:range xsd:string ;
                                                rdfs:comment "Links some entity (e.g., a device) to its revision number."@en ;
                                                rdfs:label "has revision number"@en ;
                                                rdfs:seeAlso <https://labs.etsi.org/rep/saref/saref-core/-/issues/53> .


###  https://saref.etsi.org/core/hasTimestamp
<https://saref.etsi.org/core/hasTimestamp> rdf:type owl:DatatypeProperty ;
                                           rdfs:domain [ rdf:type owl:Class ;
                                                         owl:unionOf ( <https://saref.etsi.org/core/ProcedureExecution>
                                                                       <https://saref.etsi.org/core/Profile>
                                                                     )
                                                       ] ;
                                           rdfs:range xsd:dateTime ;
                                           rdfs:comment "Links a procedure execution or a profile to an instant."@en ;
                                           rdfs:label "has timestamp"@en ;
                                           <http://www.w3.org/2004/02/skos/core#historyNote> "V3.2.1: Tried to clarify definition of saref:hasTimestamp. Still unclear."@en ;
                                           <http://www.w3.org/2004/02/skos/core#note> "Applied on a profile, it describes the applicable instant of that profile"@en ,
                                                                                      "When the execution time and the phenomenon time are the same time instants, then DP saref:hasTimestamp can be used to simply link a procedure execution to the time of these instants, expressed as an xsd:dateTime literal."@en .


###  https://saref.etsi.org/core/hasValue
<https://saref.etsi.org/core/hasValue> rdf:type owl:DatatypeProperty ;
                                       rdfs:comment "Value of a property value expressed as an RDF literal. Note that, even if decimal values are expected, values could use other datatypes."@en ;
                                       rdfs:label "has value"@en ;
                                       <http://www.w3.org/2004/02/skos/core#historyNote> "V3.2.1: Clarified definition of saref:hasValue."@en .


###  https://saref.etsi.org/core/hasVersion
<https://saref.etsi.org/core/hasVersion> rdf:type owl:DatatypeProperty ;
                                         rdfs:range xsd:string ;
                                         rdfs:comment "Links some entity (e.g., a device) to its version."@en ;
                                         rdfs:label "has version"@en ;
                                         rdfs:seeAlso <https://labs.etsi.org/rep/saref/saref-core/-/issues/53> .


###  https://saref.etsi.org/saref4bldg/accessType
<https://saref.etsi.org/saref4bldg/accessType> rdf:type owl:DatatypeProperty ;
                                               rdfs:range xsd:string ;
                                               rdfs:comment "Defines the types of access (or cover) to a tank that may be specified. Note that covers are generally specified for rectangular tanks. For cylindrical tanks, access will normally be via a manhole."@en ;
                                               rdfs:label "access type"@en .


###  https://saref.etsi.org/saref4bldg/application
<https://saref.etsi.org/saref4bldg/application> rdf:type owl:DatatypeProperty ;
                                                rdfs:range xsd:string ;
                                                rdfs:comment "Humidifier application. Fixed: Humidifier installed in a ducted flow distribution system. Portable: Humidifier is not installed in a ducted flow distribution system."@en ;
                                                rdfs:label "application"@en .


###  https://saref.etsi.org/saref4bldg/arrangement
<https://saref.etsi.org/saref4bldg/arrangement> rdf:type owl:DatatypeProperty ;
                                                rdfs:range xsd:string ;
                                                rdfs:comment "Defines the basic flow arrangements for the heat exchanger: COUNTERFLOW: Counterflow heat exchanger arrangement. CROSSFLOW: Crossflow heat exchanger arrangement. PARALLELFLOW: Parallel flow heat exchanger arrangement. MULTIPASS: Multipass flow heat exchanger arrangement. OTHER: Other type of heat exchanger flow arrangement not defined above."@en ;
                                                rdfs:label "arrangement"@en .


###  https://saref.etsi.org/saref4bldg/bladeAction
<https://saref.etsi.org/saref4bldg/bladeAction> rdf:type owl:DatatypeProperty ;
                                                rdfs:range xsd:string ;
                                                rdfs:comment "Blade action."@en ;
                                                rdfs:label "blade action"@en .


###  https://saref.etsi.org/saref4bldg/bladeEdge
<https://saref.etsi.org/saref4bldg/bladeEdge> rdf:type owl:DatatypeProperty ;
                                              rdfs:range xsd:string ;
                                              rdfs:comment "Blade edge."@en ;
                                              rdfs:label "blade edge"@en .


###  https://saref.etsi.org/saref4bldg/bladeShape
<https://saref.etsi.org/saref4bldg/bladeShape> rdf:type owl:DatatypeProperty ;
                                               rdfs:range xsd:string ;
                                               rdfs:comment "Blade shape. Flat means triple V-groove."@en ;
                                               rdfs:label "blade shape"@en .


###  https://saref.etsi.org/saref4bldg/capacityControl
<https://saref.etsi.org/saref4bldg/capacityControl> rdf:type owl:DatatypeProperty ;
                                                    rdfs:range xsd:string ;
                                                    rdfs:comment "FanCycling: Fan is cycled on and off to control duty. TwoSpeedFan: Fan is switched between low and high speed to control duty. VariableSpeedFan: Fan speed is varied to control duty. DampersControl: Dampers modulate the air flow to control duty. BypassValveControl: Bypass valve modulates the water flow to control duty. MultipleSeriesPumps: Turn on/off multiple series pump to control duty. TwoSpeedPump: Switch between high/low pump speed to control duty. VariableSpeedPump: vary pump speed to control duty."@en ;
                                                    rdfs:label "capacity control"@en .


###  https://saref.etsi.org/saref4bldg/capacityControlType
<https://saref.etsi.org/saref4bldg/capacityControlType> rdf:type owl:DatatypeProperty ;
                                                        rdfs:range xsd:string ;
                                                        rdfs:comment "InletVane: Control by adjusting inlet vane. VariableSpeedDrive: Control by variable speed drive. BladePitchAngle: Control by adjusting blade pitch angle. TwoSpeed: Control by switch between high and low speed. DischargeDamper: Control by modulating discharge damper."@en ;
                                                        rdfs:label "capacity control type"@en .


###  https://saref.etsi.org/saref4bldg/capacityPeople
<https://saref.etsi.org/saref4bldg/capacityPeople> rdf:type owl:DatatypeProperty ;
                                                   rdfs:range xsd:nonNegativeInteger ;
                                                   rdfs:comment "Capacity of the transportation element measured in numbers of person."@en ;
                                                   rdfs:label "capacity people"@en .


###  https://saref.etsi.org/saref4bldg/circuitType
<https://saref.etsi.org/saref4bldg/circuitType> rdf:type owl:DatatypeProperty ;
                                                rdfs:range xsd:string ;
                                                rdfs:comment "OpenCircuit: Exposes water directly to the cooling atmosphere. CloseCircuit: The fluid is separated from the atmosphere by a heat exchanger. Wet: The air stream or the heat exchange surface is evaporatively cooled. Dry: No evaporation into the air stream. DryWet: A combination of a dry tower and a wet tower."@en ;
                                                rdfs:label "circuit type"@en .


###  https://saref.etsi.org/saref4bldg/colorAppearance
<https://saref.etsi.org/saref4bldg/colorAppearance> rdf:type owl:DatatypeProperty ;
                                                    rdfs:range xsd:string ;
                                                    rdfs:comment "In both the DIN and CIE standards, artificial light sources are classified in terms of their color appearance. To the human eye they all appear to be white the difference can only be detected by direct comparison. Visual performance is not directly affected by differences in color appearance."@en ;
                                                    rdfs:label "color appearance"@en .


###  https://saref.etsi.org/saref4bldg/colorRenderingIndex
<https://saref.etsi.org/saref4bldg/colorRenderingIndex> rdf:type owl:DatatypeProperty ;
                                                        rdfs:range xsd:integer ;
                                                        rdfs:comment "The CRI indicates how well a light source renders eight standard colors compared to perfect reference lamp with the same color temperature. The CRI scale ranges from 1 to 100, with 100 representing perfect rendering properties."@en ;
                                                        rdfs:label "color rendering index"@en .


###  https://saref.etsi.org/saref4bldg/controlStrategy
<https://saref.etsi.org/saref4bldg/controlStrategy> rdf:type owl:DatatypeProperty ;
                                                    rdfs:range xsd:string ;
                                                    rdfs:comment "FixedExitingWaterTemp: The capacity is controlled to maintain a fixed exiting water temperature. WetBulbTempReset: The set-point is reset based on the wet-bulb temperature."@en ;
                                                    rdfs:label "control strategy"@en .


###  https://saref.etsi.org/saref4bldg/endShapeType
<https://saref.etsi.org/saref4bldg/endShapeType> rdf:type owl:DatatypeProperty ;
                                                 rdfs:range xsd:string ;
                                                 rdfs:comment "Defines the types of end shapes that can be used for preformed tanks. The convention for reading these enumerated values is that for a vertical cylinder, the first value is the base and the second is the top for a horizontal cylinder, the order of reading should be left to right. For a speherical tank, the value UNSET should be used.B5"@en ;
                                                 rdfs:label "end shape type"@en .


###  https://saref.etsi.org/saref4bldg/energySource
<https://saref.etsi.org/saref4bldg/energySource> rdf:type owl:DatatypeProperty ;
                                                 rdfs:range xsd:string ;
                                                 rdfs:comment "Enumeration defining the energy source or fuel cumbusted to generate heat."@en ,
                                                              "The source of energy."@en ;
                                                 rdfs:label "energy source"@en .


###  https://saref.etsi.org/saref4bldg/evaporationCoolant
<https://saref.etsi.org/saref4bldg/evaporationCoolant> rdf:type owl:DatatypeProperty ;
                                                       rdfs:range xsd:string ;
                                                       rdfs:comment "The fluid used for the coolant in the evaporator."@en ;
                                                       rdfs:label "evaporation coolant"@en .


###  https://saref.etsi.org/saref4bldg/evaporationMediumType
<https://saref.etsi.org/saref4bldg/evaporationMediumType> rdf:type owl:DatatypeProperty ;
                                                          rdfs:range xsd:string ;
                                                          rdfs:comment "ColdLiquid: Evaporator is using liquid type of fluid to exchange heat with refrigerant. ColdAir: Evaporator is using air to exchange heat with refrigerant."@en ;
                                                          rdfs:label "evaporation medium type"@en .


###  https://saref.etsi.org/saref4bldg/failPosition
<https://saref.etsi.org/saref4bldg/failPosition> rdf:type owl:DatatypeProperty ;
                                                 rdfs:range xsd:string ;
                                                 rdfs:comment "Specifies the required fail-safe position of the actuator."@en ;
                                                 rdfs:label "fail position"@en .


###  https://saref.etsi.org/saref4bldg/finishColor
<https://saref.etsi.org/saref4bldg/finishColor> rdf:type owl:DatatypeProperty ;
                                                rdfs:range xsd:string ;
                                                rdfs:comment "Finish color for cooled beam."@en ;
                                                rdfs:label "finish color"@en .


###  https://saref.etsi.org/saref4bldg/fireExit
<https://saref.etsi.org/saref4bldg/fireExit> rdf:type owl:DatatypeProperty ;
                                             rdfs:range xsd:boolean ;
                                             rdfs:comment "Indication whether this object is designed to serve as an exit in the case of fire (TRUE) or not (FALSE). Here whether the transport element (in case of e.g., a lift) is designed to serve as a fire exit, e.g., for fire escape purposes."@en ;
                                             rdfs:label "fire exit"@en .


###  https://saref.etsi.org/saref4bldg/flowArrangement
<https://saref.etsi.org/saref4bldg/flowArrangement> rdf:type owl:DatatypeProperty ;
                                                    rdfs:range xsd:string ;
                                                    rdfs:comment "CounterFlow: Air and water flow enter in different directions. CrossFlow: Air and water flow are perpendicular. ParallelFlow: air and water flow enter in same directions."@en ;
                                                    rdfs:label "flow arrangement"@en .


###  https://saref.etsi.org/saref4bldg/frameSize
<https://saref.etsi.org/saref4bldg/frameSize> rdf:type owl:DatatypeProperty ;
                                              rdfs:range xsd:string ;
                                              rdfs:comment "Designation of the frame size according to the named range of frame sizes designated at the place of use or according to a given standard."@en ;
                                              rdfs:label "frame size"@en .


###  https://saref.etsi.org/saref4bldg/frameType
<https://saref.etsi.org/saref4bldg/frameType> rdf:type owl:DatatypeProperty ;
                                              rdfs:range xsd:string ;
                                              rdfs:comment "The type of frame used by the damper (e.g., Standard, Single Flange, Single Reversed Flange, Double Flange, etc.)."@en ;
                                              rdfs:label "frame type"@en .


###  https://saref.etsi.org/saref4bldg/hasDefrost
<https://saref.etsi.org/saref4bldg/hasDefrost> rdf:type owl:DatatypeProperty ;
                                               rdfs:range xsd:boolean ;
                                               rdfs:comment "Whether the heat exchanger has defrost function or not."@en ;
                                               rdfs:label "has defrost"@en .


###  https://saref.etsi.org/saref4bldg/hasExteriorInsulation
<https://saref.etsi.org/saref4bldg/hasExteriorInsulation> rdf:type owl:DatatypeProperty ;
                                                          rdfs:range xsd:boolean ;
                                                          rdfs:comment "TRUE if the silencer has exterior insulation. FALSE if it does not."@en ;
                                                          rdfs:label "has exterior insulation"@en .


###  https://saref.etsi.org/saref4bldg/hasHotGasBypass
<https://saref.etsi.org/saref4bldg/hasHotGasBypass> rdf:type owl:DatatypeProperty ;
                                                    rdfs:range xsd:boolean ;
                                                    rdfs:comment "Whether or not hot gas bypass is provided for the compressor. TRUE = Yes, FALSE = No."@en ;
                                                    rdfs:label "has hot gas bypass"@en .


###  https://saref.etsi.org/saref4bldg/hasLock
<https://saref.etsi.org/saref4bldg/hasLock> rdf:type owl:DatatypeProperty ;
                                            rdfs:range xsd:boolean ;
                                            rdfs:comment "Indication of whether a switching device has a key operated lock (=TRUE) or not (= FALSE)."@en ;
                                            rdfs:label "has lock"@en .


###  https://saref.etsi.org/saref4bldg/hasPartWinding
<https://saref.etsi.org/saref4bldg/hasPartWinding> rdf:type owl:DatatypeProperty ;
                                                   rdfs:range xsd:boolean ;
                                                   rdfs:comment "Indication of whether the motor is single speed, i.e. has a single winding (= FALSE) or multi-speed i.e.has part winding (= TRUE) ."@en ;
                                                   rdfs:label "has part winding"@en .


###  https://saref.etsi.org/saref4bldg/hasTurbulator
<https://saref.etsi.org/saref4bldg/hasTurbulator> rdf:type owl:DatatypeProperty ;
                                                  rdfs:range xsd:boolean ;
                                                  rdfs:comment "TRUE if the tube has a turbulator, FALSE if it does not."@en ;
                                                  rdfs:label "has turbulator"@en .


###  https://saref.etsi.org/saref4bldg/heatTransferDimension
<https://saref.etsi.org/saref4bldg/heatTransferDimension> rdf:type owl:DatatypeProperty ;
                                                          rdfs:range xsd:string ;
                                                          rdfs:comment "Indicates how heat is transmitted according to the shape of the space heater."@en ;
                                                          rdfs:label "heat transfer dimension"@en .


###  https://saref.etsi.org/saref4bldg/heatTransferMedium
<https://saref.etsi.org/saref4bldg/heatTransferMedium> rdf:type owl:DatatypeProperty ;
                                                       rdfs:range xsd:string ;
                                                       rdfs:comment "Enumeration defining the heat transfer medium if applicable."@en ;
                                                       rdfs:label "heat transfer medium"@en .


###  https://saref.etsi.org/saref4bldg/heatTransferTypeEnum
<https://saref.etsi.org/saref4bldg/heatTransferTypeEnum> rdf:type owl:DatatypeProperty ;
                                                         rdfs:range xsd:string ;
                                                         rdfs:comment "Type of heat transfer between the two air streams."@en ;
                                                         rdfs:label "heat transfer type enum"@en .


###  https://saref.etsi.org/saref4bldg/integratedLightingType
<https://saref.etsi.org/saref4bldg/integratedLightingType> rdf:type owl:DatatypeProperty ;
                                                           rdfs:range xsd:string ;
                                                           rdfs:comment "Integrated lighting in cooled beam."@en ;
                                                           rdfs:label "integrated lighting type"@en .


###  https://saref.etsi.org/saref4bldg/internalControl
<https://saref.etsi.org/saref4bldg/internalControl> rdf:type owl:DatatypeProperty ;
                                                    rdfs:range xsd:string ;
                                                    rdfs:comment "Internal modulation control."@en ;
                                                    rdfs:label "internal control"@en .


###  https://saref.etsi.org/saref4bldg/isExternal
<https://saref.etsi.org/saref4bldg/isExternal> rdf:type owl:DatatypeProperty ;
                                               rdfs:range xsd:boolean ;
                                               rdfs:comment "Indication whether the element is designed for use in the exterior (TRUE) or not (FALSE). If (TRUE) it is an external element and faces the outside of the building."@en ;
                                               rdfs:label "is external"@en .


###  https://saref.etsi.org/saref4bldg/isFreeHanging
<https://saref.etsi.org/saref4bldg/isFreeHanging> rdf:type owl:DatatypeProperty ;
                                                  rdfs:range xsd:boolean ;
                                                  rdfs:comment "Is it free hanging type (not mounted in a false ceiling)?"@en ;
                                                  rdfs:label "is free hanging"@en .


###  https://saref.etsi.org/saref4bldg/isGuarded
<https://saref.etsi.org/saref4bldg/isGuarded> rdf:type owl:DatatypeProperty ;
                                              rdfs:range xsd:boolean ;
                                              rdfs:comment "Indication of whether the motor enclosure is guarded (= TRUE) or not (= FALSE)."@en ;
                                              rdfs:label "is guarded"@en .


###  https://saref.etsi.org/saref4bldg/isIlluminated
<https://saref.etsi.org/saref4bldg/isIlluminated> rdf:type owl:DatatypeProperty ;
                                                  rdfs:range xsd:boolean ;
                                                  rdfs:comment "An indication of whether there is an illuminated indicator to show that the switch is on (=TRUE) or not (= FALSE)."@en ;
                                                  rdfs:label "is illuminated"@en .


###  https://saref.etsi.org/saref4bldg/isNeutralPrimaryTerminalAvailable
<https://saref.etsi.org/saref4bldg/isNeutralPrimaryTerminalAvailable> rdf:type owl:DatatypeProperty ;
                                                                      rdfs:range xsd:boolean ;
                                                                      rdfs:comment "An indication of whether the neutral point of the primary winding is available as a terminal (=TRUE) or not (= FALSE)."@en ;
                                                                      rdfs:label "is neutral primary terminal available"@en .


###  https://saref.etsi.org/saref4bldg/isNeutralSecondaryTerminalAvailable
<https://saref.etsi.org/saref4bldg/isNeutralSecondaryTerminalAvailable> rdf:type owl:DatatypeProperty ;
                                                                        rdfs:range xsd:boolean ;
                                                                        rdfs:comment "An indication of whether the neutral point of the secondary winding is available as a terminal (=TRUE) or not (= FALSE)."@en ;
                                                                        rdfs:label "is neutral secondary terminal available"@en .


###  https://saref.etsi.org/saref4bldg/isPluggableOutlet
<https://saref.etsi.org/saref4bldg/isPluggableOutlet> rdf:type owl:DatatypeProperty ;
                                                      rdfs:range xsd:boolean ;
                                                      rdfs:comment "Indication of whether the outlet accepts a loose plug connection (= TRUE) or whether it is directly connected (= FALSE) or whether the form of connection has not yet been determined (= UNKNOWN)."@en ;
                                                      rdfs:label "is pluggable outlet"@en .


###  https://saref.etsi.org/saref4bldg/isWaterStorageHeater
<https://saref.etsi.org/saref4bldg/isWaterStorageHeater> rdf:type owl:DatatypeProperty ;
                                                         rdfs:range xsd:boolean ;
                                                         rdfs:comment "This is used to identify if the boiler has storage capacity (TRUE). If FALSE, then there is no storage capacity built into the boiler, such as an instantaneous hot water heater."@en ;
                                                         rdfs:label "is water storage heater"@en .


###  https://saref.etsi.org/saref4bldg/lampBallastType
<https://saref.etsi.org/saref4bldg/lampBallastType> rdf:type owl:DatatypeProperty ;
                                                    rdfs:range xsd:string ;
                                                    rdfs:comment "The type of ballast used to stabilise gas discharge by limiting the current during operation and to deliver the necessary striking voltage for starting. Ballasts are needed to operate Discharge Lamps such as Fluorescent, Compact Fluorescent, High-pressure Mercury, Metal Halide and High-pressure Sodium Lamps. Magnetic ballasts are chokes which limit the current passing through a lamp connected in series on the principle of self-induction. The resultant current and power are decisive for the efficient operation of the lamp. A specially designed ballast is required for every type of lamp to comply with lamp rating in terms of Luminous Flux, Color Appearance and service life. The two types of magnetic ballasts for fluorescent lamps are KVG Conventional (EC-A series) and VVG Low-loss ballasts (EC-B series). Low-loss ballasts have a higher efficiency, which means reduced ballast losses and a lower thermal load. Electronic ballasts are used to run fluorescent lamps at high frequencies (approx. 35 - 40 kHz)."@en ;
                                                    rdfs:label "lamp ballast type"@en .


###  https://saref.etsi.org/saref4bldg/lampCompensationType
<https://saref.etsi.org/saref4bldg/lampCompensationType> rdf:type owl:DatatypeProperty ;
                                                         rdfs:range xsd:string ;
                                                         rdfs:comment "Identifies the form of compensation used for power factor correction and radio suppression."@en ;
                                                         rdfs:label "lamp compensation type"@en .


###  https://saref.etsi.org/saref4bldg/legend
<https://saref.etsi.org/saref4bldg/legend> rdf:type owl:DatatypeProperty ;
                                           rdfs:range xsd:string ;
                                           rdfs:comment "A text inscribed or applied to the switch as a legend to indicate purpose or function."@en ;
                                           rdfs:label "legend"@en .


###  https://saref.etsi.org/saref4bldg/manualOverride
<https://saref.etsi.org/saref4bldg/manualOverride> rdf:type owl:DatatypeProperty ;
                                                   rdfs:range xsd:boolean ;
                                                   rdfs:comment "Identifies whether hand-operated operation is provided as an override (= TRUE) or not (= FALSE). Note that this value should be set to FALSE by default in the case of a Hand Operated Actuator."@en ;
                                                   rdfs:label "manual override"@en .


###  https://saref.etsi.org/saref4bldg/mechanicalOperated
<https://saref.etsi.org/saref4bldg/mechanicalOperated> rdf:type owl:DatatypeProperty ;
                                                       rdfs:range xsd:boolean ;
                                                       rdfs:comment "Indication whether the element is operated machanically (TRUE) or not, i.e. manually (FALSE)."@en ;
                                                       rdfs:label "mechanical operated"@en .


###  https://saref.etsi.org/saref4bldg/mediaSource
<https://saref.etsi.org/saref4bldg/mediaSource> rdf:type owl:DatatypeProperty ;
                                                rdfs:range xsd:string ;
                                                rdfs:comment "Indicates media sources and corresponding names of ports (DistributionPort with FlowDirection=SINK and PredefinedType=AUDIOVISUAL) or aggregated audio/video components (AudioVisualAppliance)."@en ;
                                                rdfs:label "media source"@en .


###  https://saref.etsi.org/saref4bldg/motorDriveType
<https://saref.etsi.org/saref4bldg/motorDriveType> rdf:type owl:DatatypeProperty ;
                                                   rdfs:range xsd:string ;
                                                   rdfs:comment "Motor drive type: DIRECTDRIVE: Direct drive. BELTDRIVE: Belt drive. COUPLING: Coupling. OTHER: Other type of motor drive. UNKNOWN: Unknown motor drive type. "@en ;
                                                   rdfs:label "motor drive type"@en .


###  https://saref.etsi.org/saref4bldg/motorEnclosureType
<https://saref.etsi.org/saref4bldg/motorEnclosureType> rdf:type owl:DatatypeProperty ;
                                                       rdfs:range xsd:string ;
                                                       rdfs:comment "A list of the available types of motor enclosure from which that required may be selected."@en ;
                                                       rdfs:label "motor enclosure type"@en .


###  https://saref.etsi.org/saref4bldg/numberOfBlades
<https://saref.etsi.org/saref4bldg/numberOfBlades> rdf:type owl:DatatypeProperty ;
                                                   rdfs:range xsd:integer ;
                                                   rdfs:comment "Number of blades."@en ;
                                                   rdfs:label "number of blades"@en .


###  https://saref.etsi.org/saref4bldg/numberOfCells
<https://saref.etsi.org/saref4bldg/numberOfCells> rdf:type owl:DatatypeProperty ;
                                                  rdfs:range xsd:integer ;
                                                  rdfs:comment "Number of cells in one cooling tower unit."@en ;
                                                  rdfs:label "number of cells"@en .


###  https://saref.etsi.org/saref4bldg/numberOfCircuits
<https://saref.etsi.org/saref4bldg/numberOfCircuits> rdf:type owl:DatatypeProperty ;
                                                     rdfs:range xsd:integer ;
                                                     rdfs:comment "Number of parallel fluid tube circuits."@en ;
                                                     rdfs:label "number of circuits"@en .


###  https://saref.etsi.org/saref4bldg/numberOfGangs
<https://saref.etsi.org/saref4bldg/numberOfGangs> rdf:type owl:DatatypeProperty ;
                                                  rdfs:range xsd:integer ;
                                                  rdfs:comment "Number of gangs/buttons on this switch."@en ;
                                                  rdfs:label "number of gangs"@en .


###  https://saref.etsi.org/saref4bldg/numberOfPanels
<https://saref.etsi.org/saref4bldg/numberOfPanels> rdf:type owl:DatatypeProperty ;
                                                   rdfs:range xsd:integer ;
                                                   rdfs:comment "Number of panels."@en ;
                                                   rdfs:label "number of panels"@en .


###  https://saref.etsi.org/saref4bldg/numberOfRows
<https://saref.etsi.org/saref4bldg/numberOfRows> rdf:type owl:DatatypeProperty ;
                                                 rdfs:range xsd:integer ;
                                                 rdfs:comment "Number of tube rows in the tube bundle assembly."@en ;
                                                 rdfs:label "number of rows"@en .


###  https://saref.etsi.org/saref4bldg/numberOfSections
<https://saref.etsi.org/saref4bldg/numberOfSections> rdf:type owl:DatatypeProperty ;
                                                     rdfs:range xsd:integer ;
                                                     rdfs:comment "Number of sections used."@en ;
                                                     rdfs:label "number of sections"@en .


###  https://saref.etsi.org/saref4bldg/numberOsSockets
<https://saref.etsi.org/saref4bldg/numberOsSockets> rdf:type owl:DatatypeProperty ;
                                                    rdfs:range xsd:integer ;
                                                    rdfs:comment "The number of sockets that may be connected. In case of inconsistency, sockets defined on ports take precedence."@en ;
                                                    rdfs:label "number os sockets"@en .


###  https://saref.etsi.org/saref4bldg/operatingMode
<https://saref.etsi.org/saref4bldg/operatingMode> rdf:type owl:DatatypeProperty ;
                                                  rdfs:range xsd:string ;
                                                  rdfs:comment "Identifies the operating mode of the boiler."@en ;
                                                  rdfs:label "operating mode"@en .


###  https://saref.etsi.org/saref4bldg/operation
<https://saref.etsi.org/saref4bldg/operation> rdf:type owl:DatatypeProperty ;
                                              rdfs:range xsd:string ;
                                              rdfs:comment "The operational mechanism for the damper operation."@en ;
                                              rdfs:label "operation"@en .


###  https://saref.etsi.org/saref4bldg/orientation
<https://saref.etsi.org/saref4bldg/orientation> rdf:type owl:DatatypeProperty ;
                                                rdfs:range xsd:string ;
                                                rdfs:comment "The intended orientation for the damper as specified by the manufacturer."@en ;
                                                rdfs:label "orientation"@en .


###  https://saref.etsi.org/saref4bldg/patternType
<https://saref.etsi.org/saref4bldg/patternType> rdf:type owl:DatatypeProperty ;
                                                rdfs:range xsd:string ;
                                                rdfs:comment "Defines the types of pattern (or shape of a tank that may be specified."@en ;
                                                rdfs:label "pattern type"@en .


###  https://saref.etsi.org/saref4bldg/pipeConnectionEnum
<https://saref.etsi.org/saref4bldg/pipeConnectionEnum> rdf:type owl:DatatypeProperty ;
                                                       rdfs:range xsd:string ;
                                                       rdfs:comment "The manner in which the pipe connection is made to the cooled beam."@en ;
                                                       rdfs:label "pipe connection enum"@en .


###  https://saref.etsi.org/saref4bldg/placementType
<https://saref.etsi.org/saref4bldg/placementType> rdf:type owl:DatatypeProperty ;
                                                  rdfs:range xsd:string ;
                                                  rdfs:comment "Indicates how the device is designed to be placed."@en ;
                                                  rdfs:label "placement type"@en .


###  https://saref.etsi.org/saref4bldg/powerSource
<https://saref.etsi.org/saref4bldg/powerSource> rdf:type owl:DatatypeProperty ;
                                                rdfs:range xsd:string ;
                                                rdfs:comment "Type of power driving the compressor."@en ;
                                                rdfs:label "power source"@en .


###  https://saref.etsi.org/saref4bldg/readOutType
<https://saref.etsi.org/saref4bldg/readOutType> rdf:type owl:DatatypeProperty ;
                                                rdfs:range xsd:string ;
                                                rdfs:comment "Indication of the form that readout from the meter takes. In the case of a dial read out, this may comprise multiple dials that give a cumulative reading and/or a mechanical odometer."@en ;
                                                rdfs:label "read out type"@en .


###  https://saref.etsi.org/saref4bldg/refrigerantClass
<https://saref.etsi.org/saref4bldg/refrigerantClass> rdf:type owl:DatatypeProperty ;
                                                     rdfs:range xsd:string ;
                                                     rdfs:comment "Refrigerant class used by the compressor. CFC: Chlorofluorocarbons. HCFC: Hydrochlorofluorocarbons. HFC: Hydrofluorocarbons."@en ;
                                                     rdfs:label "refrigerant class"@en .


###  https://saref.etsi.org/saref4bldg/remoteReading
<https://saref.etsi.org/saref4bldg/remoteReading> rdf:type owl:DatatypeProperty ;
                                                  rdfs:range xsd:boolean ;
                                                  rdfs:comment "Indicates whether the meter has a connection for remote reading through connection of a communication device (set TRUE) or not (set FALSE)."@en ;
                                                  rdfs:label "remote reading"@en .


###  https://saref.etsi.org/saref4bldg/roughness
<https://saref.etsi.org/saref4bldg/roughness> rdf:type owl:DatatypeProperty ;
                                              rdfs:range xsd:string ;
                                              rdfs:comment "A measure of the vertical deviations of the surface."@en ;
                                              rdfs:label "roughness"@en .


###  https://saref.etsi.org/saref4bldg/secondaryCurrentType
<https://saref.etsi.org/saref4bldg/secondaryCurrentType> rdf:type owl:DatatypeProperty ;
                                                         rdfs:range xsd:string ;
                                                         rdfs:comment "A list of the secondary current types that can result from transformer output."@en ;
                                                         rdfs:label "secondary current type"@en .


###  https://saref.etsi.org/saref4bldg/shadingDeviceType
<https://saref.etsi.org/saref4bldg/shadingDeviceType> rdf:type owl:DatatypeProperty ;
                                                      rdfs:range xsd:string ;
                                                      rdfs:comment "Specifies the type of shading device."@en ;
                                                      rdfs:label "shading device type"@en .


###  https://saref.etsi.org/saref4bldg/sprayType
<https://saref.etsi.org/saref4bldg/sprayType> rdf:type owl:DatatypeProperty ;
                                              rdfs:range xsd:string ;
                                              rdfs:comment "SprayFilled: Water is sprayed into airflow. SplashTypeFill: water cascades over successive rows of splash bars. FilmTypeFill: water flows in a thin layer over closely spaced sheets."@en ;
                                              rdfs:label "spray type"@en .


###  https://saref.etsi.org/saref4bldg/standard
<https://saref.etsi.org/saref4bldg/standard> rdf:type owl:DatatypeProperty ;
                                             rdfs:range xsd:string ;
                                             rdfs:comment "The designation of the standard applicable for the definition of the characteristics of the unit."@en ;
                                             rdfs:label "standard"@en .


###  https://saref.etsi.org/saref4bldg/storageType
<https://saref.etsi.org/saref4bldg/storageType> rdf:type owl:DatatypeProperty ;
                                                rdfs:range xsd:string ;
                                                rdfs:comment "Defines the general material category intended to be stored."@en ;
                                                rdfs:label "storage type"@en .


###  https://saref.etsi.org/saref4bldg/switchFunction
<https://saref.etsi.org/saref4bldg/switchFunction> rdf:type owl:DatatypeProperty ;
                                                   rdfs:range xsd:string ;
                                                   rdfs:comment "Indicates types of switches which differs in functionality."@en ;
                                                   rdfs:label "switch function"@en .


###  https://saref.etsi.org/saref4bldg/temperatureClassification
<https://saref.etsi.org/saref4bldg/temperatureClassification> rdf:type owl:DatatypeProperty ;
                                                              rdfs:range xsd:string ;
                                                              rdfs:comment "Enumeration defining the temperature classification of the space heater surface temperature. low temperature - surface temperature is relatively low, usually heated by hot water or electricity. high temperature - surface temperature is relatively high, usually heated by gas or steam."@en ;
                                                              rdfs:label "temperature classification"@en .


###  https://saref.etsi.org/saref4bldg/transformerVectorGroup
<https://saref.etsi.org/saref4bldg/transformerVectorGroup> rdf:type owl:DatatypeProperty ;
                                                           rdfs:range xsd:string ;
                                                           rdfs:comment "List of the possible vector groups for the transformer from which that required may be set. Values in the enumeration list follow a standard international code where the first letter describes how the primary windings are connected, the second letter describes how the secondary windings are connected, and the numbers describe the rotation of voltages and currents from the primary to the secondary side in multiples of 30 degrees. D: means that the windings are delta-connected. Y: means that the windings are star-connected. Z: means that the windings are zig-zag connected (a special start-connected providing low reactance of the transformer). The connectivity is only relevant for three-phase transformers."@en ;
                                                           rdfs:label "transformer vector group"@en .


###  https://saref.etsi.org/saref4bldg/valveMechanism
<https://saref.etsi.org/saref4bldg/valveMechanism> rdf:type owl:DatatypeProperty ;
                                                   rdfs:range xsd:string ;
                                                   rdfs:comment "The mechanism by which the valve function is achieved where: BALL: Valve that has a ported ball that can be turned relative to the body seat ports. BUTTERFLY: Valve in which a streamlined disc pivots about a diametric axis. CONFIGUREDGATE: Screwdown valve in which the closing gate is shaped in a configured manner to have a more precise control of pressure and flow change across the valve. GLAND: Valve with a tapered seating, in which a rotatable plug is retained by means of a gland and gland packing. GLOBE: Screwdown valve that has a spherical body. LUBRICATEDPLUG: Plug valve in which a lubricant is injected under pressure between the plug face and the body. NEEDLE: Valve for regulating the flow in or from a pipe, in which a slender cone moves along the axis of flow to close against a fixed conical seat. PARALLELSLIDE: Screwdown valve that has a machined plate that slides in formed grooves to form a seal. PLUG: Valve that has a ported plug that can be turned relative to the body seat ports. WEDGEGATE: Screwdown valve that has a wedge shaped plate fitting into tapered guides to form a seal."@en ;
                                                   rdfs:label "valve mechanism"@en .


###  https://saref.etsi.org/saref4bldg/valveOperation
<https://saref.etsi.org/saref4bldg/valveOperation> rdf:type owl:DatatypeProperty ;
                                                   rdfs:range xsd:string ;
                                                   rdfs:comment "The method of valve operation where: DROPWEIGHT: A valve that is closed by the action of a weighted lever being released, the weight normally being prevented from dropping by being held by a wire, the closure normally being made by the action of heat on a fusible link in the wire FLOAT: A valve that is opened and closed by the action of a float that rises and falls with water level. The float may be a ball attached to a lever or other mechanism HYDRAULIC: A valve that is opened and closed by hydraulic actuation LEVER: A valve that is opened and closed by the action of a lever rotating the gate within the valve. LOCKSHIELD: A valve that requires the use of a special lockshield key for opening and closing, the operating mechanism being protected by a shroud during normal operation. MOTORIZED: A valve that is opened and closed by the action of an electric motor on an actuator PNEUMATIC: A valve that is opened and closed by pneumatic actuation SOLENOID: A valve that is normally held open by a magnetic field in a coil acting on the gate but that is closed immediately if the electrical current generating the magnetic field is removed. SPRING: A valve that is normally held in position by the pressure of a spring on a plate but that may be caused to open if the pressure of the fluid is sufficient to overcome the spring pressure. THERMOSTATIC: A valve in which the ports are opened or closed to maintain a required predetermined temperature. WHEEL: A valve that is opened and closed by the action of a wheel moving the gate within the valve."@en ;
                                                   rdfs:label "valve operation"@en .


###  https://saref.etsi.org/saref4bldg/valvePattern
<https://saref.etsi.org/saref4bldg/valvePattern> rdf:type owl:DatatypeProperty ;
                                                 rdfs:range xsd:string ;
                                                 rdfs:comment "The configuration of the ports of a valve according to either the linear route taken by a fluid flowing through the valve or by the number of ports where: SINGLEPORT: Valve that has a single entry port from the system that it serves, the exit port being to the surrounding environment. ANGLED_2_PORT: Valve in which the direction of flow is changed through 90 degrees. STRAIGHT_2_PORT: Valve in which the flow is straight through. STRAIGHT_3_PORT: Valve with three separate ports. CROSSOVER_4_PORT: Valve with 4 separate ports."@en ;
                                                 rdfs:label "valve pattern"@en .


###  https://saref.etsi.org/saref4bldg/waterFlowControlSystemType
<https://saref.etsi.org/saref4bldg/waterFlowControlSystemType> rdf:type owl:DatatypeProperty ;
                                                               rdfs:range xsd:string ;
                                                               rdfs:comment "Factory fitted waterflow control system."@en ;
                                                               rdfs:label "water flow control system type"@en .


#################################################################
#    Classes
#################################################################

###  http://www.opengis.net/ont/geosparql#SpatialThing
<http://www.opengis.net/ont/geosparql#SpatialThing> rdf:type owl:Class .


###  http://www.w3.org/2006/time#TemporalEntity
<http://www.w3.org/2006/time#TemporalEntity> rdf:type owl:Class .


###  http://www.w3.org/2006/time#TemporalPosition
<http://www.w3.org/2006/time#TemporalPosition> rdf:type owl:Class .


###  https://saref.etsi.org/core/Actuation
<https://saref.etsi.org/core/Actuation> rdf:type owl:Class ;
                                        rdfs:subClassOf <https://saref.etsi.org/core/ProcedureExecution> ,
                                                        [ rdf:type owl:Restriction ;
                                                          owl:onProperty <https://saref.etsi.org/core/madeBy> ;
                                                          owl:allValuesFrom <https://saref.etsi.org/core/Actuator>
                                                        ] ,
                                                        [ rdf:type owl:Restriction ;
                                                          owl:onProperty <https://saref.etsi.org/core/controls> ;
                                                          owl:minCardinality "1"^^xsd:nonNegativeInteger
                                                        ] ;
                                        rdfs:comment "A saref:Actuation is the act of carrying out a procedure to control the state of the world using an actuator. It links to an actuator to describe what made the actuation, and to the controlled feature, property, property of interest, state, or state of interest. Typically, its input is a property value or a state. An actuation of a state (OP saref:controls) should have a state as input (OP saref:hasInput). Respectively, an actuation of a property should have a property value as input."@en ;
                                        rdfs:label "Actuation"@en .


###  https://saref.etsi.org/core/Actuator
<https://saref.etsi.org/core/Actuator> rdf:type owl:Class ;
                                       rdfs:subClassOf <https://saref.etsi.org/core/Device> ,
                                                       [ rdf:type owl:Restriction ;
                                                         owl:onProperty <https://saref.etsi.org/core/controls> ;
                                                         owl:minCardinality "1"^^xsd:nonNegativeInteger
                                                       ] ;
                                       rdfs:comment "A device designed to control one or more properties or states of one or more features of interest."@en ;
                                       rdfs:label "Actuator"@en ;
                                       <http://www.w3.org/2004/02/skos/core#historyNote> "V3.2.1: Definition of Actuator is simplified and grounded on saref:controls. Local restriction on saref:hasFunction is deleted."@en .


###  https://saref.etsi.org/core/Appliance
<https://saref.etsi.org/core/Appliance> rdf:type owl:Class ;
                                        rdfs:subClassOf <https://saref.etsi.org/core/Device> ;
                                        rdfs:comment "A device designed to accomplish a particular task for occupant use. It consumes, produces, or stores, some commodity."@en ;
                                        rdfs:label "Appliance"@en ;
                                        <http://www.w3.org/2004/02/skos/core#historyNote> "V3.2.1: Definition of saref:Appliance is grounded on tasks and commodities."@en .


###  https://saref.etsi.org/core/Command
<https://saref.etsi.org/core/Command> rdf:type owl:Class ;
                                      rdfs:subClassOf [ rdf:type owl:Restriction ;
                                                        owl:onProperty <http://www.w3.org/2004/02/skos/core#broader> ;
                                                        owl:allValuesFrom <https://saref.etsi.org/core/Command>
                                                      ] ,
                                                      [ rdf:type owl:Restriction ;
                                                        owl:onProperty <http://www.w3.org/2004/02/skos/core#narrower> ;
                                                        owl:allValuesFrom <https://saref.etsi.org/core/Command>
                                                      ] ;
                                      rdfs:comment "The lowest-level directives a function exposes to some network. Commands can target (OP saref:targets and its sub-properties) features, properties, or states. An instance of saref:Command is independent of any device."@en ;
                                      rdfs:label "Command"@en ;
                                      <http://www.w3.org/2004/02/skos/core#example> "Observe property, control property, observe state, control state, invoke action, cancel action, turn on or off, change color, subscribe, publish, etc. are all commands."@en ;
                                      <http://www.w3.org/2004/02/skos/core#historyNote> "V3.2.1: Simplified definition and axiomatization of saref:Command. Added examples."@en .


###  https://saref.etsi.org/core/CommandExecution
<https://saref.etsi.org/core/CommandExecution> rdf:type owl:Class ;
                                               rdfs:subClassOf <https://saref.etsi.org/core/ProcedureExecution> ,
                                                               [ rdf:type owl:Restriction ;
                                                                 owl:onProperty <https://saref.etsi.org/core/isExecutionOf> ;
                                                                 owl:allValuesFrom [ rdf:type owl:Class ;
                                                                                     owl:unionOf ( <https://saref.etsi.org/core/Command>
                                                                                                   <https://saref.etsi.org/core/CommandOfInterest>
                                                                                                 )
                                                                                   ]
                                                               ] ;
                                               rdfs:comment "Describes the execution of a command. Typically, its inputs and outputs are human understandable and relate to some feature of interest, such as its state (e.g., s4abcd:On), or the value of its temperature (e.g., property value 21.0 C)."@en ;
                                               rdfs:label "Command Execution"@en .


###  https://saref.etsi.org/core/CommandOfInterest
<https://saref.etsi.org/core/CommandOfInterest> rdf:type owl:Class ;
                                                rdfs:subClassOf [ rdf:type owl:Restriction ;
                                                                  owl:onProperty <https://saref.etsi.org/core/isCommandOfInterestOf> ;
                                                                  owl:cardinality "1"^^xsd:nonNegativeInteger
                                                                ] ;
                                                rdfs:comment "The lowest-level directives a device supports and exposes to some network. Commands can target (OP saref:targets and its sub-properties) features, properties, or states. A saref:CommandOfInterest is a directives actually supported by a device and exposed to some network."@en ;
                                                rdfs:label "Command Of Interest"@en ;
                                                <http://www.w3.org/2004/02/skos/core#example> "The corridor smart light switch supports a command of kind turn on/off, which controls the state of the outdoor light."@en ,
                                                                                              "The smart fridge supports a command of kind observe temperature, which observes the temperature of the fridge."@en ;
                                                <http://www.w3.org/2004/02/skos/core#historyNote> "V3.2.1: Introduced saref:CommandOfInterest, parallel to saref:PropertyOfInterest."@en ;
                                                <http://www.w3.org/2004/02/skos/core#note> "Commands of interest need not always be explicited. It depends on the use case. Typically, commands of interest are useful to specify the actual property of interest or state of interest that is expected as input parameter, output, or that will be targeted."@en ,
                                                                                           "Like for commands, commands of interest may be described in terms of their input parameters, outputs, and which properties or states they target."@en .


###  https://saref.etsi.org/core/Commodity
<https://saref.etsi.org/core/Commodity> rdf:type owl:Class ;
                                        rdfs:subClassOf [ rdf:type owl:Restriction ;
                                                          owl:onProperty <http://www.w3.org/2004/02/skos/core#broader> ;
                                                          owl:allValuesFrom <https://saref.etsi.org/core/Commodity>
                                                        ] ,
                                                        [ rdf:type owl:Restriction ;
                                                          owl:onProperty <http://www.w3.org/2004/02/skos/core#narrower> ;
                                                          owl:allValuesFrom <https://saref.etsi.org/core/Commodity>
                                                        ] ;
                                        rdfs:comment "A marketable item which may be supplied without qualitative differentiation."@en ;
                                        rdfs:label "Commodity"@en ;
                                        <http://www.w3.org/2004/02/skos/core#historyNote> "V3.2.1: Definition of saref:Commodity is simplified."@en ,
                                                                                          "V4.1.1: Removed examples of commodity categories."@en ;
                                        <http://www.w3.org/2004/02/skos/core#note> "Concepts from existing code lists, vocabularies, and taxonomies, may be used as instances of saref:Commodity, for example from the ISDA taxonomy of commodities, the Standard International Energy product Classification (SIEC), the IRENA Energy Taxonomy or Wikidata."@en ,
                                                                                   "SAREF refers to energy commodities such as electricity, gas, coal and oil."@en .


###  https://saref.etsi.org/core/Device
<https://saref.etsi.org/core/Device> rdf:type owl:Class ;
                                     rdfs:subClassOf <https://saref.etsi.org/core/FeatureOfInterest> ,
                                                     <https://saref.etsi.org/saref4syst/System> ;
                                     rdfs:comment "A tangible object designed to accomplish a particular task. In order to accomplish this task, the device performs one or more functions. An instance of saref:Device represents one specific real world entity."@en ;
                                     rdfs:label "Device"@en ;
                                     <http://www.w3.org/2004/02/skos/core#example> "Examples of devices are a light switch, a temperature sensor, an energy meter, a water flow meter, and a laundry dryer. A laundry dryer is designed to dry laundry, and to accomplish this task it has a start/stop function."@en ,
                                                                                   "For example, a washing machine is designed to wash (task) and to accomplish this task it performs a start and stop function."@en ;
                                     <http://www.w3.org/2004/02/skos/core#historyNote> "V3.2.1: Most axioms on saref:Device were useless and have been deleted."@en ,
                                                                                       "V3.2.1: definition of saref:Device clarifies it's a real world entity."@en ,
                                                                                       "V3.2.1: saref:Device is explicitly a subclass of saref:FeatureOfInterest and s4syst:System."@en .


###  https://saref.etsi.org/core/DeviceKind
<https://saref.etsi.org/core/DeviceKind> rdf:type owl:Class ;
                                         rdfs:subClassOf <https://saref.etsi.org/core/FeatureKind> ,
                                                         [ rdf:type owl:Restriction ;
                                                           owl:onProperty <http://www.w3.org/2004/02/skos/core#broader> ;
                                                           owl:allValuesFrom <https://saref.etsi.org/core/FeatureKind>
                                                         ] ,
                                                         [ rdf:type owl:Restriction ;
                                                           owl:onProperty <http://www.w3.org/2004/02/skos/core#narrower> ;
                                                           owl:allValuesFrom <https://saref.etsi.org/core/FeatureKind>
                                                         ] ;
                                         rdfs:comment "Device kinds allow to describe kinds of devices, with common properties and common states having the same value, targeting the same properties and states, common functions, and common services. Devices kinds may be used to describe models of devices in online catalogues."@en ;
                                         rdfs:label "Device kinds"@en ;
                                         <http://www.w3.org/2004/02/skos/core#historyNote> "V4.1.1: Introduced class saref:DeviceKind"@en ,
                                                                                           "V4.1.1: Use SKOS to organize generic classes in taxonomies."@en .


###  https://saref.etsi.org/core/FeatureKind
<https://saref.etsi.org/core/FeatureKind> rdf:type owl:Class ;
                                          rdfs:subClassOf [ rdf:type owl:Restriction ;
                                                            owl:onProperty <http://www.w3.org/2004/02/skos/core#broader> ;
                                                            owl:allValuesFrom <https://saref.etsi.org/core/FeatureKind>
                                                          ] ,
                                                          [ rdf:type owl:Restriction ;
                                                            owl:onProperty <http://www.w3.org/2004/02/skos/core#narrower> ;
                                                            owl:allValuesFrom <https://saref.etsi.org/core/FeatureKind>
                                                          ] ,
                                                          [ rdf:type owl:Restriction ;
                                                            owl:onProperty <https://saref.etsi.org/core/consistsOf> ;
                                                            owl:allValuesFrom <https://saref.etsi.org/core/FeatureKind>
                                                          ] ;
                                          rdfs:comment "Feature kinds allow to describe kinds of features of interest, with common properties having the same value, and common states being the same. An instance of saref:FeatureKind represents an archetype of real world entities, for example to populate product catalogs."@en ;
                                          rdfs:label "Feature kinds"@en ;
                                          <http://www.w3.org/2004/02/skos/core#historyNote> "V3.2.1: Introduced class saref:FeatureKind"@en ,
                                                                                            "V3.2.1: Use SKOS to organize generic classes in taxonomies."@en .


###  https://saref.etsi.org/core/FeatureOfInterest
<https://saref.etsi.org/core/FeatureOfInterest> rdf:type owl:Class ;
                                                rdfs:subClassOf [ rdf:type owl:Restriction ;
                                                                  owl:onProperty <https://saref.etsi.org/core/consistsOf> ;
                                                                  owl:allValuesFrom <https://saref.etsi.org/core/FeatureOfInterest>
                                                                ] ;
                                                rdfs:comment "A feature of interest represents any real world entity from which a property or a state may be targeted, such as observed and controlled. An instance of saref:FeatureOfInterest represents one specific real world entity."@en ;
                                                rdfs:label "Feature of interest"@en ;
                                                <http://www.w3.org/2004/02/skos/core#historyNote> "V3.2.1: Definition of saref:FeatureOfInterest is clarified, not only properties are measured, but properties and states can be observed and controlled."@en ,
                                                                                                  "V3.2.1: Definition of saref:FeatureOfInterest: Clarify it's a specific real world entity."@en ,
                                                                                                  "V3.2.1: Definition of saref:FeatureOfInterest: allValuesFrom axioms are unnecessary and have been deleted."@en .


###  https://saref.etsi.org/core/Function
<https://saref.etsi.org/core/Function> rdf:type owl:Class ;
                                       rdfs:subClassOf [ rdf:type owl:Restriction ;
                                                         owl:onProperty <http://www.w3.org/2004/02/skos/core#broader> ;
                                                         owl:allValuesFrom <https://saref.etsi.org/core/Function>
                                                       ] ,
                                                       [ rdf:type owl:Restriction ;
                                                         owl:onProperty <http://www.w3.org/2004/02/skos/core#narrower> ;
                                                         owl:allValuesFrom <https://saref.etsi.org/core/Function>
                                                       ] ;
                                       rdfs:comment "Logical groups of commands that devices support to accomplish their tasks. Function can target (OP saref:targets and its sub-properties) features, properties, or states. An instance of saref:Function can apply to different devices."@en ;
                                       rdfs:label "Function"@en ;
                                       <http://www.w3.org/2004/02/skos/core#example> "To accomplish the task of controlling the light, a smart light switch may have a function for turning on and off the light, and another to set the luminosity of the light."@en ,
                                                                                     "To accomplish the task of sensing the temperature, a temperature sensor should have a sensing function."@en ,
                                                                                     "To accomplish the task of washing clothes, a washing machine should have a function for washing."@en ;
                                       <http://www.w3.org/2004/02/skos/core#historyNote> "V3.2.1: Simplified definition and axiomatization of saref:Function. Added examples."@en .


###  https://saref.etsi.org/core/FunctionOfInterest
<https://saref.etsi.org/core/FunctionOfInterest> rdf:type owl:Class ;
                                                 rdfs:subClassOf [ rdf:type owl:Restriction ;
                                                                   owl:onProperty <https://saref.etsi.org/core/isFunctionOfInterestOf> ;
                                                                   owl:cardinality "1"^^xsd:nonNegativeInteger
                                                                 ] ;
                                                 rdfs:comment "Logical groups of commands that devices support to accomplish their tasks. Function can target (OP saref:targets and its sub-properties) features, properties, or states. An instance of saref:FunctionOfInterest is supported by exactly one device."@en ;
                                                 rdfs:label "Function of Interest"@en ;
                                                 <http://www.w3.org/2004/02/skos/core#historyNote> "V3.2.1: Introduced saref:FunctionOfInterest, parallel to saref:PropertyOfInterest."@en ;
                                                 <http://www.w3.org/2004/02/skos/core#note> "A function of interest is the function of (OP saref:isFunctionOfInterestOf) exactly one device."@en ,
                                                                                            "Functions of interest need not always be explicited. It depends on the use case. Typically, functions of interest are useful to specify which command is actually exposed, and which actual property of interest or state of interest it targets."@en .


###  https://saref.etsi.org/core/Meter
<https://saref.etsi.org/core/Meter> rdf:type owl:Class ;
                                    rdfs:subClassOf <https://saref.etsi.org/core/Device> ,
                                                    [ rdf:type owl:Restriction ;
                                                      owl:onProperty <https://saref.etsi.org/core/observes> ;
                                                      owl:minCardinality "1"^^xsd:nonNegativeInteger
                                                    ] ;
                                    rdfs:comment "A device designed to observe and additionally do some computation and/or display one or more properties of one or more features of interest."@en ;
                                    rdfs:label "Meter"@en ;
                                    <http://www.w3.org/2004/02/skos/core#historyNote> "V3.2.1: Definition of Meter is simplified and grounded on saref:observes. Local restriction on saref:hasFunction is deleted."@en ,
                                                                                      "V4.1.1: Definition of Sensor and Meter are updated to better distinguish one from the other."@en .


###  https://saref.etsi.org/core/Observation
<https://saref.etsi.org/core/Observation> rdf:type owl:Class ;
                                          rdfs:subClassOf <https://saref.etsi.org/core/ProcedureExecution> ,
                                                          [ rdf:type owl:Restriction ;
                                                            owl:onProperty <https://saref.etsi.org/core/madeBy> ;
                                                            owl:allValuesFrom <https://saref.etsi.org/core/Sensor>
                                                          ] ,
                                                          [ rdf:type owl:Restriction ;
                                                            owl:onProperty <https://saref.etsi.org/core/observes> ;
                                                            owl:minCardinality "1"^^xsd:nonNegativeInteger
                                                          ] ;
                                          rdfs:comment "A saref:Observation is the act of carrying out a procedure to estimate or calculate a value of a property of a feature of interest, or a state of a feature of interest. It links to a sensor to describe what made the observation, and to the observed feature, property, property of interest, state, or state of interest. Typically, its result is a property value or a state. An observation of a state (OP saref:observes) should have a state as a result (OP saref:hasResult). Respectively, an observation of a property should have a property value as a result."@en ;
                                          rdfs:label "Observation"@en .


###  https://saref.etsi.org/core/Operation
<https://saref.etsi.org/core/Operation> rdf:type owl:Class ;
                                        rdfs:subClassOf [ rdf:type owl:Restriction ;
                                                          owl:onProperty <https://saref.etsi.org/core/represents> ;
                                                          owl:allValuesFrom [ rdf:type owl:Class ;
                                                                              owl:unionOf ( <https://saref.etsi.org/core/Command>
                                                                                            <https://saref.etsi.org/core/CommandOfInterest>
                                                                                          )
                                                                            ]
                                                        ] ,
                                                        [ rdf:type owl:Restriction ;
                                                          owl:onProperty <https://saref.etsi.org/core/represents> ;
                                                          owl:minQualifiedCardinality "1"^^xsd:nonNegativeInteger ;
                                                          owl:onClass <https://saref.etsi.org/core/CommandOfInterest>
                                                        ] ,
                                                        [ rdf:type owl:Restriction ;
                                                          owl:onProperty <https://saref.etsi.org/core/isOperationOf> ;
                                                          owl:cardinality "1"^^xsd:nonNegativeInteger
                                                        ] ;
                                        rdfs:comment "A saref:Operation is the means of a service to communicate in a procedure-type manner over the network (i.e. transmit data to/from other devices). It is the machine interpretable exposure of a human understandable command to a network."@en ;
                                        rdfs:label "Operation"@en ;
                                        <http://www.w3.org/2004/02/skos/core#example> "In the set of operations exposed by a smart light bulb on a given network, one may be dedicated to turn on and off the light and expect a boolean as input. Another one may be dedicated to set the luminosity status and expect a target luminosity level (a byte) and a transition time (encoded on two bytes)."@en ,
                                                                                      "In the set of operations exposed by a smart washing machine on a given network, one may be dedicated to set the water temperature for the washing cycle, and expected as input a enumerated value. Another one may be dedicated to start, pause, or stop the washing cycle."@en ,
                                                                                      "To turn on a light, send a CoAP PUT request with CBOR content 0xf5 (true)"@en ;
                                        <http://www.w3.org/2004/02/skos/core#historyNote> "V3.2.1: Introduced saref:Operation and associated properties from oneM2M base ontology."@en ;
                                        <http://www.w3.org/2004/02/skos/core#note> "An operation may be described in terms of its inputs and outputs using OP saref:hasInput and saref:hasOutput. Inputs and outputs of operations typically describe the expected schema or shape of network messages."@en ,
                                                                                   "Typically, a device connected to a given network offers one service for each of its functions of interest, and each service has one operation per command of interest of the function of interest it represents."@en .


###  https://saref.etsi.org/core/OperationExecution
<https://saref.etsi.org/core/OperationExecution> rdf:type owl:Class ;
                                                 rdfs:subClassOf <https://saref.etsi.org/core/ProcedureExecution> ,
                                                                 [ rdf:type owl:Restriction ;
                                                                   owl:onProperty <https://saref.etsi.org/core/isExecutionOf> ;
                                                                   owl:allValuesFrom <https://saref.etsi.org/core/Operation>
                                                                 ] ;
                                                 rdfs:comment "Describes the execution of an operation in a network: themachine interpretable  description of a communication between devices over the network. Typically, its input and result are network messages, that conform to the input and output of the executed operation."@en ;
                                                 rdfs:label "Operation Execution"@en .


###  https://saref.etsi.org/core/ProcedureExecution
<https://saref.etsi.org/core/ProcedureExecution> rdf:type owl:Class ;
                                                 rdfs:comment "Represents the act of carrying out a procedure."@en ;
                                                 rdfs:label "Procedure Execution"@en ;
                                                 <http://www.w3.org/2004/02/skos/core#historyNote> "V3.2.1: Introduced saref:ProcedureExecution."@en .


###  https://saref.etsi.org/core/Profile
<https://saref.etsi.org/core/Profile> rdf:type owl:Class ;
                                      rdfs:comment "A saref:Profile describes the money earned (negative values) or paied (positive values) for the use (production or consumption) of a commodity by a device in a certain context."@en ;
                                      rdfs:label "Profile"@en ;
                                      <http://www.w3.org/2004/02/skos/core#historyNote> "V3.2.1: Class saref:Profile has been re-specified, to take into account findings from SAREF4ENER V1.2.1."@en ;
                                      <http://www.w3.org/2004/02/skos/core#note> "OP saref:hasPrice links a profile to the money earned (negative values) or paid (positive values) for the use (production or consumption) of the commodity by the device."@en ,
                                                                                 "OP saref:hasProfile links a device to its profile. The device should be linked to a certain commodity using OP saref:consumes, saref:produces, or saref:stores, and optionally to some property or state using OP saref:targets or its sub-properties."@en ,
                                                                                 "The applicable context can be restricted to when a feature of interest has a certain state (OPs saref:whenState)."@en ,
                                                                                 "The applicable context can be restricted to when the property of a feature of interest has some value (OPs saref:whenPropertyValue)"@en ,
                                                                                 "The applicable context of a profile can be bound temporally using DP saref:hasTimestamp or its subproperties defined by SAREF extensions, or OP saref:hasApplicableTime which links to instant or interval or other compound temporal entity expressed using OWL Time."@en .


###  https://saref.etsi.org/core/Property
<https://saref.etsi.org/core/Property> rdf:type owl:Class ;
                                       rdfs:subClassOf [ rdf:type owl:Restriction ;
                                                         owl:onProperty <http://www.w3.org/2004/02/skos/core#broader> ;
                                                         owl:allValuesFrom <https://saref.etsi.org/core/Property>
                                                       ] ,
                                                       [ rdf:type owl:Restriction ;
                                                         owl:onProperty <http://www.w3.org/2004/02/skos/core#narrower> ;
                                                         owl:allValuesFrom <https://saref.etsi.org/core/Property>
                                                       ] ,
                                                       [ rdf:type owl:Restriction ;
                                                         owl:onProperty <https://saref.etsi.org/core/consistsOf> ;
                                                         owl:allValuesFrom [ rdf:type owl:Class ;
                                                                             owl:unionOf ( <https://saref.etsi.org/core/FeatureKind>
                                                                                           <https://saref.etsi.org/core/Property>
                                                                                           <https://saref.etsi.org/core/State>
                                                                                         )
                                                                           ]
                                                       ] ;
                                       rdfs:comment "Identifiable qualities of features of interest that can be target of devices, such as observed or controlled. A property can apply to different features of interest."@en ;
                                       rdfs:label "Property"@en ;
                                       <http://www.w3.org/2004/02/skos/core#example> "Air temperature, pressure, luminance, etc. are all properties."@en ,
                                                                                     """Two examples using the QUDT Quantity Kind vocabulary, and the British Oceanographic Data Centre Parameter Usage Vocabulary.

<https://qudt.org/2.1/vocab/quantitykind/ActiveEnergy> a saref:Property ;
    rdfs:label \"Active Energy\"@en ;
    rdfs:comment \"\"Active Energy\" is the electrical energy transformable into some other form of energy.\"@en .

<http://vocab.nerc.ac.uk/collection/P01/current/CDTSZZ01/> a saref:Property ;
    skos:prefLabel \"Absolute temperature standard deviation of the atmosphere by dry bulb thermometer\"@en .
"""@en ;
                                       <http://www.w3.org/2004/02/skos/core#historyNote> "Until SAREF V3.1.1, there was an ambiguity between whether properties should be specific or generic to features of interest. This ambiguity has been solved in SAREF V3.2.1, and the new modeling will be enforced in the next major revision of SAREF."@en ,
                                                                                         "V3.2.1: The definition and scope of usage for saref:Property is clarified. Axiomatization is simplified."@en ;
                                       <http://www.w3.org/2004/02/skos/core#note> "Concepts from existing code lists, vocabularies, and taxonomies, may be used as instances of saref:Property."@en .


###  https://saref.etsi.org/core/PropertyOfInterest
<https://saref.etsi.org/core/PropertyOfInterest> rdf:type owl:Class ;
                                                 rdfs:subClassOf [ rdf:type owl:Restriction ;
                                                                   owl:onProperty <https://saref.etsi.org/core/consistsOf> ;
                                                                   owl:allValuesFrom [ rdf:type owl:Class ;
                                                                                       owl:unionOf ( <https://saref.etsi.org/core/FeatureKind>
                                                                                                     <https://saref.etsi.org/core/Property>
                                                                                                     <https://saref.etsi.org/core/PropertyOfInterest>
                                                                                                     <https://saref.etsi.org/core/State>
                                                                                                     <https://saref.etsi.org/core/StateOfInterest>
                                                                                                   )
                                                                                     ]
                                                                 ] ,
                                                                 [ rdf:type owl:Restriction ;
                                                                   owl:onProperty <https://saref.etsi.org/core/isPropertyOfInterestOf> ;
                                                                   owl:cardinality "1"^^xsd:nonNegativeInteger
                                                                 ] ;
                                                 rdfs:comment "Identifiable qualities of features of interest that can be target of devices, such as observed or controlled. An instance of saref:PropertyOfInterest is specific to a feature of interest. It is inherent to and cannot exist without that feature of interest."@en ;
                                                 rdfs:label "Property of Interest"@en ;
                                                 <http://www.w3.org/2004/02/skos/core#example> """The air temperature of the atmosphere sample at a certain location and altitude, the received signal strength indicator of an wireless IoT connection, the luminance of the ETSI ATHENA amphitheatre.

<etsi_premises/athena#luminance> a saref:PropertyOfInterest ;
    saref:isPropertyOfInterestOf <etsi_premises/athena> ;
    saref:hasPropertyKind saref:Luminance ;
    rdfs:comment \"The luminance of amphitheatre ATHENA\"@en .
"""@en ;
                                                 <http://www.w3.org/2004/02/skos/core#historyNote> "V3.2.1: Introduced saref:PropertyOfInterest to solved the ambiguity between generic vs specific properties."@en ;
                                                 <http://www.w3.org/2004/02/skos/core#note> "A property of interest is the property of (OP saref:isPropertyOfInterestOf) exactly one feature of interest."@en ,
                                                                                            "Per convention, the IRI of properties of interest should consist of the IRI of their feature of interest, suffixed with a fragment identifier #{P} where {P} refers to the name of the property."@en ,
                                                                                            "Properties of interest need not always be explicited. It depends on the use case. Typically, properties of interest are useful in applications, where the association between a feature of interest and a property (i.e., the property of interest) needs to be identified and related to other properties of interest."@en .


###  https://saref.etsi.org/core/PropertyValue
<https://saref.etsi.org/core/PropertyValue> rdf:type owl:Class ;
                                            rdfs:subClassOf [ rdf:type owl:Restriction ;
                                                              owl:onProperty <https://saref.etsi.org/core/consistsOf> ;
                                                              owl:allValuesFrom [ rdf:type owl:Class ;
                                                                                  owl:unionOf ( <https://saref.etsi.org/core/FeatureKind>
                                                                                                <https://saref.etsi.org/core/FeatureOfInterest>
                                                                                                <https://saref.etsi.org/core/Property>
                                                                                                <https://saref.etsi.org/core/PropertyOfInterest>
                                                                                                <https://saref.etsi.org/core/PropertyValue>
                                                                                                <https://saref.etsi.org/core/State>
                                                                                                <https://saref.etsi.org/core/StateOfInterest>
                                                                                                <https://saref.etsi.org/core/StateValue>
                                                                                              )
                                                                                ]
                                                            ] ,
                                                            [ rdf:type owl:Restriction ;
                                                              owl:onProperty <https://saref.etsi.org/core/isMeasuredIn> ;
                                                              owl:maxCardinality "1"^^xsd:nonNegativeInteger
                                                            ] ,
                                                            [ rdf:type owl:Restriction ;
                                                              owl:onProperty <https://saref.etsi.org/core/hasValue> ;
                                                              owl:maxCardinality "1"^^xsd:nonNegativeInteger
                                                            ] ;
                                            rdfs:comment "Describes the value for a property. The property value is optionally linked to its value expressed as an RDF literal (DP saref:hasValue), optionally to the unit of measurement (OP saref:isMeasuredIn), and optionally to the properties or properties of interest it is a value of (OP saref:isValueOfProperty)."@en ;
                                            rdfs:label "Property Value"@en ;
                                            <http://www.w3.org/2004/02/skos/core#historyNote> "V3.2.1: Introduced saref:PropertyValue to simplify the association of a measure to a property, without always needing it to be a measurement made by a device."@en ,
                                                                                              "V4.1.1: saref:hasValue is now optional on saref:PropertyValue."@en .


###  https://saref.etsi.org/core/Sensor
<https://saref.etsi.org/core/Sensor> rdf:type owl:Class ;
                                     rdfs:subClassOf <https://saref.etsi.org/core/Device> ,
                                                     [ rdf:type owl:Restriction ;
                                                       owl:onProperty <https://saref.etsi.org/core/observes> ;
                                                       owl:minCardinality "1"^^xsd:nonNegativeInteger
                                                     ] ;
                                     rdfs:comment "A device designed to observe and measure one or more properties or states of one or more features of interest."@en ;
                                     rdfs:label "Sensor"@en ;
                                     <http://www.w3.org/2004/02/skos/core#historyNote> "V3.2.1: Definition of Sensor is simplified and grounded on saref:observes. Local restriction on saref:hasFunction is deleted."@en ,
                                                                                       "V4.1.1: Definition of Sensor and Meter are updated to better distinguish one from the other."@en .


###  https://saref.etsi.org/core/Service
<https://saref.etsi.org/core/Service> rdf:type owl:Class ;
                                      rdfs:subClassOf [ rdf:type owl:Restriction ;
                                                        owl:onProperty <https://saref.etsi.org/core/represents> ;
                                                        owl:allValuesFrom [ rdf:type owl:Class ;
                                                                            owl:unionOf ( <https://saref.etsi.org/core/Function>
                                                                                          <https://saref.etsi.org/core/FunctionOfInterest>
                                                                                        )
                                                                          ]
                                                      ] ,
                                                      [ rdf:type owl:Restriction ;
                                                        owl:onProperty <https://saref.etsi.org/core/represents> ;
                                                        owl:minQualifiedCardinality "1"^^xsd:nonNegativeInteger ;
                                                        owl:onClass <https://saref.etsi.org/core/FunctionOfInterest>
                                                      ] ,
                                                      [ rdf:type owl:Restriction ;
                                                        owl:onProperty <https://saref.etsi.org/core/isOfferedBy> ;
                                                        owl:cardinality "1"^^xsd:nonNegativeInteger
                                                      ] ;
                                      rdfs:comment "A saref:Service is a digital representation of a function in a network, making it discoverable, registerable and remotely controllable in the network."@en ;
                                      rdfs:label "Service"@en ;
                                      <http://www.w3.org/2004/02/skos/core#example> "For example, a light switch can offer the service of remotely switching the lights in a home through mobile phone devices that are connected to the local network (ex:SwitchOnService class). This \"remote switching\" service represents the ex:OnOffFunction."@en ;
                                      <http://www.w3.org/2004/02/skos/core#historyNote> "V3.2.1: Simplified definition of saref:Service. Added examples."@en ;
                                      <http://www.w3.org/2004/02/skos/core#note> "Typically, a device connected to a given network offers one service for each of its functions of interest."@en .


###  https://saref.etsi.org/core/State
<https://saref.etsi.org/core/State> rdf:type owl:Class ;
                                    rdfs:subClassOf [ rdf:type owl:Restriction ;
                                                      owl:onProperty <http://www.w3.org/2004/02/skos/core#broader> ;
                                                      owl:allValuesFrom <https://saref.etsi.org/core/State>
                                                    ] ,
                                                    [ rdf:type owl:Restriction ;
                                                      owl:onProperty <http://www.w3.org/2004/02/skos/core#narrower> ;
                                                      owl:allValuesFrom <https://saref.etsi.org/core/State>
                                                    ] ;
                                    rdfs:comment "Identifiable conditions that features of interest are or may be in, and that can be target of devices, such as observed and controlled. A state can apply to different features of interest."@en ;
                                    rdfs:label "State"@en ;
                                    <http://www.w3.org/2004/02/skos/core#example> "A switch can be found in the saref:OnOffState."@en ;
                                    <http://www.w3.org/2004/02/skos/core#historyNote> "V3.2.1: Clarified and generalized definition of saref:State. Can now apply to all features of interest, not just devices."@en ;
                                    <http://www.w3.org/2004/02/skos/core#note> "Concepts from existing code lists, vocabularies, and taxonomies, may be used as instances of saref:State."@en ,
                                                                               "SAREF is not restricted to binary states such as the ex:OnOffState, but allows to define also enumerated states."@en .


###  https://saref.etsi.org/core/StateOfInterest
<https://saref.etsi.org/core/StateOfInterest> rdf:type owl:Class ;
                                              rdfs:subClassOf [ rdf:type owl:Restriction ;
                                                                owl:onProperty <https://saref.etsi.org/core/isStateOfInterestOf> ;
                                                                owl:cardinality "1"^^xsd:nonNegativeInteger
                                                              ] ;
                                              rdfs:comment "Identifiable conditions that features of interest are or may be in, and that can be target of devices, such as observed and controlled. An instance of saref:StateOfInterest is specific to a feature of interest. It is inherent to and cannot exist without that feature of interest."@en ;
                                              rdfs:label "State of Interest"@en ;
                                              <http://www.w3.org/2004/02/skos/core#historyNote> "V3.2.1: Introduced saref:StateOfInterest, parallel to saref:PropertyOfInterest."@en ;
                                              <http://www.w3.org/2004/02/skos/core#note> "A state of interest is the state of (OP saref:isStateOfInterestOf) exactly one feature of interest."@en ,
                                                                                         "Per convention, the IRI of states of interest should consist of the IRI of their feature of interest, suffixed with a fragment identifier #{S} where {S} refers to the name of the state."@en ,
                                                                                         "States of interest need not always be explicited. It depends on the use case. Typically, states of interest are useful in applications, where the association between a feature of interest and a state (i.e., the state of interest) needs to be identified and related to other states of interest."@en .


###  https://saref.etsi.org/core/StateValue
<https://saref.etsi.org/core/StateValue> rdf:type owl:Class ;
                                         rdfs:comment "Describes the value for a state. The state value is optionally linked the states or states of interest it is a value of (OP saref:isValueOfState)."@en ;
                                         rdfs:label "State Value"@en ;
                                         <http://www.w3.org/2004/02/skos/core#historyNote> "V4.1.1: Introduced saref:StateValue."@en .


###  https://saref.etsi.org/core/Task
<https://saref.etsi.org/core/Task> rdf:type owl:Class ;
                                   rdfs:subClassOf [ rdf:type owl:Restriction ;
                                                     owl:onProperty <http://www.w3.org/2004/02/skos/core#broader> ;
                                                     owl:allValuesFrom <https://saref.etsi.org/core/Task>
                                                   ] ,
                                                   [ rdf:type owl:Restriction ;
                                                     owl:onProperty <http://www.w3.org/2004/02/skos/core#narrower> ;
                                                     owl:allValuesFrom <https://saref.etsi.org/core/Task>
                                                   ] ;
                                   rdfs:comment "The goal for which a device is designed, from a user perspective."@en ;
                                   rdfs:label "Task"@en ;
                                   <http://www.w3.org/2004/02/skos/core#example> "For example, a washing machine is designed for the task of washing."@en ;
                                   <http://www.w3.org/2004/02/skos/core#note> "Tasks can be accomplished by devices (saref:isAccomplishedBy)."@en .


###  https://saref.etsi.org/core/UnitOfMeasure
<https://saref.etsi.org/core/UnitOfMeasure> rdf:type owl:Class ;
                                            rdfs:comment "The unit of measure is a standard for measurement of a quantity, such as a Property."@en ;
                                            rdfs:label "Unit of measure"@en ;
                                            <http://www.w3.org/2004/02/skos/core#example> "For example, consumption power is a property and Watt is a unit of power that represents a definite predetermined power: when we say 10 Watt, we actually mean 10 times the definite predetermined power \"Watt\"."@en ;
                                            <http://www.w3.org/2004/02/skos/core#note> "Concepts from existing code lists, vocabularies, and taxonomies, may be used as instances of saref:UnitOfMeasure. For example the QUDT Unit vocabulary"@en ,
                                                                                       "Our definition is based on the definition of unit of measure in the Ontology of units of Measure (OM)."@en .


###  https://saref.etsi.org/saref4bldg/Actuator
<https://saref.etsi.org/saref4bldg/Actuator> rdf:type owl:Class ;
                                             rdfs:subClassOf <https://saref.etsi.org/core/Actuator> ,
                                                             <https://saref.etsi.org/saref4bldg/DistributionControlDevice> ;
                                             <http://purl.org/dc/terms/source> <https://standards.buildingsmart.org/IFC/RELEASE/IFC4_1/FINAL/HTML/schema/ifcbuildingcontrolsdomain/lexical/ifcactuator.htm> ,
                                                                               <https://standards.buildingsmart.org/IFC/RELEASE/IFC4_1/FINAL/HTML/schema/ifcbuildingcontrolsdomain/pset/pset_actuatortypecommon.htm> ;
                                             rdfs:comment "An actuator is a mechanical device for moving or controlling a mechanism or system. An actuator takes energy, usually created by air, electricity, or liquid, and converts that into some kind of motion."@en ;
                                             rdfs:label "Actuator"@en ;
                                             rdfs:seeAlso "https://w3id.org/ifc/IFC4_ADD1#IfcActuator" .


###  https://saref.etsi.org/saref4bldg/AirToAirHeatRecovery
<https://saref.etsi.org/saref4bldg/AirToAirHeatRecovery> rdf:type owl:Class ;
                                                         rdfs:subClassOf <https://saref.etsi.org/saref4bldg/EnergyConversionDevice> ,
                                                                         [ rdf:type owl:Restriction ;
                                                                           owl:onProperty <https://saref.etsi.org/core/hasProperty> ;
                                                                           owl:hasValue <https://saref.etsi.org/saref4bldg/operationTemperatureMax>
                                                                         ] ,
                                                                         [ rdf:type owl:Restriction ;
                                                                           owl:onProperty <https://saref.etsi.org/core/hasProperty> ;
                                                                           owl:hasValue <https://saref.etsi.org/saref4bldg/operationTemperatureMin>
                                                                         ] ,
                                                                         [ rdf:type owl:Restriction ;
                                                                           owl:onProperty <https://saref.etsi.org/core/hasProperty> ;
                                                                           owl:hasValue <https://saref.etsi.org/saref4bldg/primaryAirFlowRateMax>
                                                                         ] ,
                                                                         [ rdf:type owl:Restriction ;
                                                                           owl:onProperty <https://saref.etsi.org/core/hasProperty> ;
                                                                           owl:hasValue <https://saref.etsi.org/saref4bldg/primaryAirFlowRateMin>
                                                                         ] ,
                                                                         [ rdf:type owl:Restriction ;
                                                                           owl:onProperty <https://saref.etsi.org/core/hasProperty> ;
                                                                           owl:hasValue <https://saref.etsi.org/saref4bldg/secondaryAirFlowRateMax>
                                                                         ] ,
                                                                         [ rdf:type owl:Restriction ;
                                                                           owl:onProperty <https://saref.etsi.org/core/hasProperty> ;
                                                                           owl:hasValue <https://saref.etsi.org/saref4bldg/secondaryAirFlowRateMin>
                                                                         ] ;
                                                         <http://purl.org/dc/terms/source> <https://standards.buildingsmart.org/IFC/RELEASE/IFC4_1/FINAL/HTML/schema/ifchvacdomain/lexical/ifcairtoairheatrecovery.htm> ,
                                                                                           <https://standards.buildingsmart.org/IFC/RELEASE/IFC4_1/FINAL/HTML/schema/ifchvacdomain/pset/pset_airtoairheatrecoverytypecommon.htm> ;
                                                         rdfs:comment "An air-to-air heat recovery device employs a counter-flow heat exchanger between inbound and outbound air flow. It is typically used to transfer heat from warmer air in one chamber to cooler air in the second chamber (i.e., typically used to recover heat from the conditioned air being exhausted and the outside air being supplied to a building), resulting in energy savings from reduced heating (or cooling) requirements."@en ;
                                                         rdfs:label "Air to air heat recovery"@en ;
                                                         rdfs:seeAlso "https://w3id.org/ifc/IFC4_ADD1#IfcAirToAirHeatRecovery" .


###  https://saref.etsi.org/saref4bldg/Alarm
<https://saref.etsi.org/saref4bldg/Alarm> rdf:type owl:Class ;
                                          rdfs:subClassOf <https://saref.etsi.org/saref4bldg/DistributionControlDevice> ;
                                          <http://purl.org/dc/terms/source> <https://standards.buildingsmart.org/IFC/RELEASE/IFC4_1/FINAL/HTML/schema/ifcbuildingcontrolsdomain/lexical/ifcalarm.htm> ,
                                                                            <https://standards.buildingsmart.org/IFC/RELEASE/IFC4_1/FINAL/HTML/schema/ifcbuildingcontrolsdomain/pset/pset_alarmtypecommon.htm> ;
                                          rdfs:comment """An alarm is a device that signals the existence of a condition or situation that is outside the boundaries of normal expectation or that activates such a device.

Alarms include the provision of break glass buttons and manual pull boxes that are used to activate alarms."""@en ;
                                          rdfs:label "Alarm"@en ;
                                          rdfs:seeAlso "https://w3id.org/ifc/IFC4_ADD1#IfcAlarm" .


###  https://saref.etsi.org/saref4bldg/AudioVisualAppliance
<https://saref.etsi.org/saref4bldg/AudioVisualAppliance> rdf:type owl:Class ;
                                                         rdfs:subClassOf <https://saref.etsi.org/saref4bldg/FlowTerminal> ,
                                                                         [ rdf:type owl:Restriction ;
                                                                           owl:onProperty <https://saref.etsi.org/core/hasProperty> ;
                                                                           owl:hasValue <https://saref.etsi.org/saref4bldg/audioVolume>
                                                                         ] ;
                                                         <http://purl.org/dc/terms/source> <https://standards.buildingsmart.org/IFC/RELEASE/IFC4_1/FINAL/HTML/schema/ifcelectricaldomain/lexical/ifcaudiovisualappliance.htm> ,
                                                                                           <https://standards.buildingsmart.org/IFC/RELEASE/IFC4_1/FINAL/HTML/schema/ifcelectricaldomain/pset/pset_audiovisualappliancetypecommon.htm> ;
                                                         rdfs:comment """An audio-visual appliance is a device that displays, captures, transmits, or receives audio or video.

Audio-visual appliances may be fixed in place or may be able to be moved from one space to another. They may require an electrical supply that may be supplied either by an electrical circuit or provided from a local battery source. Audio-visual appliances may be connected to data circuits including specialist circuits for audio visual purposes only."""@en ;
                                                         rdfs:label "Audio visual appliance"@en ;
                                                         rdfs:seeAlso "https://w3id.org/ifc/IFC4_ADD1#IfcAudioVisualApplicance" .


###  https://saref.etsi.org/saref4bldg/Boiler
<https://saref.etsi.org/saref4bldg/Boiler> rdf:type owl:Class ;
                                           rdfs:subClassOf <https://saref.etsi.org/saref4bldg/EnergyConversionDevice> ,
                                                           [ rdf:type owl:Restriction ;
                                                             owl:onProperty <https://saref.etsi.org/core/hasProperty> ;
                                                             owl:hasValue <https://saref.etsi.org/saref4bldg/heatTransferSurfaceArea>
                                                           ] ,
                                                           [ rdf:type owl:Restriction ;
                                                             owl:onProperty <https://saref.etsi.org/core/hasProperty> ;
                                                             owl:hasValue <https://saref.etsi.org/saref4bldg/nominalEnergyConsumption>
                                                           ] ,
                                                           [ rdf:type owl:Restriction ;
                                                             owl:onProperty <https://saref.etsi.org/core/hasProperty> ;
                                                             owl:hasValue <https://saref.etsi.org/saref4bldg/nominalPartLoadRatio>
                                                           ] ,
                                                           [ rdf:type owl:Restriction ;
                                                             owl:onProperty <https://saref.etsi.org/core/hasProperty> ;
                                                             owl:hasValue <https://saref.etsi.org/saref4bldg/outletTemperatureMax>
                                                           ] ,
                                                           [ rdf:type owl:Restriction ;
                                                             owl:onProperty <https://saref.etsi.org/core/hasProperty> ;
                                                             owl:hasValue <https://saref.etsi.org/saref4bldg/outletTemperatureMin>
                                                           ] ,
                                                           [ rdf:type owl:Restriction ;
                                                             owl:onProperty <https://saref.etsi.org/core/hasProperty> ;
                                                             owl:hasValue <https://saref.etsi.org/saref4bldg/pressureRating>
                                                           ] ,
                                                           [ rdf:type owl:Restriction ;
                                                             owl:onProperty <https://saref.etsi.org/core/hasProperty> ;
                                                             owl:hasValue <https://saref.etsi.org/saref4bldg/waterInletTemperatureMax>
                                                           ] ,
                                                           [ rdf:type owl:Restriction ;
                                                             owl:onProperty <https://saref.etsi.org/core/hasProperty> ;
                                                             owl:hasValue <https://saref.etsi.org/saref4bldg/waterInletTemperatureMin>
                                                           ] ,
                                                           [ rdf:type owl:Restriction ;
                                                             owl:onProperty <https://saref.etsi.org/core/hasProperty> ;
                                                             owl:hasValue <https://saref.etsi.org/saref4bldg/waterStorageCapacity>
                                                           ] ;
                                           <http://purl.org/dc/terms/source> <https://standards.buildingsmart.org/IFC/RELEASE/IFC4_1/FINAL/HTML/schema/ifchvacdomain/lexical/ifcboiler.htm> ,
                                                                             <https://standards.buildingsmart.org/IFC/RELEASE/IFC4_1/FINAL/HTML/schema/ifchvacdomain/pset/pset_boilertypecommon.htm> ;
                                           rdfs:comment "A boiler is a closed, pressure-rated vessel in which water or other fluid is heated using an energy source such as natural gas, heating oil, or electricity. The fluid in the vessel is then circulated out of the boiler for use in various processes or heating applications."@en ;
                                           rdfs:label "Boiler"@en ;
                                           rdfs:seeAlso "https://w3id.org/ifc/IFC4_ADD1#IfcBoiler" .


###  https://saref.etsi.org/saref4bldg/Building
<https://saref.etsi.org/saref4bldg/Building> rdf:type owl:Class ;
                                             rdfs:subClassOf <http://www.opengis.net/ont/geosparql#SpatialThing> ,
                                                             [ rdf:type owl:Restriction ;
                                                               owl:onProperty <https://saref.etsi.org/saref4bldg/hasSpace> ;
                                                               owl:allValuesFrom <https://saref.etsi.org/saref4bldg/BuildingSpace>
                                                             ] ;
                                             <http://purl.org/dc/terms/source> <https://standards.buildingsmart.org/IFC/RELEASE/IFC4_1/FINAL/HTML/schema/ifcproductextension/lexical/ifcbuilding.htm> ;
                                             rdfs:comment "A building represents a structure that provides shelter for its occupants or contents and stands in one place. The building is also used to provide a basic element within the spatial structure hierarchy for the components of a building project (together with site, storey, and space)."@en ;
                                             rdfs:label "Building"@en ;
                                             rdfs:seeAlso <https://w3id.org/ifc/IFC4_ADD1#IfcBuilding> .


###  https://saref.etsi.org/saref4bldg/BuildingDevice
<https://saref.etsi.org/saref4bldg/BuildingDevice> rdf:type owl:Class ;
                                                   rdfs:subClassOf <https://saref.etsi.org/core/Device> ,
                                                                   <https://saref.etsi.org/saref4bldg/BuildingObject> ;
                                                   rdfs:comment "A tangible object designed to accomplish a particular task in a building."@en ;
                                                   rdfs:label "Building device"@en .


###  https://saref.etsi.org/saref4bldg/BuildingObject
<https://saref.etsi.org/saref4bldg/BuildingObject> rdf:type owl:Class ;
                                                   rdfs:subClassOf <https://saref.etsi.org/saref4bldg/PhysicalObject> ;
                                                   rdfs:comment "An object in the building that can be controlled by devices, such as a door or a window that can be automatically opened or closed by an actuator.  (Definition taken from SAREF 1.0)"@en ;
                                                   rdfs:label "Building object"@en .


###  https://saref.etsi.org/saref4bldg/BuildingSpace
<https://saref.etsi.org/saref4bldg/BuildingSpace> rdf:type owl:Class ;
                                                  rdfs:subClassOf <http://www.opengis.net/ont/geosparql#SpatialThing> ,
                                                                  [ rdf:type owl:Restriction ;
                                                                    owl:onProperty <https://saref.etsi.org/saref4bldg/contains> ;
                                                                    owl:allValuesFrom <https://saref.etsi.org/saref4bldg/PhysicalObject>
                                                                  ] ,
                                                                  [ rdf:type owl:Restriction ;
                                                                    owl:onProperty <https://saref.etsi.org/saref4bldg/hasSpace> ;
                                                                    owl:allValuesFrom <https://saref.etsi.org/saref4bldg/BuildingSpace>
                                                                  ] ,
                                                                  [ rdf:type owl:Restriction ;
                                                                    owl:onProperty <https://saref.etsi.org/saref4bldg/isSpaceOf> ;
                                                                    owl:allValuesFrom [ rdf:type owl:Class ;
                                                                                        owl:unionOf ( <https://saref.etsi.org/saref4bldg/Building>
                                                                                                      <https://saref.etsi.org/saref4bldg/BuildingSpace>
                                                                                                    )
                                                                                      ]
                                                                  ] ;
                                                  rdfs:comment "An entity used to define the physical spaces of the building. A building space contains devices or building objects."@en ;
                                                  rdfs:label "Building space"@en .


###  https://saref.etsi.org/saref4bldg/Burner
<https://saref.etsi.org/saref4bldg/Burner> rdf:type owl:Class ;
                                           rdfs:subClassOf <https://saref.etsi.org/saref4bldg/EnergyConversionDevice> ;
                                           <http://purl.org/dc/terms/source> <https://standards.buildingsmart.org/IFC/RELEASE/IFC4_1/FINAL/HTML/schema/ifchvacdomain/lexical/ifcburner.htm> ,
                                                                             <https://standards.buildingsmart.org/IFC/RELEASE/IFC4_1/FINAL/HTML/schema/ifchvacdomain/pset/pset_burnertypecommon.htm> ;
                                           rdfs:comment "A burner is a device that converts fuel into heat through combustion. It includes gas, oil, and wood burners."@en ;
                                           rdfs:label "Burner"@en ;
                                           rdfs:seeAlso "https://w3id.org/ifc/IFC4_ADD1#IfcBurner" .


###  https://saref.etsi.org/saref4bldg/Chiller
<https://saref.etsi.org/saref4bldg/Chiller> rdf:type owl:Class ;
                                            rdfs:subClassOf <https://saref.etsi.org/saref4bldg/EnergyConversionDevice> ,
                                                            [ rdf:type owl:Restriction ;
                                                              owl:onProperty <https://saref.etsi.org/core/hasProperty> ;
                                                              owl:hasValue <https://saref.etsi.org/saref4bldg/nominalCapacity>
                                                            ] ,
                                                            [ rdf:type owl:Restriction ;
                                                              owl:onProperty <https://saref.etsi.org/core/hasProperty> ;
                                                              owl:hasValue <https://saref.etsi.org/saref4bldg/nominalCondensingTemperature>
                                                            ] ,
                                                            [ rdf:type owl:Restriction ;
                                                              owl:onProperty <https://saref.etsi.org/core/hasProperty> ;
                                                              owl:hasValue <https://saref.etsi.org/saref4bldg/nominalEfficiency>
                                                            ] ,
                                                            [ rdf:type owl:Restriction ;
                                                              owl:onProperty <https://saref.etsi.org/core/hasProperty> ;
                                                              owl:hasValue <https://saref.etsi.org/saref4bldg/nominalEvaporatingTemmperature>
                                                            ] ,
                                                            [ rdf:type owl:Restriction ;
                                                              owl:onProperty <https://saref.etsi.org/core/hasProperty> ;
                                                              owl:hasValue <https://saref.etsi.org/saref4bldg/nominalHeatRejectionRate>
                                                            ] ,
                                                            [ rdf:type owl:Restriction ;
                                                              owl:onProperty <https://saref.etsi.org/core/hasProperty> ;
                                                              owl:hasValue <https://saref.etsi.org/saref4bldg/nominalPowerConsumption>
                                                            ] ;
                                            <http://purl.org/dc/terms/source> <https://standards.buildingsmart.org/IFC/RELEASE/IFC4_1/FINAL/HTML/schema/ifchvacdomain/lexical/ifcchiller.htm> ,
                                                                              <https://standards.buildingsmart.org/IFC/RELEASE/IFC4_1/FINAL/HTML/schema/ifchvacdomain/pset/pset_chillertypecommon.htm> ;
                                            rdfs:comment "A chiller is a device used to remove heat from a liquid via a vapor-compression or absorption refrigeration cycle to cool a fluid, typically water or a mixture of water and glycol. The chilled fluid is then used to cool and dehumidify air in a building."@en ;
                                            rdfs:label "Chiller"@en ;
                                            rdfs:seeAlso "https://w3id.org/ifc/IFC4_ADD1#IfcChiller" .


###  https://saref.etsi.org/saref4bldg/Coil
<https://saref.etsi.org/saref4bldg/Coil> rdf:type owl:Class ;
                                         rdfs:subClassOf <https://saref.etsi.org/saref4bldg/EnergyConversionDevice> ,
                                                         [ rdf:type owl:Restriction ;
                                                           owl:onProperty <https://saref.etsi.org/core/hasProperty> ;
                                                           owl:hasValue <https://saref.etsi.org/saref4bldg/airFlowRateMax>
                                                         ] ,
                                                         [ rdf:type owl:Restriction ;
                                                           owl:onProperty <https://saref.etsi.org/core/hasProperty> ;
                                                           owl:hasValue <https://saref.etsi.org/saref4bldg/airFlowRateMin>
                                                         ] ,
                                                         [ rdf:type owl:Restriction ;
                                                           owl:onProperty <https://saref.etsi.org/core/hasProperty> ;
                                                           owl:hasValue <https://saref.etsi.org/saref4bldg/nominalLatentCapacity>
                                                         ] ,
                                                         [ rdf:type owl:Restriction ;
                                                           owl:onProperty <https://saref.etsi.org/core/hasProperty> ;
                                                           owl:hasValue <https://saref.etsi.org/saref4bldg/nominalSensibleCapacity>
                                                         ] ,
                                                         [ rdf:type owl:Restriction ;
                                                           owl:onProperty <https://saref.etsi.org/core/hasProperty> ;
                                                           owl:hasValue <https://saref.etsi.org/saref4bldg/nominalUa>
                                                         ] ,
                                                         [ rdf:type owl:Restriction ;
                                                           owl:onProperty <https://saref.etsi.org/core/hasProperty> ;
                                                           owl:hasValue <https://saref.etsi.org/saref4bldg/operationTemperatureMax>
                                                         ] ,
                                                         [ rdf:type owl:Restriction ;
                                                           owl:onProperty <https://saref.etsi.org/core/hasProperty> ;
                                                           owl:hasValue <https://saref.etsi.org/saref4bldg/operationTemperatureMin>
                                                         ] ;
                                         <http://purl.org/dc/terms/source> <https://standards.buildingsmart.org/IFC/RELEASE/IFC4_1/FINAL/HTML/schema/ifchvacdomain/lexical/ifccoil.htm> ,
                                                                           <https://standards.buildingsmart.org/IFC/RELEASE/IFC4_1/FINAL/HTML/schema/ifchvacdomain/pset/pset_coiltypecommon.htm> ;
                                         rdfs:comment """A coil is a device used to provide heat transfer between non-mixing media. A common example is a cooling coil, which utilizes a finned coil in which circulates chilled water, antifreeze, or refrigerant that is used to remove heat from air moving across the surface of the coil. A coil may be used either for heating or cooling purposes by placing a series of tubes (the coil) carrying a heating or cooling fluid into an airstream. The coil may be constructed from tubes bundled in a serpentine form or from finned tubes that give a extended heat transfer surface.

Coils may also be used for non-airflow cases such as embedded in a floor slab."""@en ;
                                         rdfs:label "Coil"@en ;
                                         rdfs:seeAlso "https://w3id.org/ifc/IFC4_ADD1#IfcCoil" .


###  https://saref.etsi.org/saref4bldg/CommunicationAppliance
<https://saref.etsi.org/saref4bldg/CommunicationAppliance> rdf:type owl:Class ;
                                                           rdfs:subClassOf <https://saref.etsi.org/saref4bldg/FlowTerminal> ;
                                                           <http://purl.org/dc/terms/source> <https://standards.buildingsmart.org/IFC/RELEASE/IFC4_1/FINAL/HTML/schema/ifcelectricaldomain/lexical/ifccommunicationsappliance.htm> ,
                                                                                             <https://standards.buildingsmart.org/IFC/RELEASE/IFC4_1/FINAL/HTML/schema/ifcelectricaldomain/pset/pset_communicationsappliancetypecommon.htm> ;
                                                           rdfs:comment """A communications appliance transmits and receives electronic or digital information as data or sound.

Communication appliances may be fixed in place or may be able to be moved from one space to another. Communication appliances require an electrical supply that may be supplied either by an electrical circuit or provided from a local battery source."""@en ;
                                                           rdfs:label "Communication appliance"@en ;
                                                           rdfs:seeAlso "https://w3id.org/ifc/IFC4_ADD1#IfcCommunicationAppliance" .


###  https://saref.etsi.org/saref4bldg/Compressor
<https://saref.etsi.org/saref4bldg/Compressor> rdf:type owl:Class ;
                                               rdfs:subClassOf <https://saref.etsi.org/saref4bldg/FlowMovingDevice> ,
                                                               [ rdf:type owl:Restriction ;
                                                                 owl:onProperty <https://saref.etsi.org/core/hasProperty> ;
                                                                 owl:hasValue <https://saref.etsi.org/saref4bldg/compressorSpeed>
                                                               ] ,
                                                               [ rdf:type owl:Restriction ;
                                                                 owl:onProperty <https://saref.etsi.org/core/hasProperty> ;
                                                                 owl:hasValue <https://saref.etsi.org/saref4bldg/idealCapacity>
                                                               ] ,
                                                               [ rdf:type owl:Restriction ;
                                                                 owl:onProperty <https://saref.etsi.org/core/hasProperty> ;
                                                                 owl:hasValue <https://saref.etsi.org/saref4bldg/idealShaftPower>
                                                               ] ,
                                                               [ rdf:type owl:Restriction ;
                                                                 owl:onProperty <https://saref.etsi.org/core/hasProperty> ;
                                                                 owl:hasValue <https://saref.etsi.org/saref4bldg/impellerDiameter>
                                                               ] ,
                                                               [ rdf:type owl:Restriction ;
                                                                 owl:onProperty <https://saref.etsi.org/core/hasProperty> ;
                                                                 owl:hasValue <https://saref.etsi.org/saref4bldg/nominalCapacity>
                                                               ] ,
                                                               [ rdf:type owl:Restriction ;
                                                                 owl:onProperty <https://saref.etsi.org/core/hasProperty> ;
                                                                 owl:hasValue <https://saref.etsi.org/saref4bldg/partLoadRatioMax>
                                                               ] ,
                                                               [ rdf:type owl:Restriction ;
                                                                 owl:onProperty <https://saref.etsi.org/core/hasProperty> ;
                                                                 owl:hasValue <https://saref.etsi.org/saref4bldg/partLoadRatioMin>
                                                               ] ;
                                               <http://purl.org/dc/terms/source> <https://standards.buildingsmart.org/IFC/RELEASE/IFC4_1/FINAL/HTML/schema/ifchvacdomain/lexical/ifccompressor.htm> ,
                                                                                 <https://standards.buildingsmart.org/IFC/RELEASE/IFC4_1/FINAL/HTML/schema/ifchvacdomain/pset/pset_compressortypecommon.htm> ;
                                               rdfs:comment "A compressor is a device that compresses a fluid typically used in a refrigeration circuit."@en ;
                                               rdfs:label "Compressor"@en ;
                                               rdfs:seeAlso "https://w3id.org/ifc/IFC4_ADD1#IfcCompressor" .


###  https://saref.etsi.org/saref4bldg/Condenser
<https://saref.etsi.org/saref4bldg/Condenser> rdf:type owl:Class ;
                                              rdfs:subClassOf <https://saref.etsi.org/saref4bldg/EnergyConversionDevice> ,
                                                              [ rdf:type owl:Restriction ;
                                                                owl:onProperty <https://saref.etsi.org/core/hasProperty> ;
                                                                owl:hasValue <https://saref.etsi.org/saref4bldg/externalSurfaceArea>
                                                              ] ,
                                                              [ rdf:type owl:Restriction ;
                                                                owl:onProperty <https://saref.etsi.org/core/hasProperty> ;
                                                                owl:hasValue <https://saref.etsi.org/saref4bldg/internalRefrigerantVolume>
                                                              ] ,
                                                              [ rdf:type owl:Restriction ;
                                                                owl:onProperty <https://saref.etsi.org/core/hasProperty> ;
                                                                owl:hasValue <https://saref.etsi.org/saref4bldg/internalSurfaceArea>
                                                              ] ,
                                                              [ rdf:type owl:Restriction ;
                                                                owl:onProperty <https://saref.etsi.org/core/hasProperty> ;
                                                                owl:hasValue <https://saref.etsi.org/saref4bldg/internalWaterVolume>
                                                              ] ,
                                                              [ rdf:type owl:Restriction ;
                                                                owl:onProperty <https://saref.etsi.org/core/hasProperty> ;
                                                                owl:hasValue <https://saref.etsi.org/saref4bldg/nominalHeatTransferArea>
                                                              ] ,
                                                              [ rdf:type owl:Restriction ;
                                                                owl:onProperty <https://saref.etsi.org/core/hasProperty> ;
                                                                owl:hasValue <https://saref.etsi.org/saref4bldg/nominalHeatTransferCoefficient>
                                                              ] ;
                                              <http://purl.org/dc/terms/source> <https://standards.buildingsmart.org/IFC/RELEASE/IFC4_1/FINAL/HTML/schema/ifchvacdomain/lexical/ifccondenser.htm> ,
                                                                                <https://standards.buildingsmart.org/IFC/RELEASE/IFC4_1/FINAL/HTML/schema/ifchvacdomain/pset/pset_condensertypecommon.htm> ;
                                              rdfs:comment "A condenser is a device that is used to dissipate heat, typically by condensing a substance such as a refrigerant from its gaseous to its liquid state."@en ;
                                              rdfs:label "Condenser"@en ;
                                              rdfs:seeAlso "https://w3id.org/ifc/IFC4_ADD1#IfcCondenser" .


###  https://saref.etsi.org/saref4bldg/Controller
<https://saref.etsi.org/saref4bldg/Controller> rdf:type owl:Class ;
                                               rdfs:subClassOf <https://saref.etsi.org/saref4bldg/DistributionControlDevice> ;
                                               <http://purl.org/dc/terms/source> <https://standards.buildingsmart.org/IFC/RELEASE/IFC4_1/FINAL/HTML/schema/ifcbuildingcontrolsdomain/lexical/ifccontroller.htm> ,
                                                                                 <https://standards.buildingsmart.org/IFC/RELEASE/IFC4_1/FINAL/HTML/schema/ifcbuildingcontrolsdomain/pset/pset_controllertypecommon.htm> ;
                                               rdfs:comment """A controller is a device that monitors inputs and controls outputs within a building automation system.

A controller may be physical (having placement within a spatial structure) or logical (a software interface or aggregated within a programmable physical controller)."""@en ;
                                               rdfs:label "Controller"@en ;
                                               rdfs:seeAlso "https://w3id.org/ifc/IFC4_ADD1#IfcController" .


###  https://saref.etsi.org/saref4bldg/CooledBeam
<https://saref.etsi.org/saref4bldg/CooledBeam> rdf:type owl:Class ;
                                               rdfs:subClassOf <https://saref.etsi.org/saref4bldg/EnergyConversionDevice> ,
                                                               [ rdf:type owl:Restriction ;
                                                                 owl:onProperty <https://saref.etsi.org/core/hasProperty> ;
                                                                 owl:hasValue <https://saref.etsi.org/saref4bldg/coilLength>
                                                               ] ,
                                                               [ rdf:type owl:Restriction ;
                                                                 owl:onProperty <https://saref.etsi.org/core/hasProperty> ;
                                                                 owl:hasValue <https://saref.etsi.org/saref4bldg/coilWidth>
                                                               ] ,
                                                               [ rdf:type owl:Restriction ;
                                                                 owl:onProperty <https://saref.etsi.org/core/hasProperty> ;
                                                                 owl:hasValue <https://saref.etsi.org/saref4bldg/nominalCoolingCapacity>
                                                               ] ,
                                                               [ rdf:type owl:Restriction ;
                                                                 owl:onProperty <https://saref.etsi.org/core/hasProperty> ;
                                                                 owl:hasValue <https://saref.etsi.org/saref4bldg/nominalHeatingCapacity>
                                                               ] ,
                                                               [ rdf:type owl:Restriction ;
                                                                 owl:onProperty <https://saref.etsi.org/core/hasProperty> ;
                                                                 owl:hasValue <https://saref.etsi.org/saref4bldg/nominalReturnWaterTemperatureCooling>
                                                               ] ,
                                                               [ rdf:type owl:Restriction ;
                                                                 owl:onProperty <https://saref.etsi.org/core/hasProperty> ;
                                                                 owl:hasValue <https://saref.etsi.org/saref4bldg/nominalReturnWaterTemperatureHeating>
                                                               ] ,
                                                               [ rdf:type owl:Restriction ;
                                                                 owl:onProperty <https://saref.etsi.org/core/hasProperty> ;
                                                                 owl:hasValue <https://saref.etsi.org/saref4bldg/nominalSorroundingHumidityCooling>
                                                               ] ,
                                                               [ rdf:type owl:Restriction ;
                                                                 owl:onProperty <https://saref.etsi.org/core/hasProperty> ;
                                                                 owl:hasValue <https://saref.etsi.org/saref4bldg/nominalSorroundingTemperatureCooling>
                                                               ] ,
                                                               [ rdf:type owl:Restriction ;
                                                                 owl:onProperty <https://saref.etsi.org/core/hasProperty> ;
                                                                 owl:hasValue <https://saref.etsi.org/saref4bldg/nominalSorroundingTemperatureHeating>
                                                               ] ,
                                                               [ rdf:type owl:Restriction ;
                                                                 owl:onProperty <https://saref.etsi.org/core/hasProperty> ;
                                                                 owl:hasValue <https://saref.etsi.org/saref4bldg/nominalSupplyWaterTemperatureCooling>
                                                               ] ,
                                                               [ rdf:type owl:Restriction ;
                                                                 owl:onProperty <https://saref.etsi.org/core/hasProperty> ;
                                                                 owl:hasValue <https://saref.etsi.org/saref4bldg/nominalSupplyWaterTemperatureHeating>
                                                               ] ,
                                                               [ rdf:type owl:Restriction ;
                                                                 owl:onProperty <https://saref.etsi.org/core/hasProperty> ;
                                                                 owl:hasValue <https://saref.etsi.org/saref4bldg/nominalWaterFlowCooling>
                                                               ] ,
                                                               [ rdf:type owl:Restriction ;
                                                                 owl:onProperty <https://saref.etsi.org/core/hasProperty> ;
                                                                 owl:hasValue <https://saref.etsi.org/saref4bldg/nominalWaterFlowHeating>
                                                               ] ,
                                                               [ rdf:type owl:Restriction ;
                                                                 owl:onProperty <https://saref.etsi.org/core/hasProperty> ;
                                                                 owl:hasValue <https://saref.etsi.org/saref4bldg/waterPressureMax>
                                                               ] ,
                                                               [ rdf:type owl:Restriction ;
                                                                 owl:onProperty <https://saref.etsi.org/core/hasProperty> ;
                                                                 owl:hasValue <https://saref.etsi.org/saref4bldg/waterPressureMin>
                                                               ] ;
                                               <http://purl.org/dc/terms/source> <https://standards.buildingsmart.org/IFC/RELEASE/IFC4_1/FINAL/HTML/schema/ifchvacdomain/lexical/ifccooledbeam.htm> ,
                                                                                 <https://standards.buildingsmart.org/IFC/RELEASE/IFC4_1/FINAL/HTML/schema/ifchvacdomain/pset/pset_cooledbeamtypecommon.htm> ;
                                               rdfs:comment "A cooled beam (or chilled beam) is a device typically used to cool air by circulating a fluid such as chilled water through exposed finned tubes above a space. Typically mounted overhead near or within a ceiling, the cooled beam uses convection to cool the space below it by acting as a heat sink for the naturally rising warm air of the space. Once cooled, the air naturally drops back to the floor where the cycle begins again."@en ;
                                               rdfs:label "Cooled beam"@en ;
                                               rdfs:seeAlso "https://w3id.org/ifc/IFC4_ADD1#IfcCooledBeam" .


###  https://saref.etsi.org/saref4bldg/CoolingTower
<https://saref.etsi.org/saref4bldg/CoolingTower> rdf:type owl:Class ;
                                                 rdfs:subClassOf <https://saref.etsi.org/saref4bldg/EnergyConversionDevice> ,
                                                                 [ rdf:type owl:Restriction ;
                                                                   owl:onProperty <https://saref.etsi.org/core/hasProperty> ;
                                                                   owl:hasValue <https://saref.etsi.org/saref4bldg/ambientDesignDryBulbTemperature>
                                                                 ] ,
                                                                 [ rdf:type owl:Restriction ;
                                                                   owl:onProperty <https://saref.etsi.org/core/hasProperty> ;
                                                                   owl:hasValue <https://saref.etsi.org/saref4bldg/ambientDesignWetBulbTemperature>
                                                                 ] ,
                                                                 [ rdf:type owl:Restriction ;
                                                                   owl:onProperty <https://saref.etsi.org/core/hasProperty> ;
                                                                   owl:hasValue <https://saref.etsi.org/saref4bldg/basinReserveVolume>
                                                                 ] ,
                                                                 [ rdf:type owl:Restriction ;
                                                                   owl:onProperty <https://saref.etsi.org/core/hasProperty> ;
                                                                   owl:hasValue <https://saref.etsi.org/saref4bldg/liftElevationDifference>
                                                                 ] ,
                                                                 [ rdf:type owl:Restriction ;
                                                                   owl:onProperty <https://saref.etsi.org/core/hasProperty> ;
                                                                   owl:hasValue <https://saref.etsi.org/saref4bldg/nominalCapacity>
                                                                 ] ,
                                                                 [ rdf:type owl:Restriction ;
                                                                   owl:onProperty <https://saref.etsi.org/core/hasProperty> ;
                                                                   owl:hasValue <https://saref.etsi.org/saref4bldg/operationTemperatureMax>
                                                                 ] ,
                                                                 [ rdf:type owl:Restriction ;
                                                                   owl:onProperty <https://saref.etsi.org/core/hasProperty> ;
                                                                   owl:hasValue <https://saref.etsi.org/saref4bldg/operationTemperatureMin>
                                                                 ] ,
                                                                 [ rdf:type owl:Restriction ;
                                                                   owl:onProperty <https://saref.etsi.org/core/hasProperty> ;
                                                                   owl:hasValue <https://saref.etsi.org/saref4bldg/waterRequirement>
                                                                 ] ;
                                                 <http://purl.org/dc/terms/source> <https://standards.buildingsmart.org/IFC/RELEASE/IFC4_1/FINAL/HTML/schema/ifchvacdomain/lexical/ifccoolingtower.htm> ,
                                                                                   <https://standards.buildingsmart.org/IFC/RELEASE/IFC4_1/FINAL/HTML/schema/ifchvacdomain/pset/pset_coolingtowertypecommon.htm> ;
                                                 rdfs:comment "A cooling tower is a device which rejects heat to ambient air by circulating a fluid such as water through it to reduce its temperature by partial evaporation."@en ;
                                                 rdfs:label "Cooling tower"@en ;
                                                 rdfs:seeAlso "https://w3id.org/ifc/IFC4_ADD1#IfcCoolingTower" .


###  https://saref.etsi.org/saref4bldg/Damper
<https://saref.etsi.org/saref4bldg/Damper> rdf:type owl:Class ;
                                           rdfs:subClassOf <https://saref.etsi.org/saref4bldg/FlowController> ,
                                                           [ rdf:type owl:Restriction ;
                                                             owl:onProperty <https://saref.etsi.org/core/hasProperty> ;
                                                             owl:hasValue <https://saref.etsi.org/saref4bldg/airFlowRateMax>
                                                           ] ,
                                                           [ rdf:type owl:Restriction ;
                                                             owl:onProperty <https://saref.etsi.org/core/hasProperty> ;
                                                             owl:hasValue <https://saref.etsi.org/saref4bldg/bladeThickness>
                                                           ] ,
                                                           [ rdf:type owl:Restriction ;
                                                             owl:onProperty <https://saref.etsi.org/core/hasProperty> ;
                                                             owl:hasValue <https://saref.etsi.org/saref4bldg/closeOffRating>
                                                           ] ,
                                                           [ rdf:type owl:Restriction ;
                                                             owl:onProperty <https://saref.etsi.org/core/hasProperty> ;
                                                             owl:hasValue <https://saref.etsi.org/saref4bldg/faceArea>
                                                           ] ,
                                                           [ rdf:type owl:Restriction ;
                                                             owl:onProperty <https://saref.etsi.org/core/hasProperty> ;
                                                             owl:hasValue <https://saref.etsi.org/saref4bldg/frameDepth>
                                                           ] ,
                                                           [ rdf:type owl:Restriction ;
                                                             owl:onProperty <https://saref.etsi.org/core/hasProperty> ;
                                                             owl:hasValue <https://saref.etsi.org/saref4bldg/frameThickness>
                                                           ] ,
                                                           [ rdf:type owl:Restriction ;
                                                             owl:onProperty <https://saref.etsi.org/core/hasProperty> ;
                                                             owl:hasValue <https://saref.etsi.org/saref4bldg/leakageFullyClosed>
                                                           ] ,
                                                           [ rdf:type owl:Restriction ;
                                                             owl:onProperty <https://saref.etsi.org/core/hasProperty> ;
                                                             owl:hasValue <https://saref.etsi.org/saref4bldg/nominalAirFlowRate>
                                                           ] ,
                                                           [ rdf:type owl:Restriction ;
                                                             owl:onProperty <https://saref.etsi.org/core/hasProperty> ;
                                                             owl:hasValue <https://saref.etsi.org/saref4bldg/openPressureDrop>
                                                           ] ,
                                                           [ rdf:type owl:Restriction ;
                                                             owl:onProperty <https://saref.etsi.org/core/hasProperty> ;
                                                             owl:hasValue <https://saref.etsi.org/saref4bldg/operationTemperatureMax>
                                                           ] ,
                                                           [ rdf:type owl:Restriction ;
                                                             owl:onProperty <https://saref.etsi.org/core/hasProperty> ;
                                                             owl:hasValue <https://saref.etsi.org/saref4bldg/operationTemperatureMin>
                                                           ] ,
                                                           [ rdf:type owl:Restriction ;
                                                             owl:onProperty <https://saref.etsi.org/core/hasProperty> ;
                                                             owl:hasValue <https://saref.etsi.org/saref4bldg/temperatureRating>
                                                           ] ,
                                                           [ rdf:type owl:Restriction ;
                                                             owl:onProperty <https://saref.etsi.org/core/hasProperty> ;
                                                             owl:hasValue <https://saref.etsi.org/saref4bldg/workingPressureMax>
                                                           ] ;
                                           <http://purl.org/dc/terms/source> <https://standards.buildingsmart.org/IFC/RELEASE/IFC4_1/FINAL/HTML/schema/ifchvacdomain/lexical/ifcdamper.htm> ,
                                                                             <https://standards.buildingsmart.org/IFC/RELEASE/IFC4_1/FINAL/HTML/schema/ifchvacdomain/pset/pset_dampertypecommon.htm> ;
                                           rdfs:comment "A damper typically participates in an HVAC duct distribution system and is used to control or modulate the flow of air."@en ;
                                           rdfs:label "Damper"@en ;
                                           rdfs:seeAlso "https://w3id.org/ifc/IFC4_ADD1#IfcDamper" .


###  https://saref.etsi.org/saref4bldg/DistributionControlDevice
<https://saref.etsi.org/saref4bldg/DistributionControlDevice> rdf:type owl:Class ;
                                                              rdfs:subClassOf <https://saref.etsi.org/saref4bldg/DistributionDevice> ;
                                                              rdfs:comment "Represents devices of a building automation control system that are used to impart control over elements of a distribution system. (Definition adapated from https://standards.buildingsmart.org/IFC/RELEASE/IFC4_1/FINAL/HTML/schema/ifcsharedbldgserviceelements/lexical/ifcdistributioncontrolelement.htm)"@en ;
                                                              rdfs:label "Distribution control device"@en .


###  https://saref.etsi.org/saref4bldg/DistributionDevice
<https://saref.etsi.org/saref4bldg/DistributionDevice> rdf:type owl:Class ;
                                                       rdfs:subClassOf <https://saref.etsi.org/saref4bldg/BuildingDevice> ;
                                                       rdfs:comment "Generalization of all devices that participate in a distribution system. (Definition adapated from https://standards.buildingsmart.org/IFC/RELEASE/IFC4_1/FINAL/HTML/schema/ifcproductextension/lexical/ifcdistributionelement.htm)"@en ;
                                                       rdfs:label "Distribution device"@en .


###  https://saref.etsi.org/saref4bldg/DistributionFlowDevice
<https://saref.etsi.org/saref4bldg/DistributionFlowDevice> rdf:type owl:Class ;
                                                           rdfs:subClassOf <https://saref.etsi.org/saref4bldg/DistributionDevice> ;
                                                           rdfs:comment "Represents devices of a distribution system that facilitate the distribution of energy or matter, such as air, water or power. (Definition adapated from https://standards.buildingsmart.org/IFC/RELEASE/IFC4_1/FINAL/HTML/schema/ifcsharedbldgserviceelements/lexical/ifcdistributionflowelement.htm)"@en ;
                                                           rdfs:label "DistributionFlowDevice"@en .


###  https://saref.etsi.org/saref4bldg/DuctSilencer
<https://saref.etsi.org/saref4bldg/DuctSilencer> rdf:type owl:Class ;
                                                 rdfs:subClassOf <https://saref.etsi.org/saref4bldg/FlowTreatmentDevice> ,
                                                                 [ rdf:type owl:Restriction ;
                                                                   owl:onProperty <https://saref.etsi.org/core/hasProperty> ;
                                                                   owl:hasValue <https://saref.etsi.org/saref4bldg/airFlowRateMax>
                                                                 ] ,
                                                                 [ rdf:type owl:Restriction ;
                                                                   owl:onProperty <https://saref.etsi.org/core/hasProperty> ;
                                                                   owl:hasValue <https://saref.etsi.org/saref4bldg/airFlowRateMin>
                                                                 ] ,
                                                                 [ rdf:type owl:Restriction ;
                                                                   owl:onProperty <https://saref.etsi.org/core/hasProperty> ;
                                                                   owl:hasValue <https://saref.etsi.org/saref4bldg/hydraulicDiameter>
                                                                 ] ,
                                                                 [ rdf:type owl:Restriction ;
                                                                   owl:onProperty <https://saref.etsi.org/core/hasProperty> ;
                                                                   owl:hasValue <https://saref.etsi.org/saref4bldg/length>
                                                                 ] ,
                                                                 [ rdf:type owl:Restriction ;
                                                                   owl:onProperty <https://saref.etsi.org/core/hasProperty> ;
                                                                   owl:hasValue <https://saref.etsi.org/saref4bldg/operationTemperatureMax>
                                                                 ] ,
                                                                 [ rdf:type owl:Restriction ;
                                                                   owl:onProperty <https://saref.etsi.org/core/hasProperty> ;
                                                                   owl:hasValue <https://saref.etsi.org/saref4bldg/operationTemperatureMin>
                                                                 ] ,
                                                                 [ rdf:type owl:Restriction ;
                                                                   owl:onProperty <https://saref.etsi.org/core/hasProperty> ;
                                                                   owl:hasValue <https://saref.etsi.org/saref4bldg/weight>
                                                                 ] ,
                                                                 [ rdf:type owl:Restriction ;
                                                                   owl:onProperty <https://saref.etsi.org/core/hasProperty> ;
                                                                   owl:hasValue <https://saref.etsi.org/saref4bldg/workingPressureMax>
                                                                 ] ,
                                                                 [ rdf:type owl:Restriction ;
                                                                   owl:onProperty <https://saref.etsi.org/core/hasProperty> ;
                                                                   owl:hasValue <https://saref.etsi.org/saref4bldg/workingPressureMin>
                                                                 ] ;
                                                 <http://purl.org/dc/terms/source> <https://standards.buildingsmart.org/IFC/RELEASE/IFC4_1/FINAL/HTML/schema/ifchvacdomain/lexical/ifcductsilencer.htm> ,
                                                                                   <https://standards.buildingsmart.org/IFC/RELEASE/IFC4_1/FINAL/HTML/schema/ifchvacdomain/pset/pset_ductsilencertypecommon.htm> ;
                                                 rdfs:comment "A duct silencer is a device that is typically installed inside a duct distribution system for the purpose of reducing the noise levels from air movement, fan noise, etc. in the adjacent space or downstream of the duct silencer device."@en ;
                                                 rdfs:label "Duct silencer"@en ;
                                                 rdfs:seeAlso "https://w3id.org/ifc/IFC4_ADD1#IfcDuctSilencer" .


###  https://saref.etsi.org/saref4bldg/ElectricAppliance
<https://saref.etsi.org/saref4bldg/ElectricAppliance> rdf:type owl:Class ;
                                                      rdfs:subClassOf <https://saref.etsi.org/saref4bldg/FlowTerminal> ;
                                                      <http://purl.org/dc/terms/source> <https://standards.buildingsmart.org/IFC/RELEASE/IFC4_1/FINAL/HTML/schema/ifcelectricaldomain/lexical/ifcelectricappliance.htm> ,
                                                                                        <https://standards.buildingsmart.org/IFC/RELEASE/IFC4_1/FINAL/HTML/schema/ifcelectricaldomain/pset/pset_electricappliancetypecommon.htm> ;
                                                      rdfs:comment """An electric appliance is a device intended for consumer usage that is powered by electricity.

Electric appliances may be fixed in place or may be able to be moved from one space to another. Electric appliances require an electrical supply that may be supplied either by an electrical circuit or provided from a local battery source."""@en ;
                                                      rdfs:label "Electric appliance"@en ;
                                                      rdfs:seeAlso "https://w3id.org/ifc/IFC4_ADD1#IfcElectricAppliance" .


###  https://saref.etsi.org/saref4bldg/ElectricFlowStorageDevice
<https://saref.etsi.org/saref4bldg/ElectricFlowStorageDevice> rdf:type owl:Class ;
                                                              rdfs:subClassOf <https://saref.etsi.org/saref4bldg/FlowStorageDevice> ,
                                                                              [ rdf:type owl:Restriction ;
                                                                                owl:onProperty <https://saref.etsi.org/core/hasProperty> ;
                                                                                owl:hasValue <https://saref.etsi.org/saref4bldg/nominalFrequency>
                                                                              ] ,
                                                                              [ rdf:type owl:Restriction ;
                                                                                owl:onProperty <https://saref.etsi.org/core/hasProperty> ;
                                                                                owl:hasValue <https://saref.etsi.org/saref4bldg/nominalSupplyVoltage>
                                                                              ] ,
                                                                              [ rdf:type owl:Restriction ;
                                                                                owl:onProperty <https://saref.etsi.org/core/hasProperty> ;
                                                                                owl:hasValue <https://saref.etsi.org/saref4bldg/nominalSupplyVoltageMin>
                                                                              ] ;
                                                              <http://purl.org/dc/terms/source> <https://standards.buildingsmart.org/IFC/RELEASE/IFC4_1/FINAL/HTML/schema/ifcelectricaldomain/lexical/ifcelectricflowstoragedevice.htm> ,
                                                                                                <https://standards.buildingsmart.org/IFC/RELEASE/IFC4_1/FINAL/HTML/schema/ifcelectricaldomain/pset/pset_electricflowstoragedevicetypecommon.htm> ;
                                                              rdfs:comment "An electric flow storage device is a device in which electrical energy is stored and from which energy may be progressively released."@en ;
                                                              rdfs:label "Electric flow storage device"@en ;
                                                              rdfs:seeAlso "https://w3id.org/ifc/IFC4_ADD1#IfcElectricFlowStorageDevice" .


###  https://saref.etsi.org/saref4bldg/ElectricGenerator
<https://saref.etsi.org/saref4bldg/ElectricGenerator> rdf:type owl:Class ;
                                                      rdfs:subClassOf <https://saref.etsi.org/saref4bldg/EnergyConversionDevice> ,
                                                                      [ rdf:type owl:Restriction ;
                                                                        owl:onProperty <https://saref.etsi.org/core/hasProperty> ;
                                                                        owl:hasValue <https://saref.etsi.org/saref4bldg/electricGeneratorEfficiency>
                                                                      ] ,
                                                                      [ rdf:type owl:Restriction ;
                                                                        owl:onProperty <https://saref.etsi.org/core/hasProperty> ;
                                                                        owl:hasValue <https://saref.etsi.org/saref4bldg/powerOutputMax>
                                                                      ] ,
                                                                      [ rdf:type owl:Restriction ;
                                                                        owl:onProperty <https://saref.etsi.org/core/hasProperty> ;
                                                                        owl:hasValue <https://saref.etsi.org/saref4bldg/startCurrentFactor>
                                                                      ] ;
                                                      <http://purl.org/dc/terms/source> <https://standards.buildingsmart.org/IFC/RELEASE/IFC4_1/FINAL/HTML/schema/ifcelectricaldomain/lexical/ifcelectricgenerator.htm> ,
                                                                                        <https://standards.buildingsmart.org/IFC/RELEASE/IFC4_1/FINAL/HTML/schema/ifcelectricaldomain/pset/pset_electricgeneratortypecommon.htm> ;
                                                      rdfs:comment "An electric generator is an engine that is a machine for converting mechanical energy into electrical energy."@en ;
                                                      rdfs:label "Electric generator"@en ;
                                                      rdfs:seeAlso "https://w3id.org/ifc/IFC4_ADD1#IfcElectricGenerator" .


###  https://saref.etsi.org/saref4bldg/ElectricMotor
<https://saref.etsi.org/saref4bldg/ElectricMotor> rdf:type owl:Class ;
                                                  rdfs:subClassOf <https://saref.etsi.org/saref4bldg/EnergyConversionDevice> ,
                                                                  [ rdf:type owl:Restriction ;
                                                                    owl:onProperty <https://saref.etsi.org/core/hasProperty> ;
                                                                    owl:hasValue <https://saref.etsi.org/saref4bldg/electricMotorEfficiency>
                                                                  ] ,
                                                                  [ rdf:type owl:Restriction ;
                                                                    owl:onProperty <https://saref.etsi.org/core/hasProperty> ;
                                                                    owl:hasValue <https://saref.etsi.org/saref4bldg/lockedRotorCurrent>
                                                                  ] ,
                                                                  [ rdf:type owl:Restriction ;
                                                                    owl:onProperty <https://saref.etsi.org/core/hasProperty> ;
                                                                    owl:hasValue <https://saref.etsi.org/saref4bldg/powerOutputMax>
                                                                  ] ,
                                                                  [ rdf:type owl:Restriction ;
                                                                    owl:onProperty <https://saref.etsi.org/core/hasProperty> ;
                                                                    owl:hasValue <https://saref.etsi.org/saref4bldg/startCurrentFactor>
                                                                  ] ,
                                                                  [ rdf:type owl:Restriction ;
                                                                    owl:onProperty <https://saref.etsi.org/core/hasProperty> ;
                                                                    owl:hasValue <https://saref.etsi.org/saref4bldg/startingTime>
                                                                  ] ,
                                                                  [ rdf:type owl:Restriction ;
                                                                    owl:onProperty <https://saref.etsi.org/core/hasProperty> ;
                                                                    owl:hasValue <https://saref.etsi.org/saref4bldg/teTime>
                                                                  ] ;
                                                  <http://purl.org/dc/terms/source> <https://standards.buildingsmart.org/IFC/RELEASE/IFC4_1/FINAL/HTML/schema/ifcelectricaldomain/lexical/ifcelectricmotor.htm> ,
                                                                                    <https://standards.buildingsmart.org/IFC/RELEASE/IFC4_1/FINAL/HTML/schema/ifcelectricaldomain/pset/pset_electricmotortypecommon.htm> ;
                                                  rdfs:comment "An electric motor is an engine that is a machine for converting electrical energy into mechanical energy."@en ;
                                                  rdfs:label "Electric motor"@en ;
                                                  rdfs:seeAlso "https://w3id.org/ifc/IFC4_ADD1#IfcElectricMotor" .


###  https://saref.etsi.org/saref4bldg/ElectricTimeControl
<https://saref.etsi.org/saref4bldg/ElectricTimeControl> rdf:type owl:Class ;
                                                        rdfs:subClassOf <https://saref.etsi.org/saref4bldg/FlowController> ;
                                                        <http://purl.org/dc/terms/source> <https://standards.buildingsmart.org/IFC/RELEASE/IFC4_1/FINAL/HTML/schema/ifcelectricaldomain/lexical/ifcelectrictimecontrol.htm> ,
                                                                                          <https://standards.buildingsmart.org/IFC/RELEASE/IFC4_1/FINAL/HTML/schema/ifcelectricaldomain/pset/pset_electrictimecontroltypecommon.htm> ;
                                                        rdfs:comment "An electric time control is a device that applies control to the provision or flow of electrical energy over time."@en ;
                                                        rdfs:label "Electric time control"@en ;
                                                        rdfs:seeAlso "https://w3id.org/ifc/IFC4_ADD1#IfcElectricTimeControl" .


###  https://saref.etsi.org/saref4bldg/EnergyConversionDevice
<https://saref.etsi.org/saref4bldg/EnergyConversionDevice> rdf:type owl:Class ;
                                                           rdfs:subClassOf <https://saref.etsi.org/saref4bldg/DistributionFlowDevice> ;
                                                           <http://purl.org/dc/terms/source> <https://standards.buildingsmart.org/IFC/RELEASE/IFC4_1/FINAL/HTML/schema/ifcsharedbldgserviceelements/lexical/ifcenergyconversiondevice.htm> ;
                                                           rdfs:comment "The distribution flow element EnergyConversionDevice defines the occurrence of a device used to perform energy conversion or heat transfer and typically participates in a flow distribution system."@en ;
                                                           rdfs:label "Energy conversion device"@en ;
                                                           rdfs:seeAlso "https://w3id.org/ifc/IFC4_ADD1#IfcEnergyConversionDevice" .


###  https://saref.etsi.org/saref4bldg/Engine
<https://saref.etsi.org/saref4bldg/Engine> rdf:type owl:Class ;
                                           rdfs:subClassOf <https://saref.etsi.org/saref4bldg/EnergyConversionDevice> ;
                                           <http://purl.org/dc/terms/source> <https://standards.buildingsmart.org/IFC/RELEASE/IFC4_1/FINAL/HTML/schema/ifchvacdomain/lexical/ifcengine.htm> ,
                                                                             <https://standards.buildingsmart.org/IFC/RELEASE/IFC4_1/FINAL/HTML/schema/ifchvacdomain/pset/pset_enginetypecommon.htm> ;
                                           rdfs:comment "An engine is a device that converts fuel into mechanical energy through combustion."@en ;
                                           rdfs:label "Engine"@en ;
                                           rdfs:seeAlso "https://w3id.org/ifc/IFC4_ADD1#IfcEngine" .


###  https://saref.etsi.org/saref4bldg/EvaporativeCooler
<https://saref.etsi.org/saref4bldg/EvaporativeCooler> rdf:type owl:Class ;
                                                      rdfs:subClassOf <https://saref.etsi.org/saref4bldg/EnergyConversionDevice> ,
                                                                      [ rdf:type owl:Restriction ;
                                                                        owl:onProperty <https://saref.etsi.org/core/hasProperty> ;
                                                                        owl:hasValue <https://saref.etsi.org/saref4bldg/heatExchangeArea>
                                                                      ] ,
                                                                      [ rdf:type owl:Restriction ;
                                                                        owl:onProperty <https://saref.etsi.org/core/hasProperty> ;
                                                                        owl:hasValue <https://saref.etsi.org/saref4bldg/operationTemperatureMax>
                                                                      ] ,
                                                                      [ rdf:type owl:Restriction ;
                                                                        owl:onProperty <https://saref.etsi.org/core/hasProperty> ;
                                                                        owl:hasValue <https://saref.etsi.org/saref4bldg/operationTemperatureMin>
                                                                      ] ,
                                                                      [ rdf:type owl:Restriction ;
                                                                        owl:onProperty <https://saref.etsi.org/core/hasProperty> ;
                                                                        owl:hasValue <https://saref.etsi.org/saref4bldg/waterRequirement>
                                                                      ] ;
                                                      <http://purl.org/dc/terms/source> <https://standards.buildingsmart.org/IFC/RELEASE/IFC4_1/FINAL/HTML/schema/ifchvacdomain/lexical/ifcevaporativecooler.htm> ,
                                                                                        <https://standards.buildingsmart.org/IFC/RELEASE/IFC4_1/FINAL/HTML/schema/ifchvacdomain/pset/pset_evaporativecoolertypecommon.htm> ;
                                                      rdfs:comment "An evaporative cooler is a device that cools air by saturating it with water vapor."@en ;
                                                      rdfs:label "Evaporative cooler"@en ;
                                                      rdfs:seeAlso "https://w3id.org/ifc/IFC4_ADD1#IfcEvaporativeCooler" .


###  https://saref.etsi.org/saref4bldg/Evaporator
<https://saref.etsi.org/saref4bldg/Evaporator> rdf:type owl:Class ;
                                               rdfs:subClassOf <https://saref.etsi.org/saref4bldg/EnergyConversionDevice> ,
                                                               [ rdf:type owl:Restriction ;
                                                                 owl:onProperty <https://saref.etsi.org/core/hasProperty> ;
                                                                 owl:hasValue <https://saref.etsi.org/saref4bldg/externalSurfaceArea>
                                                               ] ,
                                                               [ rdf:type owl:Restriction ;
                                                                 owl:onProperty <https://saref.etsi.org/core/hasProperty> ;
                                                                 owl:hasValue <https://saref.etsi.org/saref4bldg/internalRefrigerantVolume>
                                                               ] ,
                                                               [ rdf:type owl:Restriction ;
                                                                 owl:onProperty <https://saref.etsi.org/core/hasProperty> ;
                                                                 owl:hasValue <https://saref.etsi.org/saref4bldg/internalSurfaceArea>
                                                               ] ,
                                                               [ rdf:type owl:Restriction ;
                                                                 owl:onProperty <https://saref.etsi.org/core/hasProperty> ;
                                                                 owl:hasValue <https://saref.etsi.org/saref4bldg/internalWaterVolume>
                                                               ] ,
                                                               [ rdf:type owl:Restriction ;
                                                                 owl:onProperty <https://saref.etsi.org/core/hasProperty> ;
                                                                 owl:hasValue <https://saref.etsi.org/saref4bldg/nominalHeatTransferArea>
                                                               ] ,
                                                               [ rdf:type owl:Restriction ;
                                                                 owl:onProperty <https://saref.etsi.org/core/hasProperty> ;
                                                                 owl:hasValue <https://saref.etsi.org/saref4bldg/nominalHeatTransferCoefficient>
                                                               ] ;
                                               <http://purl.org/dc/terms/source> <https://standards.buildingsmart.org/IFC/RELEASE/IFC4_1/FINAL/HTML/schema/ifchvacdomain/lexical/ifcevaporator.htm> ,
                                                                                 <https://standards.buildingsmart.org/IFC/RELEASE/IFC4_1/FINAL/HTML/schema/ifchvacdomain/pset/pset_evaporatortypecommon.htm> ;
                                               rdfs:comment "An evaporator is a device in which a liquid refrigerent is vaporized and absorbs heat from the surrounding fluid."@en ;
                                               rdfs:label "Evaporator"@en ;
                                               rdfs:seeAlso "https://w3id.org/ifc/IFC4_ADD1#IfcEvaporator" .


###  https://saref.etsi.org/saref4bldg/Fan
<https://saref.etsi.org/saref4bldg/Fan> rdf:type owl:Class ;
                                        rdfs:subClassOf <https://saref.etsi.org/saref4bldg/FlowMovingDevice> ,
                                                        [ rdf:type owl:Restriction ;
                                                          owl:onProperty <https://saref.etsi.org/core/hasProperty> ;
                                                          owl:hasValue <https://saref.etsi.org/saref4bldg/nominalAirFlowRate>
                                                        ] ,
                                                        [ rdf:type owl:Restriction ;
                                                          owl:onProperty <https://saref.etsi.org/core/hasProperty> ;
                                                          owl:hasValue <https://saref.etsi.org/saref4bldg/nominalPowerRate>
                                                        ] ,
                                                        [ rdf:type owl:Restriction ;
                                                          owl:onProperty <https://saref.etsi.org/core/hasProperty> ;
                                                          owl:hasValue <https://saref.etsi.org/saref4bldg/nominalRotationSpeed>
                                                        ] ,
                                                        [ rdf:type owl:Restriction ;
                                                          owl:onProperty <https://saref.etsi.org/core/hasProperty> ;
                                                          owl:hasValue <https://saref.etsi.org/saref4bldg/nominalStaticPressure>
                                                        ] ,
                                                        [ rdf:type owl:Restriction ;
                                                          owl:onProperty <https://saref.etsi.org/core/hasProperty> ;
                                                          owl:hasValue <https://saref.etsi.org/saref4bldg/nominalTotalPressure>
                                                        ] ,
                                                        [ rdf:type owl:Restriction ;
                                                          owl:onProperty <https://saref.etsi.org/core/hasProperty> ;
                                                          owl:hasValue <https://saref.etsi.org/saref4bldg/operationTemperatureMax>
                                                        ] ,
                                                        [ rdf:type owl:Restriction ;
                                                          owl:onProperty <https://saref.etsi.org/core/hasProperty> ;
                                                          owl:hasValue <https://saref.etsi.org/saref4bldg/operationTemperatureMin>
                                                        ] ,
                                                        [ rdf:type owl:Restriction ;
                                                          owl:onProperty <https://saref.etsi.org/core/hasProperty> ;
                                                          owl:hasValue <https://saref.etsi.org/saref4bldg/operationalRiterial>
                                                        ] ;
                                        <http://purl.org/dc/terms/source> <https://standards.buildingsmart.org/IFC/RELEASE/IFC4_1/FINAL/HTML/schema/ifchvacdomain/lexical/ifcfan.htm> ,
                                                                          <https://standards.buildingsmart.org/IFC/RELEASE/IFC4_1/FINAL/HTML/schema/ifchvacdomain/pset/pset_fantypecommon.htm> ;
                                        rdfs:comment "A fan is a device which imparts mechanical work on a gas. A typical usage of a fan is to induce airflow in a building services air distribution system."@en ;
                                        rdfs:label "Fan"@en ;
                                        rdfs:seeAlso "https://w3id.org/ifc/IFC4_ADD1#IfcFan" .


###  https://saref.etsi.org/saref4bldg/Filter
<https://saref.etsi.org/saref4bldg/Filter> rdf:type owl:Class ;
                                           rdfs:subClassOf <https://saref.etsi.org/saref4bldg/FlowTreatmentDevice> ,
                                                           [ rdf:type owl:Restriction ;
                                                             owl:onProperty <https://saref.etsi.org/core/hasProperty> ;
                                                             owl:hasValue <https://saref.etsi.org/saref4bldg/finalResistance>
                                                           ] ,
                                                           [ rdf:type owl:Restriction ;
                                                             owl:onProperty <https://saref.etsi.org/core/hasProperty> ;
                                                             owl:hasValue <https://saref.etsi.org/saref4bldg/fluidFlowRateMax>
                                                           ] ,
                                                           [ rdf:type owl:Restriction ;
                                                             owl:onProperty <https://saref.etsi.org/core/hasProperty> ;
                                                             owl:hasValue <https://saref.etsi.org/saref4bldg/fluidFlowRateMin>
                                                           ] ,
                                                           [ rdf:type owl:Restriction ;
                                                             owl:onProperty <https://saref.etsi.org/core/hasProperty> ;
                                                             owl:hasValue <https://saref.etsi.org/saref4bldg/initialResistance>
                                                           ] ,
                                                           [ rdf:type owl:Restriction ;
                                                             owl:onProperty <https://saref.etsi.org/core/hasProperty> ;
                                                             owl:hasValue <https://saref.etsi.org/saref4bldg/nominalFilterFaceVelocity>
                                                           ] ,
                                                           [ rdf:type owl:Restriction ;
                                                             owl:onProperty <https://saref.etsi.org/core/hasProperty> ;
                                                             owl:hasValue <https://saref.etsi.org/saref4bldg/nominalFlowRate>
                                                           ] ,
                                                           [ rdf:type owl:Restriction ;
                                                             owl:onProperty <https://saref.etsi.org/core/hasProperty> ;
                                                             owl:hasValue <https://saref.etsi.org/saref4bldg/nominalMediaSurfaceVelocity>
                                                           ] ,
                                                           [ rdf:type owl:Restriction ;
                                                             owl:onProperty <https://saref.etsi.org/core/hasProperty> ;
                                                             owl:hasValue <https://saref.etsi.org/saref4bldg/nominalParticleGeometricMeanDiameter>
                                                           ] ,
                                                           [ rdf:type owl:Restriction ;
                                                             owl:onProperty <https://saref.etsi.org/core/hasProperty> ;
                                                             owl:hasValue <https://saref.etsi.org/saref4bldg/nominalParticleGeometricStandardDeviation>
                                                           ] ,
                                                           [ rdf:type owl:Restriction ;
                                                             owl:onProperty <https://saref.etsi.org/core/hasProperty> ;
                                                             owl:hasValue <https://saref.etsi.org/saref4bldg/nominalPressureDrop>
                                                           ] ,
                                                           [ rdf:type owl:Restriction ;
                                                             owl:onProperty <https://saref.etsi.org/core/hasProperty> ;
                                                             owl:hasValue <https://saref.etsi.org/saref4bldg/operationTemperatureMax>
                                                           ] ,
                                                           [ rdf:type owl:Restriction ;
                                                             owl:onProperty <https://saref.etsi.org/core/hasProperty> ;
                                                             owl:hasValue <https://saref.etsi.org/saref4bldg/operationTemperatureMin>
                                                           ] ,
                                                           [ rdf:type owl:Restriction ;
                                                             owl:onProperty <https://saref.etsi.org/core/hasProperty> ;
                                                             owl:hasValue <https://saref.etsi.org/saref4bldg/weight>
                                                           ] ;
                                           <http://purl.org/dc/terms/source> <https://standards.buildingsmart.org/IFC/RELEASE/IFC4_1/FINAL/HTML/schema/ifchvacdomain/lexical/ifcfilter.htm> ,
                                                                             <https://standards.buildingsmart.org/IFC/RELEASE/IFC4_1/FINAL/HTML/schema/ifchvacdomain/pset/pset_filtertypecommon.htm> ;
                                           rdfs:comment "A filter is an apparatus used to remove particulate or gaseous matter from fluids and gases."@en ;
                                           rdfs:label "Filter"@en ;
                                           rdfs:seeAlso "https://w3id.org/ifc/IFC4_ADD1#IfcFilter" .


###  https://saref.etsi.org/saref4bldg/FireSuppressionTerminal
<https://saref.etsi.org/saref4bldg/FireSuppressionTerminal> rdf:type owl:Class ;
                                                            rdfs:subClassOf <https://saref.etsi.org/saref4bldg/FlowTerminal> ;
                                                            <http://purl.org/dc/terms/source> <https://standards.buildingsmart.org/IFC/RELEASE/IFC4_1/FINAL/HTML/schema/ifcplumbingfireprotectiondomain/lexical/ifcfiresuppressionterminal.htm> ,
                                                                                              <https://standards.buildingsmart.org/IFC/RELEASE/IFC4_1/FINAL/HTML/schema/ifcplumbingfireprotectiondomain/pset/pset_firesuppressionterminaltypecommon.htm> ;
                                                            rdfs:comment """A fire suppression terminal has the purpose of delivering a fluid (gas or liquid) that will suppress a fire.

A fire suppression terminal provides for all forms of sprinkler, spreader and other form of terminal that is connected to a pipework system and intended to act in the role of suppressing a fire."""@en ;
                                                            rdfs:label "Fire suppression terminal"@en ;
                                                            rdfs:seeAlso "https://w3id.org/ifc/IFC4_ADD1#IfcFireSuppressionTerminal" .


###  https://saref.etsi.org/saref4bldg/FlowController
<https://saref.etsi.org/saref4bldg/FlowController> rdf:type owl:Class ;
                                                   rdfs:subClassOf <https://saref.etsi.org/saref4bldg/DistributionFlowDevice> ;
                                                   <http://purl.org/dc/terms/source> <https://standards.buildingsmart.org/IFC/RELEASE/IFC4_1/FINAL/HTML/schema/ifcsharedbldgserviceelements/lexical/ifcflowcontroller.htm> ;
                                                   rdfs:comment "The distribution flow element FlowController defines the occurrence of elements of a distribution system that are used to regulate flow through a distribution system. Examples include dampers, valves, switches, and relays."@en ;
                                                   rdfs:label "Flow controller"@en ;
                                                   rdfs:seeAlso "https://w3id.org/ifc/IFC4_ADD1#IfcFlowController" .


###  https://saref.etsi.org/saref4bldg/FlowInstrument
<https://saref.etsi.org/saref4bldg/FlowInstrument> rdf:type owl:Class ;
                                                   rdfs:subClassOf <https://saref.etsi.org/saref4bldg/DistributionControlDevice> ;
                                                   <http://purl.org/dc/terms/source> <https://standards.buildingsmart.org/IFC/RELEASE/IFC4_1/FINAL/HTML/schema/ifcbuildingcontrolsdomain/lexical/ifcflowinstrument.htm> ,
                                                                                     <https://standards.buildingsmart.org/IFC/RELEASE/IFC4_1/FINAL/HTML/schema/ifcbuildingcontrolsdomain/pset/pset_flowinstrumenttypecommon.htm> ;
                                                   rdfs:comment """A flow instrument reads and displays the value of a particular property of a system at a point, or displays the difference in the value of a property between two points.

Instrumentation is typically for the purpose of determining the value of the property at a point in time. It is not the purpose of an instrument to record or integrate the values over time (although they may be connected to recording devices that do perform such a function). This entity provides for all forms of mechanical flow instrument (thermometers, pressure gauges etc.) and electrical flow instruments (ammeters, voltmeters etc.)"""@en ;
                                                   rdfs:label "Flow instrument"@en ;
                                                   rdfs:seeAlso "https://w3id.org/ifc/IFC4_ADD1#IfcFlowInstrument" .


###  https://saref.etsi.org/saref4bldg/FlowMeter
<https://saref.etsi.org/saref4bldg/FlowMeter> rdf:type owl:Class ;
                                              rdfs:subClassOf <https://saref.etsi.org/saref4bldg/FlowController> ;
                                              <http://purl.org/dc/terms/source> <https://standards.buildingsmart.org/IFC/RELEASE/IFC4_1/FINAL/HTML/schema/ifchvacdomain/lexical/ifcflowmeter.htm> ,
                                                                                <https://standards.buildingsmart.org/IFC/RELEASE/IFC4_1/FINAL/HTML/schema/ifchvacdomain/pset/pset_flowmetertypecommon.htm> ;
                                              rdfs:comment "A flow meter is a device that is used to measure the flow rate in a system."@en ;
                                              rdfs:label "Flow meter"@en ;
                                              rdfs:seeAlso "https://w3id.org/ifc/IFC4_ADD1#IfcFlowMeter" .


###  https://saref.etsi.org/saref4bldg/FlowMovingDevice
<https://saref.etsi.org/saref4bldg/FlowMovingDevice> rdf:type owl:Class ;
                                                     rdfs:subClassOf <https://saref.etsi.org/saref4bldg/DistributionFlowDevice> ;
                                                     <http://purl.org/dc/terms/source> <https://standards.buildingsmart.org/IFC/RELEASE/IFC4_1/FINAL/HTML/schema/ifcsharedbldgserviceelements/lexical/ifcflowmovingdevice.htm> ;
                                                     rdfs:comment "The distribution flow element FlowMovingDevice defines the occurrence of an apparatus used to distribute, circulate or perform conveyance of fluids, including liquids and gases (such as a pump or fan), and typically participates in a flow distribution system."@en ;
                                                     rdfs:label "Flow moving device"@en ;
                                                     rdfs:seeAlso "https://w3id.org/ifc/IFC4_ADD1#IfcFlowMovingDevice" .


###  https://saref.etsi.org/saref4bldg/FlowStorageDevice
<https://saref.etsi.org/saref4bldg/FlowStorageDevice> rdf:type owl:Class ;
                                                      rdfs:subClassOf <https://saref.etsi.org/saref4bldg/DistributionFlowDevice> ;
                                                      <http://purl.org/dc/terms/source> <https://standards.buildingsmart.org/IFC/RELEASE/IFC4_1/FINAL/HTML/schema/ifcsharedbldgserviceelements/lexical/ifcflowstoragedevice.htm> ;
                                                      rdfs:comment "The distribution flow element FlowStorageDevice defines the occurrence of a device that participates in a distribution system and is used for temporary storage (such as a tank)."@en ;
                                                      rdfs:label "Flow storage device"@en ;
                                                      rdfs:seeAlso "https://w3id.org/ifc/IFC4_ADD1#IfcFlowStorageDevice" .


###  https://saref.etsi.org/saref4bldg/FlowTerminal
<https://saref.etsi.org/saref4bldg/FlowTerminal> rdf:type owl:Class ;
                                                 rdfs:subClassOf <https://saref.etsi.org/saref4bldg/DistributionFlowDevice> ;
                                                 <http://purl.org/dc/terms/source> <https://standards.buildingsmart.org/IFC/RELEASE/IFC4_1/FINAL/HTML/schema/ifcsharedbldgserviceelements/lexical/ifcflowterminal.htm> ;
                                                 rdfs:comment "The distribution flow element FlowTerminal defines the occurrence of a permanently attached element that acts as a terminus or beginning of a distribution system (such as an air outlet, drain, water closet, or sink). A terminal is typically a point at which a system interfaces with an external environment."@en ;
                                                 rdfs:label "Flow terminal"@en ;
                                                 rdfs:seeAlso "https://w3id.org/ifc/IFC4_ADD1#IfcFlowTerminal" .


###  https://saref.etsi.org/saref4bldg/FlowTreatmentDevice
<https://saref.etsi.org/saref4bldg/FlowTreatmentDevice> rdf:type owl:Class ;
                                                        rdfs:subClassOf <https://saref.etsi.org/saref4bldg/DistributionFlowDevice> ;
                                                        <http://purl.org/dc/terms/source> <https://standards.buildingsmart.org/IFC/RELEASE/IFC4_1/FINAL/HTML/schema/ifcsharedbldgserviceelements/lexical/ifcflowtreatmentdevice.htm> ;
                                                        rdfs:comment "The distribution flow element FlowTreatmentDevice defines the occurrence of a device typically used to remove unwanted matter from a fluid, either liquid or gas, and typically participates in a flow distribution system."@en ;
                                                        rdfs:label "Flow treatment device"@en ;
                                                        rdfs:seeAlso "https://w3id.org/ifc/IFC4_ADD1#IfcFlowTreatmentDevice" .


###  https://saref.etsi.org/saref4bldg/HeatExchanger
<https://saref.etsi.org/saref4bldg/HeatExchanger> rdf:type owl:Class ;
                                                  rdfs:subClassOf <https://saref.etsi.org/saref4bldg/EnergyConversionDevice> ;
                                                  <http://purl.org/dc/terms/source> <https://standards.buildingsmart.org/IFC/RELEASE/IFC4_1/FINAL/HTML/schema/ifchvacdomain/lexical/ifcheatexchanger.htm> ,
                                                                                    <https://standards.buildingsmart.org/IFC/RELEASE/IFC4_1/FINAL/HTML/schema/ifchvacdomain/pset/pset_heatexchangertypecommon.htm> ;
                                                  rdfs:comment "A heat exchanger is a device used to provide heat transfer between non-mixing media such as plate and shell and tube heat exchangers. HeatExchanger is commonly used on water-side distribution systems to recover energy from a liquid to another liquid (typically water-based), whereas AirToAirHeatRecovery is commonly used on air-side distribution systems to recover energy from a gas to a gas (usually air)."@en ;
                                                  rdfs:label "Heat exchanger"@en ;
                                                  rdfs:seeAlso "https://w3id.org/ifc/IFC4_ADD1#IfcHeatExchanger" .


###  https://saref.etsi.org/saref4bldg/Humidifier
<https://saref.etsi.org/saref4bldg/Humidifier> rdf:type owl:Class ;
                                               rdfs:subClassOf <https://saref.etsi.org/saref4bldg/EnergyConversionDevice> ,
                                                               [ rdf:type owl:Restriction ;
                                                                 owl:onProperty <https://saref.etsi.org/core/hasProperty> ;
                                                                 owl:hasValue <https://saref.etsi.org/saref4bldg/nominalAirFlowRate>
                                                               ] ,
                                                               [ rdf:type owl:Restriction ;
                                                                 owl:onProperty <https://saref.etsi.org/core/hasProperty> ;
                                                                 owl:hasValue <https://saref.etsi.org/saref4bldg/nominalMoistureGain>
                                                               ] ,
                                                               [ rdf:type owl:Restriction ;
                                                                 owl:onProperty <https://saref.etsi.org/core/hasProperty> ;
                                                                 owl:hasValue <https://saref.etsi.org/saref4bldg/waterRequirement>
                                                               ] ,
                                                               [ rdf:type owl:Restriction ;
                                                                 owl:onProperty <https://saref.etsi.org/core/hasProperty> ;
                                                                 owl:hasValue <https://saref.etsi.org/saref4bldg/weight>
                                                               ] ;
                                               <http://purl.org/dc/terms/source> <https://standards.buildingsmart.org/IFC/RELEASE/IFC4_1/FINAL/HTML/schema/ifchvacdomain/lexical/ifchumidifier.htm> ,
                                                                                 <https://standards.buildingsmart.org/IFC/RELEASE/IFC4_1/FINAL/HTML/schema/ifchvacdomain/pset/pset_humidifiertypecommon.htm> ;
                                               rdfs:comment "A humidifier is a device that adds moisture into the air."@en ;
                                               rdfs:label "Humidifier"@en ;
                                               rdfs:seeAlso "https://w3id.org/ifc/IFC4_ADD1#IfcHumidifier" .


###  https://saref.etsi.org/saref4bldg/Interceptor
<https://saref.etsi.org/saref4bldg/Interceptor> rdf:type owl:Class ;
                                                rdfs:subClassOf <https://saref.etsi.org/saref4bldg/FlowTreatmentDevice> ,
                                                                [ rdf:type owl:Restriction ;
                                                                  owl:onProperty <https://saref.etsi.org/core/hasProperty> ;
                                                                  owl:hasValue <https://saref.etsi.org/saref4bldg/coverLength>
                                                                ] ,
                                                                [ rdf:type owl:Restriction ;
                                                                  owl:onProperty <https://saref.etsi.org/core/hasProperty> ;
                                                                  owl:hasValue <https://saref.etsi.org/saref4bldg/coverWidth>
                                                                ] ,
                                                                [ rdf:type owl:Restriction ;
                                                                  owl:onProperty <https://saref.etsi.org/core/hasProperty> ;
                                                                  owl:hasValue <https://saref.etsi.org/saref4bldg/inletConnectionSize>
                                                                ] ,
                                                                [ rdf:type owl:Restriction ;
                                                                  owl:onProperty <https://saref.etsi.org/core/hasProperty> ;
                                                                  owl:hasValue <https://saref.etsi.org/saref4bldg/nominalBodyDepth>
                                                                ] ,
                                                                [ rdf:type owl:Restriction ;
                                                                  owl:onProperty <https://saref.etsi.org/core/hasProperty> ;
                                                                  owl:hasValue <https://saref.etsi.org/saref4bldg/nominalBodyLength>
                                                                ] ,
                                                                [ rdf:type owl:Restriction ;
                                                                  owl:onProperty <https://saref.etsi.org/core/hasProperty> ;
                                                                  owl:hasValue <https://saref.etsi.org/saref4bldg/nominalBodyWidth>
                                                                ] ,
                                                                [ rdf:type owl:Restriction ;
                                                                  owl:onProperty <https://saref.etsi.org/core/hasProperty> ;
                                                                  owl:hasValue <https://saref.etsi.org/saref4bldg/outletConnectionSize>
                                                                ] ,
                                                                [ rdf:type owl:Restriction ;
                                                                  owl:onProperty <https://saref.etsi.org/core/hasProperty> ;
                                                                  owl:hasValue <https://saref.etsi.org/saref4bldg/ventilatingPipeSize>
                                                                ] ;
                                                <http://purl.org/dc/terms/source> <https://standards.buildingsmart.org/IFC/RELEASE/IFC4_1/FINAL/HTML/schema/ifcplumbingfireprotectiondomain/lexical/ifcinterceptor.htm> ,
                                                                                  <https://standards.buildingsmart.org/IFC/RELEASE/IFC4_1/FINAL/HTML/schema/ifcplumbingfireprotectiondomain/pset/pset_interceptortypecommon.htm> ;
                                                rdfs:comment "An interceptor is a device designed and installed in order to separate and retain deleterious, hazardous or undesirable matter while permitting normal sewage or liquids to discharge into a collection system by gravity."@en ;
                                                rdfs:label "Interceptor"@en ;
                                                rdfs:seeAlso "https://w3id.org/ifc/IFC4_ADD1#IfcInterceptor" .


###  https://saref.etsi.org/saref4bldg/Lamp
<https://saref.etsi.org/saref4bldg/Lamp> rdf:type owl:Class ;
                                         rdfs:subClassOf <https://saref.etsi.org/saref4bldg/FlowTerminal> ,
                                                         [ rdf:type owl:Restriction ;
                                                           owl:onProperty <https://saref.etsi.org/core/hasProperty> ;
                                                           owl:hasValue <https://saref.etsi.org/saref4bldg/colorTemperature>
                                                         ] ,
                                                         [ rdf:type owl:Restriction ;
                                                           owl:onProperty <https://saref.etsi.org/core/hasProperty> ;
                                                           owl:hasValue <https://saref.etsi.org/saref4bldg/contributedLuminousFlux>
                                                         ] ,
                                                         [ rdf:type owl:Restriction ;
                                                           owl:onProperty <https://saref.etsi.org/core/hasProperty> ;
                                                           owl:hasValue <https://saref.etsi.org/saref4bldg/lampMaintenanceFactor>
                                                         ] ,
                                                         [ rdf:type owl:Restriction ;
                                                           owl:onProperty <https://saref.etsi.org/core/hasProperty> ;
                                                           owl:hasValue <https://saref.etsi.org/saref4bldg/lightEmitterNominalPower>
                                                         ] ,
                                                         [ rdf:type owl:Restriction ;
                                                           owl:onProperty <https://saref.etsi.org/core/hasProperty> ;
                                                           owl:hasValue <https://saref.etsi.org/saref4bldg/spectrumMax>
                                                         ] ,
                                                         [ rdf:type owl:Restriction ;
                                                           owl:onProperty <https://saref.etsi.org/core/hasProperty> ;
                                                           owl:hasValue <https://saref.etsi.org/saref4bldg/spectrumMin>
                                                         ] ;
                                         <http://purl.org/dc/terms/source> <https://standards.buildingsmart.org/IFC/RELEASE/IFC4_1/FINAL/HTML/schema/ifcelectricaldomain/lexical/ifclamp.htm> ,
                                                                           <https://standards.buildingsmart.org/IFC/RELEASE/IFC4_1/FINAL/HTML/schema/ifcelectricaldomain/pset/pset_lamptypecommon.htm> ;
                                         rdfs:comment "A lamp is an artificial light source such as a light bulb or tube."@en ;
                                         rdfs:label "Lamp"@en ;
                                         rdfs:seeAlso "https://w3id.org/ifc/IFC4_ADD1#IfcLamp" .


###  https://saref.etsi.org/saref4bldg/MedicalDevice
<https://saref.etsi.org/saref4bldg/MedicalDevice> rdf:type owl:Class ;
                                                  rdfs:subClassOf <https://saref.etsi.org/saref4bldg/FlowTerminal> ;
                                                  <http://purl.org/dc/terms/source> <https://standards.buildingsmart.org/IFC/RELEASE/IFC4_1/FINAL/HTML/schema/ifchvacdomain/lexical/ifcmedicaldevice.htm> ,
                                                                                    <https://standards.buildingsmart.org/IFC/RELEASE/IFC4_1/FINAL/HTML/schema/ifchvacdomain/pset/pset_medicaldevicetypecommon.htm> ;
                                                  rdfs:comment "A medical device is attached to a medical piping system and operates upon medical gases to perform a specific function. Medical gases include medical air, medical vacuum, oxygen, carbon dioxide, nitrogen, and nitrous oxide."@en ;
                                                  rdfs:label "Medical device"@en ;
                                                  rdfs:seeAlso "https://w3id.org/ifc/IFC4_ADD1#IfcMedicalDevice" .


###  https://saref.etsi.org/saref4bldg/Outlet
<https://saref.etsi.org/saref4bldg/Outlet> rdf:type owl:Class ;
                                           rdfs:subClassOf <https://saref.etsi.org/saref4bldg/FlowTerminal> ;
                                           <http://purl.org/dc/terms/source> <https://standards.buildingsmart.org/IFC/RELEASE/IFC4_1/FINAL/HTML/schema/ifcelectricaldomain/lexical/ifcoutlet.htm> ,
                                                                             <https://standards.buildingsmart.org/IFC/RELEASE/IFC4_1/FINAL/HTML/schema/ifcelectricaldomain/pset/pset_outlettypecommon.htm> ;
                                           rdfs:comment """An outlet is a device installed at a point to receive one or more inserted plugs for electrical power or communications.

Power outlets are commonly connected within a junction box; data outlets may be directly connected to a wall. For power outlets sharing the same circuit within a junction box, the ports should indicate the logical wiring relationship to the enclosing junction box, even though they may be physically connected to a cable going to another outlet, switch, or fixture."""@en ;
                                           rdfs:label "Outlet"@en ;
                                           rdfs:seeAlso "https://w3id.org/ifc/IFC4_ADD1#IfcOutlet" .


###  https://saref.etsi.org/saref4bldg/PhysicalObject
<https://saref.etsi.org/saref4bldg/PhysicalObject> rdf:type owl:Class ;
                                                   rdfs:subClassOf <http://www.opengis.net/ont/geosparql#SpatialThing> ,
                                                                   [ rdf:type owl:Restriction ;
                                                                     owl:onProperty <https://saref.etsi.org/saref4bldg/contains> ;
                                                                     owl:allValuesFrom <https://saref.etsi.org/saref4bldg/PhysicalObject>
                                                                   ] ,
                                                                   [ rdf:type owl:Restriction ;
                                                                     owl:onProperty <https://saref.etsi.org/saref4bldg/isContainedIn> ;
                                                                     owl:allValuesFrom [ rdf:type owl:Class ;
                                                                                         owl:unionOf ( <https://saref.etsi.org/saref4bldg/BuildingSpace>
                                                                                                       <https://saref.etsi.org/saref4bldg/PhysicalObject>
                                                                                                     )
                                                                                       ]
                                                                   ] ;
                                                   rdfs:comment "Any Object that has a proper space region.  (Definition extracted from DUL ontology)"@en ;
                                                   rdfs:label "Physical object"@en .


###  https://saref.etsi.org/saref4bldg/ProtectiveDevice
<https://saref.etsi.org/saref4bldg/ProtectiveDevice> rdf:type owl:Class ;
                                                     rdfs:subClassOf <https://saref.etsi.org/saref4bldg/FlowController> ;
                                                     <http://purl.org/dc/terms/source> <https://standards.buildingsmart.org/IFC/RELEASE/IFC4_1/FINAL/HTML/schema/ifcelectricaldomain/lexical/ifcprotectivedevice.htm> ,
                                                                                       <https://standards.buildingsmart.org/IFC/RELEASE/IFC4_1/FINAL/HTML/schema/ifcelectricaldomain/pset/pset_protectivedevicetypecommon.htm> ;
                                                     rdfs:comment """A protective device breaks an electrical circuit when a stated electric current that passes through it is exceeded.

A protective device provides protection against electrical current only (not as a general protective device). It may be used to represent the complete set of elements including both the tripping unit and the breaking unit that provide the protection. This may be particularly useful at earlier stages of design where the approach to breaking the electrical supply may be determined but the method of tripping may not. Alternatively, this entity may be used to specifically represent the breaking unit alone (in which case the tripping unit will also be specifically identified). This entity is specific to dedicated protective devices and excludes electrical outlets that may have circuit protection."""@en ;
                                                     rdfs:label "Protective device"@en ;
                                                     rdfs:seeAlso "https://w3id.org/ifc/IFC4_ADD1#IfcProtectiveDevice" .


###  https://saref.etsi.org/saref4bldg/ProtectiveDeviceTrippingUnit
<https://saref.etsi.org/saref4bldg/ProtectiveDeviceTrippingUnit> rdf:type owl:Class ;
                                                                 rdfs:subClassOf <https://saref.etsi.org/saref4bldg/DistributionControlDevice> ,
                                                                                 [ rdf:type owl:Restriction ;
                                                                                   owl:onProperty <https://saref.etsi.org/core/hasProperty> ;
                                                                                   owl:hasValue <https://saref.etsi.org/saref4bldg/limitingTerminalSize>
                                                                                 ] ;
                                                                 <http://purl.org/dc/terms/source> <https://standards.buildingsmart.org/IFC/RELEASE/IFC4_1/FINAL/HTML/schema/ifcelectricaldomain/lexical/ifcprotectivedevicetrippingunit.htm> ,
                                                                                                   <https://standards.buildingsmart.org/IFC/RELEASE/IFC4_1/FINAL/HTML/schema/ifcelectricaldomain/pset/pset_protectivedevicetrippingunittypecommon.htm> ;
                                                                 rdfs:comment "A protective device tripping unit breaks an electrical circuit at a separate breaking unit when a stated electric current that passes through the unit is exceeded."@en ;
                                                                 rdfs:label "Protective device tripping unit"@en ;
                                                                 rdfs:seeAlso "https://w3id.org/ifc/IFC4_ADD1#IfcProtectiveDeviceTrippingUnit" .


###  https://saref.etsi.org/saref4bldg/Pump
<https://saref.etsi.org/saref4bldg/Pump> rdf:type owl:Class ;
                                         rdfs:subClassOf <https://saref.etsi.org/saref4bldg/FlowMovingDevice> ,
                                                         [ rdf:type owl:Restriction ;
                                                           owl:onProperty <https://saref.etsi.org/core/hasProperty> ;
                                                           owl:hasValue <https://saref.etsi.org/saref4bldg/connectionSize>
                                                         ] ,
                                                         [ rdf:type owl:Restriction ;
                                                           owl:onProperty <https://saref.etsi.org/core/hasProperty> ;
                                                           owl:hasValue <https://saref.etsi.org/saref4bldg/flowResistanceMax>
                                                         ] ,
                                                         [ rdf:type owl:Restriction ;
                                                           owl:onProperty <https://saref.etsi.org/core/hasProperty> ;
                                                           owl:hasValue <https://saref.etsi.org/saref4bldg/flowResistanceMin>
                                                         ] ,
                                                         [ rdf:type owl:Restriction ;
                                                           owl:onProperty <https://saref.etsi.org/core/hasProperty> ;
                                                           owl:hasValue <https://saref.etsi.org/saref4bldg/netPositiveSuctionHead>
                                                         ] ,
                                                         [ rdf:type owl:Restriction ;
                                                           owl:onProperty <https://saref.etsi.org/core/hasProperty> ;
                                                           owl:hasValue <https://saref.etsi.org/saref4bldg/nomminalRotationSpeed>
                                                         ] ,
                                                         [ rdf:type owl:Restriction ;
                                                           owl:onProperty <https://saref.etsi.org/core/hasProperty> ;
                                                           owl:hasValue <https://saref.etsi.org/saref4bldg/operationTemperatureMax>
                                                         ] ,
                                                         [ rdf:type owl:Restriction ;
                                                           owl:onProperty <https://saref.etsi.org/core/hasProperty> ;
                                                           owl:hasValue <https://saref.etsi.org/saref4bldg/operationTemperatureMin>
                                                         ] ,
                                                         [ rdf:type owl:Restriction ;
                                                           owl:onProperty <https://saref.etsi.org/core/hasProperty> ;
                                                           owl:hasValue <https://saref.etsi.org/saref4bldg/pumpFlowRateMax>
                                                         ] ,
                                                         [ rdf:type owl:Restriction ;
                                                           owl:onProperty <https://saref.etsi.org/core/hasProperty> ;
                                                           owl:hasValue <https://saref.etsi.org/saref4bldg/pumpFlowRateMin>
                                                         ] ;
                                         <http://purl.org/dc/terms/source> <https://standards.buildingsmart.org/IFC/RELEASE/IFC4_1/FINAL/HTML/schema/ifchvacdomain/lexical/ifcpump.htm> ,
                                                                           <https://standards.buildingsmart.org/IFC/RELEASE/IFC4_1/FINAL/HTML/schema/ifchvacdomain/pset/pset_pumptypecommon.htm> ;
                                         rdfs:comment "A pump is a device which imparts mechanical work on fluids or slurries to move them through a channel or pipeline. A typical use of a pump is to circulate chilled water or heating hot water in a building services distribution system."@en ;
                                         rdfs:label "Pump"@en ;
                                         rdfs:seeAlso "https://w3id.org/ifc/IFC4_ADD1#IfcPump" .


###  https://saref.etsi.org/saref4bldg/SanitaryTerminal
<https://saref.etsi.org/saref4bldg/SanitaryTerminal> rdf:type owl:Class ;
                                                     rdfs:subClassOf <https://saref.etsi.org/saref4bldg/FlowTerminal> ;
                                                     <http://purl.org/dc/terms/source> <https://standards.buildingsmart.org/IFC/RELEASE/IFC4_1/FINAL/HTML/schema/ifcplumbingfireprotectiondomain/lexical/ifcsanitaryterminal.htm> ,
                                                                                       <https://standards.buildingsmart.org/IFC/RELEASE/IFC4_1/FINAL/HTML/schema/ifcplumbingfireprotectiondomain/pset/pset_sanitaryterminaltypecommon.htm> ;
                                                     rdfs:comment "A sanitary terminal is a fixed appliance or terminal usually supplied with water and used for drinking, cleaning or foul water disposal or that is an item of equipment directly used with such an appliance or terminal."@en ;
                                                     rdfs:label "Sanitary terminal"@en ;
                                                     rdfs:seeAlso "https://w3id.org/ifc/IFC4_ADD1#IfcSanitaryTerminal" .


###  https://saref.etsi.org/saref4bldg/Sensor
<https://saref.etsi.org/saref4bldg/Sensor> rdf:type owl:Class ;
                                           rdfs:subClassOf <https://saref.etsi.org/core/Sensor> ,
                                                           <https://saref.etsi.org/saref4bldg/DistributionControlDevice> ;
                                           <http://purl.org/dc/terms/source> <https://standards.buildingsmart.org/IFC/RELEASE/IFC4_1/FINAL/HTML/schema/ifcbuildingcontrolsdomain/lexical/ifcsensor.htm> ,
                                                                             <https://standards.buildingsmart.org/IFC/RELEASE/IFC4_1/FINAL/HTML/schema/ifcbuildingcontrolsdomain/pset/pset_sensortypecommon.htm> ;
                                           rdfs:comment "A sensor is a device that measures a physical quantity and converts it into a signal which can be read by an observer or by an instrument."@en ;
                                           rdfs:label "Sensor"@en ;
                                           rdfs:seeAlso "https://w3id.org/ifc/IFC4_ADD1#IfcSensor" .


###  https://saref.etsi.org/saref4bldg/ShadingDevice
<https://saref.etsi.org/saref4bldg/ShadingDevice> rdf:type owl:Class ;
                                                  rdfs:subClassOf <https://saref.etsi.org/saref4bldg/BuildingDevice> ,
                                                                  [ rdf:type owl:Restriction ;
                                                                    owl:onProperty <https://saref.etsi.org/core/hasProperty> ;
                                                                    owl:hasValue <https://saref.etsi.org/saref4bldg/solarReflectance>
                                                                  ] ,
                                                                  [ rdf:type owl:Restriction ;
                                                                    owl:onProperty <https://saref.etsi.org/core/hasProperty> ;
                                                                    owl:hasValue <https://saref.etsi.org/saref4bldg/solarTransmittance>
                                                                  ] ,
                                                                  [ rdf:type owl:Restriction ;
                                                                    owl:onProperty <https://saref.etsi.org/core/hasProperty> ;
                                                                    owl:hasValue <https://saref.etsi.org/saref4bldg/thermalTransmittance>
                                                                  ] ,
                                                                  [ rdf:type owl:Restriction ;
                                                                    owl:onProperty <https://saref.etsi.org/core/hasProperty> ;
                                                                    owl:hasValue <https://saref.etsi.org/saref4bldg/visibleLightReflectance>
                                                                  ] ,
                                                                  [ rdf:type owl:Restriction ;
                                                                    owl:onProperty <https://saref.etsi.org/core/hasProperty> ;
                                                                    owl:hasValue <https://saref.etsi.org/saref4bldg/visibleLightTransmittance>
                                                                  ] ;
                                                  <http://purl.org/dc/terms/source> <https://standards.buildingsmart.org/IFC/RELEASE/IFC4_1/FINAL/HTML/schema/ifcsharedbldgelements/lexical/ifcshadingdevice.htm> ,
                                                                                    <https://standards.buildingsmart.org/IFC/RELEASE/IFC4_1/FINAL/HTML/schema/ifcsharedbldgelements/pset/pset_shadingdevicecommon.htm> ;
                                                  rdfs:comment "Shading devices are purpose built devices to protect from the sunlight, from natural light, or screening them from view. Shading devices can form part of the facade or can be mounted inside the building, they can be fixed or operable."@en ;
                                                  rdfs:label "Shading device"@en ;
                                                  rdfs:seeAlso "https://w3id.org/ifc/IFC4_ADD1#IfcShadingDevice" .


###  https://saref.etsi.org/saref4bldg/SolarDevice
<https://saref.etsi.org/saref4bldg/SolarDevice> rdf:type owl:Class ;
                                                rdfs:subClassOf <https://saref.etsi.org/saref4bldg/EnergyConversionDevice> ;
                                                <http://purl.org/dc/terms/source> <https://standards.buildingsmart.org/IFC/RELEASE/IFC4_1/FINAL/HTML/schema/ifcelectricaldomain/lexical/ifcsolardevicetypeenum.htm> ,
                                                                                  <https://standards.buildingsmart.org/IFC/RELEASE/IFC4_1/FINAL/HTML/schema/ifcelectricaldomain/pset/pset_solardevicetypecommon.htm> ;
                                                rdfs:comment "A solar device converts solar radiation into other energy such as electric current or thermal energy."@en ;
                                                rdfs:label "Solar device"@en ;
                                                rdfs:seeAlso "https://w3id.org/ifc/IFC4_ADD1#IfcSolarDevice" .


###  https://saref.etsi.org/saref4bldg/SpaceHeater
<https://saref.etsi.org/saref4bldg/SpaceHeater> rdf:type owl:Class ;
                                                rdfs:subClassOf <https://saref.etsi.org/saref4bldg/FlowTerminal> ,
                                                                [ rdf:type owl:Restriction ;
                                                                  owl:onProperty <https://saref.etsi.org/core/hasProperty> ;
                                                                  owl:hasValue <https://saref.etsi.org/saref4bldg/bodyMass>
                                                                ] ,
                                                                [ rdf:type owl:Restriction ;
                                                                  owl:onProperty <https://saref.etsi.org/core/hasProperty> ;
                                                                  owl:hasValue <https://saref.etsi.org/saref4bldg/outputCapacity>
                                                                ] ,
                                                                [ rdf:type owl:Restriction ;
                                                                  owl:onProperty <https://saref.etsi.org/core/hasProperty> ;
                                                                  owl:hasValue <https://saref.etsi.org/saref4bldg/thermalEfficiency>
                                                                ] ,
                                                                [ rdf:type owl:Restriction ;
                                                                  owl:onProperty <https://saref.etsi.org/core/hasProperty> ;
                                                                  owl:hasValue <https://saref.etsi.org/saref4bldg/thermalMassHeatCapacity>
                                                                ] ;
                                                <http://purl.org/dc/terms/source> <https://standards.buildingsmart.org/IFC/RELEASE/IFC4_1/FINAL/HTML/schema/ifchvacdomain/lexical/ifcspaceheater.htm> ,
                                                                                  <https://standards.buildingsmart.org/IFC/RELEASE/IFC4_1/FINAL/HTML/schema/ifchvacdomain/pset/pset_spaceheatertypecommon.htm> ;
                                                rdfs:comment """Space heaters utilize a combination of radiation and/or natural convection using a heating source such as electricity, steam or hot water to heat a limited space or area. Examples of space heaters include radiators, convectors, baseboard and finned-tube heaters.

UnitaryEquipment should be used for packaged units supporting a combination of heating, cooling, and/or dehumidification; Coil should be used for coil-based floor heating."""@en ;
                                                rdfs:label "Space heater"@en ;
                                                rdfs:seeAlso "https://w3id.org/ifc/IFC4_ADD1#IfcSpaceHeater" .


###  https://saref.etsi.org/saref4bldg/SwitchingDevice
<https://saref.etsi.org/saref4bldg/SwitchingDevice> rdf:type owl:Class ;
                                                    rdfs:subClassOf <https://saref.etsi.org/saref4bldg/FlowController> ;
                                                    <http://purl.org/dc/terms/source> <https://standards.buildingsmart.org/IFC/RELEASE/IFC4_1/FINAL/HTML/schema/ifcelectricaldomain/lexical/ifcswitchingdevice.htm> ,
                                                                                      <https://standards.buildingsmart.org/IFC/RELEASE/IFC4_1/FINAL/HTML/schema/ifcelectricaldomain/pset/pset_switchingdevicetypecommon.htm> ;
                                                    rdfs:comment """A switch is used in a cable distribution system (electrical circuit) to control or modulate the flow of electricity.

Switches include those used for electrical power, communications, audio-visual, or other distribution system types as determined by the available ports."""@en ;
                                                    rdfs:label "Switching device"@en ;
                                                    rdfs:seeAlso "https://w3id.org/ifc/IFC4_ADD1#IfcSwitchingDevice" .


###  https://saref.etsi.org/saref4bldg/Tank
<https://saref.etsi.org/saref4bldg/Tank> rdf:type owl:Class ;
                                         rdfs:subClassOf <https://saref.etsi.org/saref4bldg/FlowStorageDevice> ,
                                                         [ rdf:type owl:Restriction ;
                                                           owl:onProperty <https://saref.etsi.org/core/hasProperty> ;
                                                           owl:hasValue <https://saref.etsi.org/saref4bldg/effectiveCapacity>
                                                         ] ,
                                                         [ rdf:type owl:Restriction ;
                                                           owl:onProperty <https://saref.etsi.org/core/hasProperty> ;
                                                           owl:hasValue <https://saref.etsi.org/saref4bldg/firstCurvatureRadius>
                                                         ] ,
                                                         [ rdf:type owl:Restriction ;
                                                           owl:onProperty <https://saref.etsi.org/core/hasProperty> ;
                                                           owl:hasValue <https://saref.etsi.org/saref4bldg/nominalDepth>
                                                         ] ,
                                                         [ rdf:type owl:Restriction ;
                                                           owl:onProperty <https://saref.etsi.org/core/hasProperty> ;
                                                           owl:hasValue <https://saref.etsi.org/saref4bldg/nominalLengthOrDiameter>
                                                         ] ,
                                                         [ rdf:type owl:Restriction ;
                                                           owl:onProperty <https://saref.etsi.org/core/hasProperty> ;
                                                           owl:hasValue <https://saref.etsi.org/saref4bldg/nominalVolumetricCapacity>
                                                         ] ,
                                                         [ rdf:type owl:Restriction ;
                                                           owl:onProperty <https://saref.etsi.org/core/hasProperty> ;
                                                           owl:hasValue <https://saref.etsi.org/saref4bldg/nominalWidthOrDiameter>
                                                         ] ,
                                                         [ rdf:type owl:Restriction ;
                                                           owl:onProperty <https://saref.etsi.org/core/hasProperty> ;
                                                           owl:hasValue <https://saref.etsi.org/saref4bldg/operatingWeight>
                                                         ] ,
                                                         [ rdf:type owl:Restriction ;
                                                           owl:onProperty <https://saref.etsi.org/core/hasProperty> ;
                                                           owl:hasValue <https://saref.etsi.org/saref4bldg/secondCurvatureRadius>
                                                         ] ;
                                         <http://purl.org/dc/terms/source> <https://standards.buildingsmart.org/IFC/RELEASE/IFC4_1/FINAL/HTML/schema/ifchvacdomain/lexical/ifctank.htm> ,
                                                                           <https://standards.buildingsmart.org/IFC/RELEASE/IFC4_1/FINAL/HTML/schema/ifchvacdomain/pset/pset_tanktypecommon.htm> ;
                                         rdfs:comment "A tank is a vessel or container in which a fluid or gas is stored for later use."@en ;
                                         rdfs:label "Tank"@en ;
                                         rdfs:seeAlso "https://w3id.org/ifc/IFC4_ADD1#IfcTank" .


###  https://saref.etsi.org/saref4bldg/Transformer
<https://saref.etsi.org/saref4bldg/Transformer> rdf:type owl:Class ;
                                                rdfs:subClassOf <https://saref.etsi.org/saref4bldg/EnergyConversionDevice> ,
                                                                [ rdf:type owl:Restriction ;
                                                                  owl:onProperty <https://saref.etsi.org/core/hasProperty> ;
                                                                  owl:hasValue <https://saref.etsi.org/saref4bldg/apparentPowerMax>
                                                                ] ,
                                                                [ rdf:type owl:Restriction ;
                                                                  owl:onProperty <https://saref.etsi.org/core/hasProperty> ;
                                                                  owl:hasValue <https://saref.etsi.org/saref4bldg/imaginaryImpedanceRatio>
                                                                ] ,
                                                                [ rdf:type owl:Restriction ;
                                                                  owl:onProperty <https://saref.etsi.org/core/hasProperty> ;
                                                                  owl:hasValue <https://saref.etsi.org/saref4bldg/primaryApparentPower>
                                                                ] ,
                                                                [ rdf:type owl:Restriction ;
                                                                  owl:onProperty <https://saref.etsi.org/core/hasProperty> ;
                                                                  owl:hasValue <https://saref.etsi.org/saref4bldg/primaryCurrent>
                                                                ] ,
                                                                [ rdf:type owl:Restriction ;
                                                                  owl:onProperty <https://saref.etsi.org/core/hasProperty> ;
                                                                  owl:hasValue <https://saref.etsi.org/saref4bldg/primaryFrequency>
                                                                ] ,
                                                                [ rdf:type owl:Restriction ;
                                                                  owl:onProperty <https://saref.etsi.org/core/hasProperty> ;
                                                                  owl:hasValue <https://saref.etsi.org/saref4bldg/primaryVoltage>
                                                                ] ,
                                                                [ rdf:type owl:Restriction ;
                                                                  owl:onProperty <https://saref.etsi.org/core/hasProperty> ;
                                                                  owl:hasValue <https://saref.etsi.org/saref4bldg/realImpedanceRatio>
                                                                ] ,
                                                                [ rdf:type owl:Restriction ;
                                                                  owl:onProperty <https://saref.etsi.org/core/hasProperty> ;
                                                                  owl:hasValue <https://saref.etsi.org/saref4bldg/secondaryApparentPower>
                                                                ] ,
                                                                [ rdf:type owl:Restriction ;
                                                                  owl:onProperty <https://saref.etsi.org/core/hasProperty> ;
                                                                  owl:hasValue <https://saref.etsi.org/saref4bldg/secondaryCurrent>
                                                                ] ,
                                                                [ rdf:type owl:Restriction ;
                                                                  owl:onProperty <https://saref.etsi.org/core/hasProperty> ;
                                                                  owl:hasValue <https://saref.etsi.org/saref4bldg/secondaryFrequency>
                                                                ] ,
                                                                [ rdf:type owl:Restriction ;
                                                                  owl:onProperty <https://saref.etsi.org/core/hasProperty> ;
                                                                  owl:hasValue <https://saref.etsi.org/saref4bldg/secondaryVoltage>
                                                                ] ;
                                                <http://purl.org/dc/terms/source> <https://standards.buildingsmart.org/IFC/RELEASE/IFC4_1/FINAL/HTML/schema/ifcelectricaldomain/lexical/ifctransformer.htm> ,
                                                                                  <https://standards.buildingsmart.org/IFC/RELEASE/IFC4_1/FINAL/HTML/schema/ifcelectricaldomain/pset/pset_transformertypecommon.htm> ;
                                                rdfs:comment """A transformer is an inductive stationary device that transfers electrical energy from one circuit to another.

Transformer is used to transform electric power; conversion of electric signals for other purposes is handled at other entities: Controller converts arbitrary signals, AudioVisualAppliance converts signals for audio or video streams, and CommunicationsAppliance converts signals for data or other communications usage."""@en ;
                                                rdfs:label "Transformer"@en ;
                                                rdfs:seeAlso "https://w3id.org/ifc/IFC4_ADD1#IfcTransformer" .


###  https://saref.etsi.org/saref4bldg/TransportElement
<https://saref.etsi.org/saref4bldg/TransportElement> rdf:type owl:Class ;
                                                     rdfs:subClassOf <https://saref.etsi.org/core/Device> ,
                                                                     [ rdf:type owl:Restriction ;
                                                                       owl:onProperty <https://saref.etsi.org/core/hasProperty> ;
                                                                       owl:hasValue <https://saref.etsi.org/saref4bldg/capacityWeight>
                                                                     ] ,
                                                                     [ rdf:type owl:Restriction ;
                                                                       owl:onProperty <https://saref.etsi.org/saref4bldg/capacityPeople> ;
                                                                       owl:allValuesFrom xsd:positiveInteger
                                                                     ] ;
                                                     <http://purl.org/dc/terms/source> <https://standards.buildingsmart.org/IFC/RELEASE/IFC4_1/FINAL/HTML/schema/ifcproductextension/lexical/ifctransportelement.htm> ,
                                                                                       <https://standards.buildingsmart.org/IFC/RELEASE/IFC4_1/FINAL/HTML/schema/ifcproductextension/pset/pset_transportelementcommon.htm> ;
                                                     rdfs:comment "A transport element is a generalization of all transport related objects that move people, animals or goods within a building or building complex. The TransportElement defines the occurrence of a transport element. "@en ;
                                                     rdfs:label "Transport element"@en ;
                                                     rdfs:seeAlso "https://w3id.org/ifc/IFC4_ADD1#IfcTransportElement" .


###  https://saref.etsi.org/saref4bldg/TubeBundle
<https://saref.etsi.org/saref4bldg/TubeBundle> rdf:type owl:Class ;
                                               rdfs:subClassOf <https://saref.etsi.org/saref4bldg/EnergyConversionDevice> ,
                                                               [ rdf:type owl:Restriction ;
                                                                 owl:onProperty <https://saref.etsi.org/core/hasProperty> ;
                                                                 owl:hasValue <https://saref.etsi.org/saref4bldg/foulingFactor>
                                                               ] ,
                                                               [ rdf:type owl:Restriction ;
                                                                 owl:onProperty <https://saref.etsi.org/core/hasProperty> ;
                                                                 owl:hasValue <https://saref.etsi.org/saref4bldg/horizontalSpacing>
                                                               ] ,
                                                               [ rdf:type owl:Restriction ;
                                                                 owl:onProperty <https://saref.etsi.org/core/hasProperty> ;
                                                                 owl:hasValue <https://saref.etsi.org/saref4bldg/inLineRowSpacing>
                                                               ] ,
                                                               [ rdf:type owl:Restriction ;
                                                                 owl:onProperty <https://saref.etsi.org/core/hasProperty> ;
                                                                 owl:hasValue <https://saref.etsi.org/saref4bldg/insideDiameter>
                                                               ] ,
                                                               [ rdf:type owl:Restriction ;
                                                                 owl:onProperty <https://saref.etsi.org/core/hasProperty> ;
                                                                 owl:hasValue <https://saref.etsi.org/saref4bldg/length>
                                                               ] ,
                                                               [ rdf:type owl:Restriction ;
                                                                 owl:onProperty <https://saref.etsi.org/core/hasProperty> ;
                                                                 owl:hasValue <https://saref.etsi.org/saref4bldg/nominalDiameter>
                                                               ] ,
                                                               [ rdf:type owl:Restriction ;
                                                                 owl:onProperty <https://saref.etsi.org/core/hasProperty> ;
                                                                 owl:hasValue <https://saref.etsi.org/saref4bldg/outsideDiameter>
                                                               ] ,
                                                               [ rdf:type owl:Restriction ;
                                                                 owl:onProperty <https://saref.etsi.org/core/hasProperty> ;
                                                                 owl:hasValue <https://saref.etsi.org/saref4bldg/staggeredRowSpacing>
                                                               ] ,
                                                               [ rdf:type owl:Restriction ;
                                                                 owl:onProperty <https://saref.etsi.org/core/hasProperty> ;
                                                                 owl:hasValue <https://saref.etsi.org/saref4bldg/thermalConductivity>
                                                               ] ,
                                                               [ rdf:type owl:Restriction ;
                                                                 owl:onProperty <https://saref.etsi.org/core/hasProperty> ;
                                                                 owl:hasValue <https://saref.etsi.org/saref4bldg/verticalSpacing>
                                                               ] ,
                                                               [ rdf:type owl:Restriction ;
                                                                 owl:onProperty <https://saref.etsi.org/core/hasProperty> ;
                                                                 owl:hasValue <https://saref.etsi.org/saref4bldg/volumen>
                                                               ] ;
                                               <http://purl.org/dc/terms/source> <https://standards.buildingsmart.org/IFC/RELEASE/IFC4_1/FINAL/HTML/schema/ifchvacdomain/lexical/ifctubebundle.htm> ,
                                                                                 <https://standards.buildingsmart.org/IFC/RELEASE/IFC4_1/FINAL/HTML/schema/ifchvacdomain/pset/pset_tubebundletypecommon.htm> ;
                                               rdfs:comment "A tube bundle is a device consisting of tubes and bundles of tubes used for heat transfer and contained typically within other energy conversion devices, such as a chiller or coil."@en ;
                                               rdfs:label "Tube bundle"@en ;
                                               rdfs:seeAlso "https://w3id.org/ifc/IFC4_ADD1#IfcTubeBundle" .


###  https://saref.etsi.org/saref4bldg/UnitaryControlElement
<https://saref.etsi.org/saref4bldg/UnitaryControlElement> rdf:type owl:Class ;
                                                          rdfs:subClassOf <https://saref.etsi.org/saref4bldg/DistributionControlDevice> ;
                                                          <http://purl.org/dc/terms/source> <https://standards.buildingsmart.org/IFC/RELEASE/IFC4_1/FINAL/HTML/schema/ifcbuildingcontrolsdomain/lexical/ifcunitarycontrolelement.htm> ,
                                                                                            <https://standards.buildingsmart.org/IFC/RELEASE/IFC4_1/FINAL/HTML/schema/ifcbuildingcontrolsdomain/pset/pset_unitarycontrolelementtypecommon.htm> ;
                                                          rdfs:comment """A unitary control element combines a number of control components into a single product, such as a thermostat or humidistat.

A unitary control element provides a housing for an aggregation of control or electrical distribution elements that, in combination, perform a singular (unitary) purpose. Each item in the aggregation may have its own geometric representation and location."""@en ;
                                                          rdfs:label "Unitary control element"@en ;
                                                          rdfs:seeAlso "https://w3id.org/ifc/IFC4_ADD1#IfcUnitaryControlElement" .


###  https://saref.etsi.org/saref4bldg/Valve
<https://saref.etsi.org/saref4bldg/Valve> rdf:type owl:Class ;
                                          rdfs:subClassOf <https://saref.etsi.org/saref4bldg/FlowController> ,
                                                          [ rdf:type owl:Restriction ;
                                                            owl:onProperty <https://saref.etsi.org/core/hasProperty> ;
                                                            owl:hasValue <https://saref.etsi.org/saref4bldg/closeOffRating>
                                                          ] ,
                                                          [ rdf:type owl:Restriction ;
                                                            owl:onProperty <https://saref.etsi.org/core/hasProperty> ;
                                                            owl:hasValue <https://saref.etsi.org/saref4bldg/flowCoefficient>
                                                          ] ,
                                                          [ rdf:type owl:Restriction ;
                                                            owl:onProperty <https://saref.etsi.org/core/hasProperty> ;
                                                            owl:hasValue <https://saref.etsi.org/saref4bldg/size>
                                                          ] ,
                                                          [ rdf:type owl:Restriction ;
                                                            owl:onProperty <https://saref.etsi.org/core/hasProperty> ;
                                                            owl:hasValue <https://saref.etsi.org/saref4bldg/testPressure>
                                                          ] ,
                                                          [ rdf:type owl:Restriction ;
                                                            owl:onProperty <https://saref.etsi.org/core/hasProperty> ;
                                                            owl:hasValue <https://saref.etsi.org/saref4bldg/workingPressure>
                                                          ] ;
                                          <http://purl.org/dc/terms/source> <https://standards.buildingsmart.org/IFC/RELEASE/IFC4_1/FINAL/HTML/schema/ifchvacdomain/lexical/ifcvalve.htm> ,
                                                                            <https://standards.buildingsmart.org/IFC/RELEASE/IFC4_1/FINAL/HTML/schema/ifchvacdomain/pset/pset_valvetypecommon.htm> ;
                                          rdfs:comment "A valve is used in a building services piping distribution system to control or modulate the flow of the fluid."@en ;
                                          rdfs:label "Valve"@en ;
                                          rdfs:seeAlso "https://w3id.org/ifc/IFC4_ADD1#IfcValve" .


###  https://saref.etsi.org/saref4bldg/VibrationIsolator
<https://saref.etsi.org/saref4bldg/VibrationIsolator> rdf:type owl:Class ;
                                                      rdfs:subClassOf <https://saref.etsi.org/core/Device> ,
                                                                      [ rdf:type owl:Restriction ;
                                                                        owl:onProperty <https://saref.etsi.org/core/hasProperty> ;
                                                                        owl:hasValue <https://saref.etsi.org/saref4bldg/height>
                                                                      ] ,
                                                                      [ rdf:type owl:Restriction ;
                                                                        owl:onProperty <https://saref.etsi.org/core/hasProperty> ;
                                                                        owl:hasValue <https://saref.etsi.org/saref4bldg/isolatorCompressibility>
                                                                      ] ,
                                                                      [ rdf:type owl:Restriction ;
                                                                        owl:onProperty <https://saref.etsi.org/core/hasProperty> ;
                                                                        owl:hasValue <https://saref.etsi.org/saref4bldg/isolatorStaticDeflection>
                                                                      ] ,
                                                                      [ rdf:type owl:Restriction ;
                                                                        owl:onProperty <https://saref.etsi.org/core/hasProperty> ;
                                                                        owl:hasValue <https://saref.etsi.org/saref4bldg/supportedWeightMax>
                                                                      ] ,
                                                                      [ rdf:type owl:Restriction ;
                                                                        owl:onProperty <https://saref.etsi.org/core/hasProperty> ;
                                                                        owl:hasValue <https://saref.etsi.org/saref4bldg/vibrationTransmissibility>
                                                                      ] ;
                                                      <http://purl.org/dc/terms/source> <https://standards.buildingsmart.org/IFC/RELEASE/IFC4_1/FINAL/HTML/schema/ifchvacdomain/lexical/ifcvibrationisolator.htm> ,
                                                                                        <https://standards.buildingsmart.org/IFC/RELEASE/IFC4_1/FINAL/HTML/schema/ifchvacdomain/pset/pset_vibrationisolatortypecommon.htm> ;
                                                      rdfs:comment "A vibration isolator is a device used to minimize the effects of vibration transmissibility in a building."@en ;
                                                      rdfs:label "Vibration isolator"@en ;
                                                      rdfs:seeAlso "https://w3id.org/ifc/IFC4_ADD1#IfcVibrationIsolator" .


###  https://saref.etsi.org/saref4syst/System
<https://saref.etsi.org/saref4syst/System> rdf:type owl:Class .


#################################################################
#    Individuals
#################################################################

###  https://saref.etsi.org/saref4bldg/airFlowRateMax
<https://saref.etsi.org/saref4bldg/airFlowRateMax> rdf:type owl:NamedIndividual ,
                                                            <https://saref.etsi.org/core/Property> ;
                                                   rdfs:comment "Maximum allowable air flow rate. Usually measured in m3/s."@en ;
                                                   rdfs:label "air flow rate range max"@en .


###  https://saref.etsi.org/saref4bldg/airFlowRateMin
<https://saref.etsi.org/saref4bldg/airFlowRateMin> rdf:type owl:NamedIndividual ,
                                                            <https://saref.etsi.org/core/Property> ;
                                                   rdfs:comment "Minimum allowable air flow rate. Usually measured in m3/s."@en ;
                                                   rdfs:label "air flow rate range min"@en .


###  https://saref.etsi.org/saref4bldg/ambientDesignDryBulbTemperature
<https://saref.etsi.org/saref4bldg/ambientDesignDryBulbTemperature> rdf:type owl:NamedIndividual ,
                                                                             <https://saref.etsi.org/core/Property> ;
                                                                    rdfs:comment "Ambient design dry bulb temperature used for selecting the cooling tower. Usually measured in degrees Kelvin (K)."@en ;
                                                                    rdfs:label "ambient design dry bulb temperature"@en .


###  https://saref.etsi.org/saref4bldg/ambientDesignWetBulbTemperature
<https://saref.etsi.org/saref4bldg/ambientDesignWetBulbTemperature> rdf:type owl:NamedIndividual ,
                                                                             <https://saref.etsi.org/core/Property> ;
                                                                    rdfs:comment "Ambient design wet bulb temperature used for selecting the cooling tower. Usually measured in degrees Kelvin (K)."@en ;
                                                                    rdfs:label "ambient design wet bulb temperature"@en .


###  https://saref.etsi.org/saref4bldg/apparentPowerMax
<https://saref.etsi.org/saref4bldg/apparentPowerMax> rdf:type owl:NamedIndividual ,
                                                              <https://saref.etsi.org/core/Property> ;
                                                     rdfs:comment "Maximum apparent power/capacity in VA (volt ampere). Usually measured in Watts (W, J/s)."@en ;
                                                     rdfs:label "maximum apparent power"@en .


###  https://saref.etsi.org/saref4bldg/audioVolume
<https://saref.etsi.org/saref4bldg/audioVolume> rdf:type owl:NamedIndividual ,
                                                         <https://saref.etsi.org/core/Property> ;
                                                rdfs:comment "Indicates discrete audio volume levels and corresponding sound power offsets, if applicable. Missing values may be interpolated. Measured in watts."@en ;
                                                rdfs:label "audio volume"@en .


###  https://saref.etsi.org/saref4bldg/basinReserveVolume
<https://saref.etsi.org/saref4bldg/basinReserveVolume> rdf:type owl:NamedIndividual ,
                                                                <https://saref.etsi.org/core/Property> ;
                                                       rdfs:comment "Volume between operating and overflow levels in cooling tower basin. Usually measured in cubic metre (m3)."@en ;
                                                       rdfs:label "basin reserve volume"@en .


###  https://saref.etsi.org/saref4bldg/bladeThickness
<https://saref.etsi.org/saref4bldg/bladeThickness> rdf:type owl:NamedIndividual ,
                                                            <https://saref.etsi.org/core/Property> ;
                                                   rdfs:comment "The thickness of the damper blade. Usually measured in millimeters (mm)."@en ;
                                                   rdfs:label "blade thickness"@en .


###  https://saref.etsi.org/saref4bldg/bodyMass
<https://saref.etsi.org/saref4bldg/bodyMass> rdf:type owl:NamedIndividual ,
                                                      <https://saref.etsi.org/core/Property> ;
                                             rdfs:comment "Overall body mass of the heater. Usually measured in kilograms (kg) or grams (g)."@en ;
                                             rdfs:label "body mass"@en .


###  https://saref.etsi.org/saref4bldg/capacityWeight
<https://saref.etsi.org/saref4bldg/capacityWeight> rdf:type owl:NamedIndividual ,
                                                            <https://saref.etsi.org/core/Property> ;
                                                   rdfs:comment "Capacity of the transport element measured by weight. Usually measured in kilograms (kg) or grams (g)."@en ;
                                                   rdfs:label "capacity weight"@en .


###  https://saref.etsi.org/saref4bldg/closeOffRating
<https://saref.etsi.org/saref4bldg/closeOffRating> rdf:type owl:NamedIndividual ,
                                                            <https://saref.etsi.org/core/Property> ;
                                                   rdfs:comment "Close off rating. Usually measured in Pascals (Pa, N/m2)."@en ;
                                                   rdfs:label "close off rating"@en .


###  https://saref.etsi.org/saref4bldg/coilLength
<https://saref.etsi.org/saref4bldg/coilLength> rdf:type owl:NamedIndividual ,
                                                        <https://saref.etsi.org/core/Property> ;
                                               rdfs:comment "Length of coil. Usually measured in millimeters (mm)."@en ;
                                               rdfs:label "coil length"@en .


###  https://saref.etsi.org/saref4bldg/coilWidth
<https://saref.etsi.org/saref4bldg/coilWidth> rdf:type owl:NamedIndividual ,
                                                       <https://saref.etsi.org/core/Property> ;
                                              rdfs:comment "Width of coil. Usually measured in millimeters (mm"@en ;
                                              rdfs:label "coil width"@en .


###  https://saref.etsi.org/saref4bldg/colorTemperature
<https://saref.etsi.org/saref4bldg/colorTemperature> rdf:type owl:NamedIndividual ,
                                                              <https://saref.etsi.org/core/Property> ;
                                                     rdfs:comment "The color temperature of any source of radiation is defined as the temperature (in Kelvin) of a black-body or Planckian radiator whose radiation has the same chromaticity as the source of radiation. Often the values are only approximate color temperatures as the black-body radiator cannot emit radiation of every chromaticity value. The color temperatures of the commonest artificial light sources range from less than 3000K (warm white) to 4000K (intermediate) and over 5000K (daylight). Usually measured in degrees Kelvin (K)."@en ;
                                                     rdfs:label "color temperature"@en .


###  https://saref.etsi.org/saref4bldg/compressorSpeed
<https://saref.etsi.org/saref4bldg/compressorSpeed> rdf:type owl:NamedIndividual ,
                                                             <https://saref.etsi.org/core/Property> ;
                                                    rdfs:comment "Compressor speed. Usually measured in cycles/s."@en ;
                                                    rdfs:label "compressor speed"@en .


###  https://saref.etsi.org/saref4bldg/connectionSize
<https://saref.etsi.org/saref4bldg/connectionSize> rdf:type owl:NamedIndividual ,
                                                            <https://saref.etsi.org/core/Property> ;
                                                   rdfs:comment "The connection size of the to and from the pump. Usually measured in millimeters (mm)."@en ;
                                                   rdfs:label "connection size"@en .


###  https://saref.etsi.org/saref4bldg/contributedLuminousFlux
<https://saref.etsi.org/saref4bldg/contributedLuminousFlux> rdf:type owl:NamedIndividual ,
                                                                     <https://saref.etsi.org/core/Property> ;
                                                            rdfs:comment "Luminous flux is a photometric measure of radiant flux, i.e. the volume of light emitted from a light source. Luminous flux is measured either for the interior as a whole or for a part of the interior (partial luminous flux for a solid angle). All other photometric parameters are derivatives of luminous flux. Luminous flux is measured in lumens (lm). The luminous flux is given as a nominal value for each lamp. Usually measured in Lumen (lm, Candela Steradian)."@en ;
                                                            rdfs:label "contributed luminous flux"@en .


###  https://saref.etsi.org/saref4bldg/coverLength
<https://saref.etsi.org/saref4bldg/coverLength> rdf:type owl:NamedIndividual ,
                                                         <https://saref.etsi.org/core/Property> ;
                                                rdfs:comment "The length measured along the x-axis in the local coordinate system or the radius (in the case of a circular shape in plan) of the cover of the oil interceptor. Usually measured in millimeters (mm)."@en ;
                                                rdfs:label "cover length"@en .


###  https://saref.etsi.org/saref4bldg/coverWidth
<https://saref.etsi.org/saref4bldg/coverWidth> rdf:type owl:NamedIndividual ,
                                                        <https://saref.etsi.org/core/Property> ;
                                               rdfs:comment "The length measured along the x-axis in the local coordinate system of the cover of the oil interceptor. Usually measured in millimeters (mm)."@en ;
                                               rdfs:label "cover width"@en .


###  https://saref.etsi.org/saref4bldg/effectiveCapacity
<https://saref.etsi.org/saref4bldg/effectiveCapacity> rdf:type owl:NamedIndividual ,
                                                               <https://saref.etsi.org/core/Property> ;
                                                      rdfs:comment "The total effective or actual volumetric capacity of the tank. Usually measured in cubic metre (m3).B3"@en ;
                                                      rdfs:label "effective capacity"@en .


###  https://saref.etsi.org/saref4bldg/electricGeneratorEfficiency
<https://saref.etsi.org/saref4bldg/electricGeneratorEfficiency> rdf:type owl:NamedIndividual ,
                                                                         <https://saref.etsi.org/core/Property> ;
                                                                rdfs:comment "The ratio of output capacity to intake capacity."@en ;
                                                                rdfs:label "electric generator efficiency"@en .


###  https://saref.etsi.org/saref4bldg/electricMotorEfficiency
<https://saref.etsi.org/saref4bldg/electricMotorEfficiency> rdf:type owl:NamedIndividual ,
                                                                     <https://saref.etsi.org/core/Property> ;
                                                            rdfs:comment "The ratio of output capacity to intake capacity."@en ;
                                                            rdfs:label "electric motor efficiency"@en .


###  https://saref.etsi.org/saref4bldg/externalSurfaceArea
<https://saref.etsi.org/saref4bldg/externalSurfaceArea> rdf:type owl:NamedIndividual ,
                                                                 <https://saref.etsi.org/core/Property> ;
                                                        rdfs:comment "External surface area (both primary and secondary area). Usually measured in square metre (m2)."@en ;
                                                        rdfs:label "external surface area"@en .


###  https://saref.etsi.org/saref4bldg/faceArea
<https://saref.etsi.org/saref4bldg/faceArea> rdf:type owl:NamedIndividual ,
                                                      <https://saref.etsi.org/core/Property> ;
                                             rdfs:comment "Face area open to the airstream. Usually measured in square metre (m2)."@en ;
                                             rdfs:label "face area"@en .


###  https://saref.etsi.org/saref4bldg/finalResistance
<https://saref.etsi.org/saref4bldg/finalResistance> rdf:type owl:NamedIndividual ,
                                                             <https://saref.etsi.org/core/Property> ;
                                                    rdfs:comment "Filter fluid resistance when replacement is required (i.e., Pressure drop at the maximum air flowrate across the filter when the filter needs replacement per ASHRAE Standard 52.1). Usually measured in Pascals (Pa, N/m2)."@en ;
                                                    rdfs:label "final resistance"@en .


###  https://saref.etsi.org/saref4bldg/firstCurvatureRadius
<https://saref.etsi.org/saref4bldg/firstCurvatureRadius> rdf:type owl:NamedIndividual ,
                                                                  <https://saref.etsi.org/core/Property> ;
                                                         rdfs:comment "FirstCurvatureRadius should be defined as the base or left side radius of curvature value. Usually measured in millimeters (mm)."@en ;
                                                         rdfs:label "first curvature radius"@en .


###  https://saref.etsi.org/saref4bldg/flowCoefficient
<https://saref.etsi.org/saref4bldg/flowCoefficient> rdf:type owl:NamedIndividual ,
                                                             <https://saref.etsi.org/core/Property> ;
                                                    rdfs:comment "Flow coefficient (the quantity of fluid that passes through a fully open valve at unit pressure drop), typically expressed as the Kv or Cv value for the valve."@en ;
                                                    rdfs:label "flow coefficient"@en .


###  https://saref.etsi.org/saref4bldg/flowResistanceMax
<https://saref.etsi.org/saref4bldg/flowResistanceMax> rdf:type owl:NamedIndividual ,
                                                               <https://saref.etsi.org/core/Property> ;
                                                      rdfs:comment "Allowable range of frictional resistance against which the fluid is being pumped. Usually measured in Pascals (Pa, N/m2)."@en ;
                                                      rdfs:label "flow resistance range"@en .


###  https://saref.etsi.org/saref4bldg/flowResistanceMin
<https://saref.etsi.org/saref4bldg/flowResistanceMin> rdf:type owl:NamedIndividual ,
                                                               <https://saref.etsi.org/core/Property> ;
                                                      rdfs:comment "Allowable range of frictional resistance against which the fluid is being pumped. Usually measured in Pascals (Pa, N/m2)."@en ;
                                                      rdfs:label "flow resistance range"@en .


###  https://saref.etsi.org/saref4bldg/fluidFlowRateMax
<https://saref.etsi.org/saref4bldg/fluidFlowRateMax> rdf:type owl:NamedIndividual ,
                                                              <https://saref.etsi.org/core/Property> ;
                                                     rdfs:comment "Possible range of fluid flowrate that can be delivered. Usually measured in m3/s."@en ;
                                                     rdfs:label "fluid flow rate range"@en .


###  https://saref.etsi.org/saref4bldg/fluidFlowRateMin
<https://saref.etsi.org/saref4bldg/fluidFlowRateMin> rdf:type owl:NamedIndividual ,
                                                              <https://saref.etsi.org/core/Property> ;
                                                     rdfs:comment "Possible range of fluid flowrate that can be delivered. Usually measured in m3/s."@en ;
                                                     rdfs:label "fluid flow rate range"@en .


###  https://saref.etsi.org/saref4bldg/foulingFactor
<https://saref.etsi.org/saref4bldg/foulingFactor> rdf:type owl:NamedIndividual ,
                                                           <https://saref.etsi.org/core/Property> ;
                                                  rdfs:comment "Fouling factor of the tubes in the tube bundle. Usually measured in m2 Kelvin/Watt."@en ;
                                                  rdfs:label "fouling factor"@en .


###  https://saref.etsi.org/saref4bldg/frameDepth
<https://saref.etsi.org/saref4bldg/frameDepth> rdf:type owl:NamedIndividual ,
                                                        <https://saref.etsi.org/core/Property> ;
                                               rdfs:comment "The length (or depth) of the damper frame. Usually measured in millimeters (mm)."@en ;
                                               rdfs:label "frame depth"@en .


###  https://saref.etsi.org/saref4bldg/frameThickness
<https://saref.etsi.org/saref4bldg/frameThickness> rdf:type owl:NamedIndividual ,
                                                            <https://saref.etsi.org/core/Property> ;
                                                   rdfs:comment "The thickness of the damper frame material. Usually measured in millimeters (mm)."@en ;
                                                   rdfs:label "frame thickness"@en .


###  https://saref.etsi.org/saref4bldg/heatExchangeArea
<https://saref.etsi.org/saref4bldg/heatExchangeArea> rdf:type owl:NamedIndividual ,
                                                              <https://saref.etsi.org/core/Property> ;
                                                     rdfs:comment "Heat exchange area. Usually measured in square metre (m2)."@en ;
                                                     rdfs:label "heat exchange area"@en .


###  https://saref.etsi.org/saref4bldg/heatTransferSurfaceArea
<https://saref.etsi.org/saref4bldg/heatTransferSurfaceArea> rdf:type owl:NamedIndividual ,
                                                                     <https://saref.etsi.org/core/Property> ;
                                                            rdfs:comment "Total heat transfer area of the vessel. Usually measured in square metre (m2)."@en ;
                                                            rdfs:label "heat transfer surface area"@en .


###  https://saref.etsi.org/saref4bldg/height
<https://saref.etsi.org/saref4bldg/height> rdf:type owl:NamedIndividual ,
                                                    <https://saref.etsi.org/core/Property> ;
                                           rdfs:comment "Height of the vibration isolator before tha application of load. Usually measured in millimeters (mm)."@en ;
                                           rdfs:label "height"@en .


###  https://saref.etsi.org/saref4bldg/horizontalSpacing
<https://saref.etsi.org/saref4bldg/horizontalSpacing> rdf:type owl:NamedIndividual ,
                                                               <https://saref.etsi.org/core/Property> ;
                                                      rdfs:comment "Horizontal spacing between tubes in the tube bundle. Usually measured in millimeters (mm)."@en ;
                                                      rdfs:label "horizontal spacing"@en .


###  https://saref.etsi.org/saref4bldg/hydraulicDiameter
<https://saref.etsi.org/saref4bldg/hydraulicDiameter> rdf:type owl:NamedIndividual ,
                                                               <https://saref.etsi.org/core/Property> ;
                                                      rdfs:comment "Hydraulic diameter. Usually measured in millimeters (mm)."@en ;
                                                      rdfs:label "hydraulic diameter"@en .


###  https://saref.etsi.org/saref4bldg/idealCapacity
<https://saref.etsi.org/saref4bldg/idealCapacity> rdf:type owl:NamedIndividual ,
                                                           <https://saref.etsi.org/core/Property> ;
                                                  rdfs:comment "Compressor capacity under ideal conditions. Usually measured in Watts (W, J/s)."@en ;
                                                  rdfs:label "ideal capacity"@en .


###  https://saref.etsi.org/saref4bldg/idealShaftPower
<https://saref.etsi.org/saref4bldg/idealShaftPower> rdf:type owl:NamedIndividual ,
                                                             <https://saref.etsi.org/core/Property> ;
                                                    rdfs:comment "Compressor shaft power under ideal conditions. Usually measured in Watts (W, J/s)."@en ;
                                                    rdfs:label "ideal shaft power"@en .


###  https://saref.etsi.org/saref4bldg/imaginaryImpedanceRatio
<https://saref.etsi.org/saref4bldg/imaginaryImpedanceRatio> rdf:type owl:NamedIndividual ,
                                                                     <https://saref.etsi.org/core/Property> ;
                                                            rdfs:comment "The ratio between the imaginary part of the zero sequence impedance and the imaginary part of the positive impedance (i.e. imaginary part of the short-circuit voltage) of the transformer. Used for three-phase transformer which includes a N-conductor."@en ;
                                                            rdfs:label "imaginary impedance ratio"@en .


###  https://saref.etsi.org/saref4bldg/impellerDiameter
<https://saref.etsi.org/saref4bldg/impellerDiameter> rdf:type owl:NamedIndividual ,
                                                              <https://saref.etsi.org/core/Property> ;
                                                     rdfs:comment "Diameter of compressor impeller - used to scale performance of geometrically similar compressors. Usually measured in millimeters (mm)."@en ;
                                                     rdfs:label "impeller diameter"@en .


###  https://saref.etsi.org/saref4bldg/inLineRowSpacing
<https://saref.etsi.org/saref4bldg/inLineRowSpacing> rdf:type owl:NamedIndividual ,
                                                              <https://saref.etsi.org/core/Property> ;
                                                     rdfs:comment "In-line tube row spacing. Usually measured in millimeters (mm)."@en ;
                                                     rdfs:label "in line row spacing"@en .


###  https://saref.etsi.org/saref4bldg/initialResistance
<https://saref.etsi.org/saref4bldg/initialResistance> rdf:type owl:NamedIndividual ,
                                                               <https://saref.etsi.org/core/Property> ;
                                                      rdfs:comment "Initial new filter fluid resistance (i.e., pressure drop at the maximum air flowrate across the filter when the filter is new per ASHRAE Standard 52.1). Usually measured in Pascals (Pa, N/m2)."@en ;
                                                      rdfs:label "initial resistance"@en .


###  https://saref.etsi.org/saref4bldg/inletConnectionSize
<https://saref.etsi.org/saref4bldg/inletConnectionSize> rdf:type owl:NamedIndividual ,
                                                                 <https://saref.etsi.org/core/Property> ;
                                                        rdfs:comment "Size of the inlet connection. Usually measured in millimeters (mm)."@en ;
                                                        rdfs:label "inlet connection size"@en .


###  https://saref.etsi.org/saref4bldg/insideDiameter
<https://saref.etsi.org/saref4bldg/insideDiameter> rdf:type owl:NamedIndividual ,
                                                            <https://saref.etsi.org/core/Property> ;
                                                   rdfs:comment "Actual inner diameter of the tube in the tube bundle. Usually measured in millimeters (mm)."@en ;
                                                   rdfs:label "inside diameter"@en .


###  https://saref.etsi.org/saref4bldg/internalRefrigerantVolume
<https://saref.etsi.org/saref4bldg/internalRefrigerantVolume> rdf:type owl:NamedIndividual ,
                                                                       <https://saref.etsi.org/core/Property> ;
                                                              rdfs:comment "Internal volume of evaporator (refrigerant side). Usually measured in cubic metre (m3)."@en ;
                                                              rdfs:label "internal refrigerant volume"@en .


###  https://saref.etsi.org/saref4bldg/internalSurfaceArea
<https://saref.etsi.org/saref4bldg/internalSurfaceArea> rdf:type owl:NamedIndividual ,
                                                                 <https://saref.etsi.org/core/Property> ;
                                                        rdfs:comment "Internal surface area. Usually measured in square metre (m2)."@en ;
                                                        rdfs:label "internal surface area"@en .


###  https://saref.etsi.org/saref4bldg/internalWaterVolume
<https://saref.etsi.org/saref4bldg/internalWaterVolume> rdf:type owl:NamedIndividual ,
                                                                 <https://saref.etsi.org/core/Property> ;
                                                        rdfs:comment "Internal volume of evaporator (water side). Usually measured in cubic metre (m3)."@en ;
                                                        rdfs:label "internal water volume"@en .


###  https://saref.etsi.org/saref4bldg/isolatorCompressibility
<https://saref.etsi.org/saref4bldg/isolatorCompressibility> rdf:type owl:NamedIndividual ,
                                                                     <https://saref.etsi.org/core/Property> ;
                                                            rdfs:comment "The compressibility of the vibration isolator."@en ;
                                                            rdfs:label "isolator compressibility"@en .


###  https://saref.etsi.org/saref4bldg/isolatorStaticDeflection
<https://saref.etsi.org/saref4bldg/isolatorStaticDeflection> rdf:type owl:NamedIndividual ,
                                                                      <https://saref.etsi.org/core/Property> ;
                                                             rdfs:comment "Static deflection of the vibration isolator. Usually measured in millimeters (mm)."@en ;
                                                             rdfs:label "isolator static deflection"@en .


###  https://saref.etsi.org/saref4bldg/lampMaintenanceFactor
<https://saref.etsi.org/saref4bldg/lampMaintenanceFactor> rdf:type owl:NamedIndividual ,
                                                                   <https://saref.etsi.org/core/Property> ;
                                                          rdfs:comment "Non recoverable losses of luminous flux of a lamp due to lamp depreciation i.e. the decreasing of light output of a luminaire due to aging and dirt."@en ;
                                                          rdfs:label "lamp maintenance factor"@en .


###  https://saref.etsi.org/saref4bldg/leakageFullyClosed
<https://saref.etsi.org/saref4bldg/leakageFullyClosed> rdf:type owl:NamedIndividual ,
                                                                <https://saref.etsi.org/core/Property> ;
                                                       rdfs:comment "Leakage when fully closed. Usually measured in m3/s."@en ;
                                                       rdfs:label "leakage fully closed"@en .


###  https://saref.etsi.org/saref4bldg/length
<https://saref.etsi.org/saref4bldg/length> rdf:type owl:NamedIndividual ,
                                                    <https://saref.etsi.org/core/Property> ;
                                           rdfs:comment "The finished length of the device. Usually measured in millimeters (mm)."@en ;
                                           rdfs:label "length"@en .


###  https://saref.etsi.org/saref4bldg/liftElevationDifference
<https://saref.etsi.org/saref4bldg/liftElevationDifference> rdf:type owl:NamedIndividual ,
                                                                     <https://saref.etsi.org/core/Property> ;
                                                            rdfs:comment "Elevation difference between cooling tower sump and the top of the tower. Usually measured in millimeters (mm)."@en ;
                                                            rdfs:label "lift elevation difference"@en .


###  https://saref.etsi.org/saref4bldg/lightEmitterNominalPower
<https://saref.etsi.org/saref4bldg/lightEmitterNominalPower> rdf:type owl:NamedIndividual ,
                                                                      <https://saref.etsi.org/core/Property> ;
                                                             rdfs:comment "Light emitter nominal power. Usually measured in Watts (W, J/s)."@en ;
                                                             rdfs:label "light emitter nominal power"@en .


###  https://saref.etsi.org/saref4bldg/limitingTerminalSize
<https://saref.etsi.org/saref4bldg/limitingTerminalSize> rdf:type owl:NamedIndividual ,
                                                                  <https://saref.etsi.org/core/Property> ;
                                                         rdfs:comment "The maximum terminal size capacity of the device. Usually measured in square metre (m2)."@en ;
                                                         rdfs:label "limiting terminal size"@en .


###  https://saref.etsi.org/saref4bldg/lockedRotorCurrent
<https://saref.etsi.org/saref4bldg/lockedRotorCurrent> rdf:type owl:NamedIndividual ,
                                                                <https://saref.etsi.org/core/Property> ;
                                                       rdfs:comment "Input current when a motor armature is energized but not rotating. Usually measured in Ampere (A)."@en ;
                                                       rdfs:label "locked rotor current"@en .


###  https://saref.etsi.org/saref4bldg/netPositiveSuctionHead
<https://saref.etsi.org/saref4bldg/netPositiveSuctionHead> rdf:type owl:NamedIndividual ,
                                                                    <https://saref.etsi.org/core/Property> ;
                                                           rdfs:comment "Minimum liquid pressure at the pump inlet to prevent cavitation. Usually measured in Pascals (Pa, N/m2)."@en ;
                                                           rdfs:label "net positive suction head"@en .


###  https://saref.etsi.org/saref4bldg/nominalAirFlowRate
<https://saref.etsi.org/saref4bldg/nominalAirFlowRate> rdf:type owl:NamedIndividual ,
                                                                <https://saref.etsi.org/core/Property> ;
                                                       rdfs:comment "Nominal rate of air flow. Usually measured in m3/s."@en ;
                                                       rdfs:label "nominal air flow rate"@en .


###  https://saref.etsi.org/saref4bldg/nominalBodyDepth
<https://saref.etsi.org/saref4bldg/nominalBodyDepth> rdf:type owl:NamedIndividual ,
                                                              <https://saref.etsi.org/core/Property> ;
                                                     rdfs:comment "Nominal or quoted =length, measured along the z-axis of the local coordinate system of the object, of the body of the object. Usually measured in millimeters (mm)."@en ;
                                                     rdfs:label "nominal body depth"@en .


###  https://saref.etsi.org/saref4bldg/nominalBodyLength
<https://saref.etsi.org/saref4bldg/nominalBodyLength> rdf:type owl:NamedIndividual ,
                                                               <https://saref.etsi.org/core/Property> ;
                                                      rdfs:comment "Nominal or quoted length, measured along the x-axis of the local coordinate system of the object, of the body of the object. Usually measured in millimeters (mm)."@en ;
                                                      rdfs:label "nominal body length"@en .


###  https://saref.etsi.org/saref4bldg/nominalBodyWidth
<https://saref.etsi.org/saref4bldg/nominalBodyWidth> rdf:type owl:NamedIndividual ,
                                                              <https://saref.etsi.org/core/Property> ;
                                                     rdfs:comment "Nominal or quoted length, measured along the y-axis of the local coordinate system of the object, of the body of the object. Usually measured in millimeters (mm)."@en ;
                                                     rdfs:label "nominal body width"@en .


###  https://saref.etsi.org/saref4bldg/nominalCapacity
<https://saref.etsi.org/saref4bldg/nominalCapacity> rdf:type owl:NamedIndividual ,
                                                             <https://saref.etsi.org/core/Property> ;
                                                    rdfs:comment "Nominal capacity. Usually measured in Watts (W, J/s)."@en ;
                                                    rdfs:label "nominal capacity"@en .


###  https://saref.etsi.org/saref4bldg/nominalCondensingTemperature
<https://saref.etsi.org/saref4bldg/nominalCondensingTemperature> rdf:type owl:NamedIndividual ,
                                                                          <https://saref.etsi.org/core/Property> ;
                                                                 rdfs:comment "Chiller condensing temperature. Usually measured in degrees Kelvin (K)."@en ;
                                                                 rdfs:label "nominal condensing temperature"@en .


###  https://saref.etsi.org/saref4bldg/nominalCoolingCapacity
<https://saref.etsi.org/saref4bldg/nominalCoolingCapacity> rdf:type owl:NamedIndividual ,
                                                                    <https://saref.etsi.org/core/Property> ;
                                                           rdfs:comment "Nominal cooling capacity. Usually measured in Watts (W, J/s)."@en ;
                                                           rdfs:label "nominal cooling capacity"@en .


###  https://saref.etsi.org/saref4bldg/nominalDepth
<https://saref.etsi.org/saref4bldg/nominalDepth> rdf:type owl:NamedIndividual ,
                                                          <https://saref.etsi.org/core/Property> ;
                                                 rdfs:comment "The nominal depth of the tank. Note: Not required for a horizontal cylindrical tank. Usually measured in millimeters (mm)."@en ;
                                                 rdfs:label "nominal depth"@en .


###  https://saref.etsi.org/saref4bldg/nominalDiameter
<https://saref.etsi.org/saref4bldg/nominalDiameter> rdf:type owl:NamedIndividual ,
                                                             <https://saref.etsi.org/core/Property> ;
                                                    rdfs:comment "Nominal diameter or width of the tubes in the tube bundle. Usually measured in millimeters (mm)."@en ;
                                                    rdfs:label "nominal diameter"@en .


###  https://saref.etsi.org/saref4bldg/nominalEfficiency
<https://saref.etsi.org/saref4bldg/nominalEfficiency> rdf:type owl:NamedIndividual ,
                                                               <https://saref.etsi.org/core/Property> ;
                                                      rdfs:comment "Nominal chiller efficiency under nominal conditions. "@en ;
                                                      rdfs:label "nominal efficiency"@en .


###  https://saref.etsi.org/saref4bldg/nominalEnergyConsumption
<https://saref.etsi.org/saref4bldg/nominalEnergyConsumption> rdf:type owl:NamedIndividual ,
                                                                      <https://saref.etsi.org/core/Property> ;
                                                             rdfs:comment "Nominal fuel consumption rate required to produce the total boiler heat output. Usually measured in Watts (W, J/s)."@en ;
                                                             rdfs:label "nominal energy consumption"@en .


###  https://saref.etsi.org/saref4bldg/nominalEvaporatingTemmperature
<https://saref.etsi.org/saref4bldg/nominalEvaporatingTemmperature> rdf:type owl:NamedIndividual ,
                                                                            <https://saref.etsi.org/core/Property> ;
                                                                   rdfs:comment "Chiller evaporating temperature.Usually measured in degrees Kelvin (K)."@en ;
                                                                   rdfs:label "nominal evaporating temmperature"@en .


###  https://saref.etsi.org/saref4bldg/nominalFilterFaceVelocity
<https://saref.etsi.org/saref4bldg/nominalFilterFaceVelocity> rdf:type owl:NamedIndividual ,
                                                                       <https://saref.etsi.org/core/Property> ;
                                                              rdfs:comment "Filter face velocity. Usually measured in m/s."@en ;
                                                              rdfs:label "nominal filter face velocity"@en .


###  https://saref.etsi.org/saref4bldg/nominalFlowRate
<https://saref.etsi.org/saref4bldg/nominalFlowRate> rdf:type owl:NamedIndividual ,
                                                             <https://saref.etsi.org/core/Property> ;
                                                    rdfs:comment "Nominal fluid flow rate through the filter. Usually measured in m3/s."@en ;
                                                    rdfs:label "nominal flow rate"@en .


###  https://saref.etsi.org/saref4bldg/nominalFrequency
<https://saref.etsi.org/saref4bldg/nominalFrequency> rdf:type owl:NamedIndividual ,
                                                              <https://saref.etsi.org/core/Property> ;
                                                     rdfs:comment "The nominal frequency of the supply. Usually measured in cycles/s or Hertz (Hz)."@en ;
                                                     rdfs:label "nominal frequency"@en .


###  https://saref.etsi.org/saref4bldg/nominalHeatRejectionRate
<https://saref.etsi.org/saref4bldg/nominalHeatRejectionRate> rdf:type owl:NamedIndividual ,
                                                                      <https://saref.etsi.org/core/Property> ;
                                                             rdfs:comment "Sum of the refrigeration effect and the heat equivalent of the power input to the compressor. Usually measured in Watts (W, J/s)."@en ;
                                                             rdfs:label "nominal heat rejection rate"@en .


###  https://saref.etsi.org/saref4bldg/nominalHeatTransferArea
<https://saref.etsi.org/saref4bldg/nominalHeatTransferArea> rdf:type owl:NamedIndividual ,
                                                                     <https://saref.etsi.org/core/Property> ;
                                                            rdfs:comment "Nominal heat transfer surface area associated with nominal overall heat transfer coefficient. Usually measured in square metre (m2)."@en ;
                                                            rdfs:label "nominal heat transfer area"@en .


###  https://saref.etsi.org/saref4bldg/nominalHeatTransferCoefficient
<https://saref.etsi.org/saref4bldg/nominalHeatTransferCoefficient> rdf:type owl:NamedIndividual ,
                                                                            <https://saref.etsi.org/core/Property> ;
                                                                   rdfs:comment "Nominal overall heat transfer coefficient associated with nominal heat transfer area. Usually measured in Watts/m2 Kelvin."@en ;
                                                                   rdfs:label "nominal heat transfer coefficient"@en .


###  https://saref.etsi.org/saref4bldg/nominalHeatingCapacity
<https://saref.etsi.org/saref4bldg/nominalHeatingCapacity> rdf:type owl:NamedIndividual ,
                                                                    <https://saref.etsi.org/core/Property> ;
                                                           rdfs:comment "Nominal heating capacity. Usually measured in Watts (W, J/s)."@en ;
                                                           rdfs:label "nominal heating capacity"@en .


###  https://saref.etsi.org/saref4bldg/nominalLatentCapacity
<https://saref.etsi.org/saref4bldg/nominalLatentCapacity> rdf:type owl:NamedIndividual ,
                                                                   <https://saref.etsi.org/core/Property> ;
                                                          rdfs:comment "Nominal latent capacity. Usually measured in Watts (W, J/s)."@en ;
                                                          rdfs:label "nominal latent capacity"@en .


###  https://saref.etsi.org/saref4bldg/nominalLengthOrDiameter
<https://saref.etsi.org/saref4bldg/nominalLengthOrDiameter> rdf:type owl:NamedIndividual ,
                                                                     <https://saref.etsi.org/core/Property> ;
                                                            rdfs:comment "The nominal length or, in the case of a vertical cylindrical tank, the nominal diameter of the tank. Usually measured in millimeters (mm)."@en ;
                                                            rdfs:label "nominal length or diameter"@en .


###  https://saref.etsi.org/saref4bldg/nominalMediaSurfaceVelocity
<https://saref.etsi.org/saref4bldg/nominalMediaSurfaceVelocity> rdf:type owl:NamedIndividual ,
                                                                         <https://saref.etsi.org/core/Property> ;
                                                                rdfs:comment "Average fluid velocity at the media surface. Usually measured in m/s."@en ;
                                                                rdfs:label "nominal media surface velocity"@en .


###  https://saref.etsi.org/saref4bldg/nominalMoistureGain
<https://saref.etsi.org/saref4bldg/nominalMoistureGain> rdf:type owl:NamedIndividual ,
                                                                 <https://saref.etsi.org/core/Property> ;
                                                        rdfs:comment "Nominal rate of water vapor added into the airstream. Usually measured in kg/s."@en ;
                                                        rdfs:label "nominal moisture gain"@en .


###  https://saref.etsi.org/saref4bldg/nominalPartLoadRatio
<https://saref.etsi.org/saref4bldg/nominalPartLoadRatio> rdf:type owl:NamedIndividual ,
                                                                  <https://saref.etsi.org/core/Property> ;
                                                         rdfs:comment "Allowable part load ratio range."@en ;
                                                         rdfs:label "nominal part load ratio"@en .


###  https://saref.etsi.org/saref4bldg/nominalParticleGeometricMeanDiameter
<https://saref.etsi.org/saref4bldg/nominalParticleGeometricMeanDiameter> rdf:type owl:NamedIndividual ,
                                                                                  <https://saref.etsi.org/core/Property> ;
                                                                         rdfs:comment "Particle geometric mean diameter associated with nominal efficiency. Usually measured in millimeters (mm)."@en ;
                                                                         rdfs:label "nominal particle geometric mean diameter"@en .


###  https://saref.etsi.org/saref4bldg/nominalParticleGeometricStandardDeviation
<https://saref.etsi.org/saref4bldg/nominalParticleGeometricStandardDeviation> rdf:type owl:NamedIndividual ,
                                                                                       <https://saref.etsi.org/core/Property> ;
                                                                              rdfs:comment "Particle geometric standard deviation associated with nominal efficiency. "@en ;
                                                                              rdfs:label "nominal particle geometric standard deviation"@en .


###  https://saref.etsi.org/saref4bldg/nominalPowerConsumption
<https://saref.etsi.org/saref4bldg/nominalPowerConsumption> rdf:type owl:NamedIndividual ,
                                                                     <https://saref.etsi.org/core/Property> ;
                                                            rdfs:comment "Nominal total power consumption. Usually measured in Watts (W, J/s)."@en ;
                                                            rdfs:label "nominal power consumption"@en .


###  https://saref.etsi.org/saref4bldg/nominalPowerRate
<https://saref.etsi.org/saref4bldg/nominalPowerRate> rdf:type owl:NamedIndividual ,
                                                              <https://saref.etsi.org/core/Property> ;
                                                     rdfs:comment "Nominal fan power rate.Usually measured in Watts (W, J/s)."@en ;
                                                     rdfs:label "nominal power rate"@en .


###  https://saref.etsi.org/saref4bldg/nominalPressureDrop
<https://saref.etsi.org/saref4bldg/nominalPressureDrop> rdf:type owl:NamedIndividual ,
                                                                 <https://saref.etsi.org/core/Property> ;
                                                        rdfs:comment "Total pressure drop across the filter. Usually measured in Pascals (Pa, N/m2)."@en ;
                                                        rdfs:label "nominal pressure drop"@en .


###  https://saref.etsi.org/saref4bldg/nominalReturnWaterTemperatureCooling
<https://saref.etsi.org/saref4bldg/nominalReturnWaterTemperatureCooling> rdf:type owl:NamedIndividual ,
                                                                                  <https://saref.etsi.org/core/Property> ;
                                                                         rdfs:comment "Nominal return water temperature (refers to nominal cooling capacity). Usually measured in degrees Kelvin (K)."@en ;
                                                                         rdfs:label "nominal return water temperature cooling"@en .


###  https://saref.etsi.org/saref4bldg/nominalReturnWaterTemperatureHeating
<https://saref.etsi.org/saref4bldg/nominalReturnWaterTemperatureHeating> rdf:type owl:NamedIndividual ,
                                                                                  <https://saref.etsi.org/core/Property> ;
                                                                         rdfs:comment "Nominal return water temperature (refers to nominal heating capacity). Usually measured in degrees Kelvin (K)."@en ;
                                                                         rdfs:label "nominal return water temperature heating"@en .


###  https://saref.etsi.org/saref4bldg/nominalRotationSpeed
<https://saref.etsi.org/saref4bldg/nominalRotationSpeed> rdf:type owl:NamedIndividual ,
                                                                  <https://saref.etsi.org/core/Property> ;
                                                         rdfs:comment "Nominal fan wheel speed. Usually measured in cycles/s."@en ;
                                                         rdfs:label "nominal rotation speed"@en .


###  https://saref.etsi.org/saref4bldg/nominalSensibleCapacity
<https://saref.etsi.org/saref4bldg/nominalSensibleCapacity> rdf:type owl:NamedIndividual ,
                                                                     <https://saref.etsi.org/core/Property> ;
                                                            rdfs:comment "Nominal sensible capacity. Usually measured in Watts (W, J/s)."@en ;
                                                            rdfs:label "nominal sensible capacity"@en .


###  https://saref.etsi.org/saref4bldg/nominalSorroundingHumidityCooling
<https://saref.etsi.org/saref4bldg/nominalSorroundingHumidityCooling> rdf:type owl:NamedIndividual ,
                                                                               <https://saref.etsi.org/core/Property> ;
                                                                      rdfs:comment "Nominal surrounding humidity (refers to nominal cooling capacity). Usually measured in degrees Kelvin (K)."@en ;
                                                                      rdfs:label "nominal sorrounding humidity cooling"@en .


###  https://saref.etsi.org/saref4bldg/nominalSorroundingTemperatureCooling
<https://saref.etsi.org/saref4bldg/nominalSorroundingTemperatureCooling> rdf:type owl:NamedIndividual ,
                                                                                  <https://saref.etsi.org/core/Property> ;
                                                                         rdfs:comment "Nominal surrounding temperature (refers to nominal cooling capacity). Usually measured in degrees Kelvin (K)."@en ;
                                                                         rdfs:label "nominal sorrounding temperature cooling"@en .


###  https://saref.etsi.org/saref4bldg/nominalSorroundingTemperatureHeating
<https://saref.etsi.org/saref4bldg/nominalSorroundingTemperatureHeating> rdf:type owl:NamedIndividual ,
                                                                                  <https://saref.etsi.org/core/Property> ;
                                                                         rdfs:comment "Nominal surrounding temperature (refers to nominal heating capacity). Usually measured in degrees Kelvin (K)."@en ;
                                                                         rdfs:label "nominal sorrounding temperature heating"@en .


###  https://saref.etsi.org/saref4bldg/nominalStaticPressure
<https://saref.etsi.org/saref4bldg/nominalStaticPressure> rdf:type owl:NamedIndividual ,
                                                                   <https://saref.etsi.org/core/Property> ;
                                                          rdfs:comment "The static pressure within the air stream that the fan must overcome to insure designed circulation of air. Usually measured in Pascals (Pa, N/m2)."@en ;
                                                          rdfs:label "nominal static pressure"@en .


###  https://saref.etsi.org/saref4bldg/nominalSupplyVoltage
<https://saref.etsi.org/saref4bldg/nominalSupplyVoltage> rdf:type owl:NamedIndividual ,
                                                                  <https://saref.etsi.org/core/Property> ;
                                                         rdfs:comment "The nominal voltage of the supply. Usually measured in Volts (V, W/A)."@en ;
                                                         rdfs:label "nominal supply voltage"@en .


###  https://saref.etsi.org/saref4bldg/nominalSupplyVoltageMin
<https://saref.etsi.org/saref4bldg/nominalSupplyVoltageMin> rdf:type owl:NamedIndividual ,
                                                                     <https://saref.etsi.org/core/Property> ;
                                                            rdfs:comment "The maximum and minimum allowed voltage of the supply e.g. boundaries of 380V/440V may be applied for a nominal voltage of 400V."@en ;
                                                            rdfs:label "nominal supply voltage offset"@en .


###  https://saref.etsi.org/saref4bldg/nominalSupplyWaterTemperatureCooling
<https://saref.etsi.org/saref4bldg/nominalSupplyWaterTemperatureCooling> rdf:type owl:NamedIndividual ,
                                                                                  <https://saref.etsi.org/core/Property> ;
                                                                         rdfs:comment "Nominal supply water temperature (refers to nominal cooling capacity). Usually measured in degrees Kelvin (K)."@en ;
                                                                         rdfs:label "nominal supply water temperature cooling"@en .


###  https://saref.etsi.org/saref4bldg/nominalSupplyWaterTemperatureHeating
<https://saref.etsi.org/saref4bldg/nominalSupplyWaterTemperatureHeating> rdf:type owl:NamedIndividual ,
                                                                                  <https://saref.etsi.org/core/Property> ;
                                                                         rdfs:comment "Nominal supply water temperature (refers to nominal heating capacity). Usually measured in degrees Kelvin (K)."@en ;
                                                                         rdfs:label "nominal supply water temperature heating"@en .


###  https://saref.etsi.org/saref4bldg/nominalTotalPressure
<https://saref.etsi.org/saref4bldg/nominalTotalPressure> rdf:type owl:NamedIndividual ,
                                                                  <https://saref.etsi.org/core/Property> ;
                                                         rdfs:comment "Nominal total pressure rise across the fan. Usually measured in Pascals (Pa, N/m2)."@en ;
                                                         rdfs:label "nominal total pressure"@en .


###  https://saref.etsi.org/saref4bldg/nominalUa
<https://saref.etsi.org/saref4bldg/nominalUa> rdf:type owl:NamedIndividual ,
                                                       <https://saref.etsi.org/core/Property> ;
                                              rdfs:comment "Nominal UA value."@en ;
                                              rdfs:label "nominal ua"@en .


###  https://saref.etsi.org/saref4bldg/nominalVolumetricCapacity
<https://saref.etsi.org/saref4bldg/nominalVolumetricCapacity> rdf:type owl:NamedIndividual ,
                                                                       <https://saref.etsi.org/core/Property> ;
                                                              rdfs:comment "The total nominal or design volumetric capacity of the tank. Usually measured in cubic metre (m3)."@en ;
                                                              rdfs:label "nominal volumetric capacity"@en .


###  https://saref.etsi.org/saref4bldg/nominalWaterFlowCooling
<https://saref.etsi.org/saref4bldg/nominalWaterFlowCooling> rdf:type owl:NamedIndividual ,
                                                                     <https://saref.etsi.org/core/Property> ;
                                                            rdfs:comment "Nominal water flow (refers to nominal cooling capacity). Usually measured in m3/s."@en ;
                                                            rdfs:label "nominal water flow cooling"@en .


###  https://saref.etsi.org/saref4bldg/nominalWaterFlowHeating
<https://saref.etsi.org/saref4bldg/nominalWaterFlowHeating> rdf:type owl:NamedIndividual ,
                                                                     <https://saref.etsi.org/core/Property> ;
                                                            rdfs:comment "Nominal water flow (refers to nominal heating capacity). Usually measured in m3/s."@en ;
                                                            rdfs:label "nominal water flow heating"@en .


###  https://saref.etsi.org/saref4bldg/nominalWidthOrDiameter
<https://saref.etsi.org/saref4bldg/nominalWidthOrDiameter> rdf:type owl:NamedIndividual ,
                                                                    <https://saref.etsi.org/core/Property> ;
                                                           rdfs:comment "The nominal width or, in the case of a horizontal cylindrical tank, the nominal diameter of the tank. Note: Not required for a vertical cylindrical tank. Usually measured in millimeters (mm)."@en ;
                                                           rdfs:label "nominal width or diameter"@en .


###  https://saref.etsi.org/saref4bldg/nomminalRotationSpeed
<https://saref.etsi.org/saref4bldg/nomminalRotationSpeed> rdf:type owl:NamedIndividual ,
                                                                   <https://saref.etsi.org/core/Property> ;
                                                          rdfs:comment "Pump rotational speed under nominal conditions. Usually measured in cycles/s."@en ;
                                                          rdfs:label "nomminal rotation speed"@en .


###  https://saref.etsi.org/saref4bldg/openPressureDrop
<https://saref.etsi.org/saref4bldg/openPressureDrop> rdf:type owl:NamedIndividual ,
                                                              <https://saref.etsi.org/core/Property> ;
                                                     rdfs:comment "Total pressure drop across damper. Usually measured in Pascals (Pa, N/m2)."@en ;
                                                     rdfs:label "open pressure drop"@en .


###  https://saref.etsi.org/saref4bldg/operatingWeight
<https://saref.etsi.org/saref4bldg/operatingWeight> rdf:type owl:NamedIndividual ,
                                                             <https://saref.etsi.org/core/Property> ;
                                                    rdfs:comment "Operating weight of the tank including all of its contents. Usually measured in kilograms (kg) or grams (g)."@en ;
                                                    rdfs:label "operating weight"@en .


###  https://saref.etsi.org/saref4bldg/operationTemperatureMax
<https://saref.etsi.org/saref4bldg/operationTemperatureMax> rdf:type owl:NamedIndividual ,
                                                                     <https://saref.etsi.org/core/Property> ;
                                                            rdfs:comment "Allowable operation ambient (air, fluid) temperature range. Usually measured in degrees Kelvin (K)."@en ;
                                                            rdfs:label "operation temperature range"@en .


###  https://saref.etsi.org/saref4bldg/operationTemperatureMin
<https://saref.etsi.org/saref4bldg/operationTemperatureMin> rdf:type owl:NamedIndividual ,
                                                                     <https://saref.etsi.org/core/Property> ;
                                                            rdfs:comment "Allowable operation ambient (air, fluid) temperature range. Usually measured in degrees Kelvin (K)."@en ;
                                                            rdfs:label "operation temperature range"@en .


###  https://saref.etsi.org/saref4bldg/operationalRiterial
<https://saref.etsi.org/saref4bldg/operationalRiterial> rdf:type owl:NamedIndividual ,
                                                                 <https://saref.etsi.org/core/Property> ;
                                                        rdfs:comment "Time of operation at maximum operational ambient air temperature. Measured in seconds (s) or days (d) or other units of time."@en ;
                                                        rdfs:label "operational riterial"@en .


###  https://saref.etsi.org/saref4bldg/outletConnectionSize
<https://saref.etsi.org/saref4bldg/outletConnectionSize> rdf:type owl:NamedIndividual ,
                                                                  <https://saref.etsi.org/core/Property> ;
                                                         rdfs:comment "Size of the outlet connection. Usually measured in millimeters (mm)."@en ;
                                                         rdfs:label "outlet connection size"@en .


###  https://saref.etsi.org/saref4bldg/outletTemperatureMax
<https://saref.etsi.org/saref4bldg/outletTemperatureMax> rdf:type owl:NamedIndividual ,
                                                                  <https://saref.etsi.org/core/Property> ;
                                                         rdfs:comment "Allowable outlet temperature of either the water or the steam. Usually measured in degrees Kelvin (K)."@en ;
                                                         rdfs:label "outlet temperature range"@en .


###  https://saref.etsi.org/saref4bldg/outletTemperatureMin
<https://saref.etsi.org/saref4bldg/outletTemperatureMin> rdf:type owl:NamedIndividual ,
                                                                  <https://saref.etsi.org/core/Property> ;
                                                         rdfs:comment "Allowable outlet temperature of either the water or the steam. Usually measured in degrees Kelvin (K)."@en ;
                                                         rdfs:label "outlet temperature range"@en .


###  https://saref.etsi.org/saref4bldg/outputCapacity
<https://saref.etsi.org/saref4bldg/outputCapacity> rdf:type owl:NamedIndividual ,
                                                            <https://saref.etsi.org/core/Property> ;
                                                   rdfs:comment "Total nominal heat output as listed by the manufacturer. Usually measured in Watts (W, J/s)."@en ;
                                                   rdfs:label "output capacity"@en .


###  https://saref.etsi.org/saref4bldg/outsideDiameter
<https://saref.etsi.org/saref4bldg/outsideDiameter> rdf:type owl:NamedIndividual ,
                                                             <https://saref.etsi.org/core/Property> ;
                                                    rdfs:comment "Actual outside diameter of the tube in the tube bundle. Usually measured in millimeters (mm)."@en ;
                                                    rdfs:label "outside diameter"@en .


###  https://saref.etsi.org/saref4bldg/partLoadRatioMax
<https://saref.etsi.org/saref4bldg/partLoadRatioMax> rdf:type owl:NamedIndividual ,
                                                              <https://saref.etsi.org/core/Property> ;
                                                     rdfs:comment "Maximum part load ratio as a fraction of nominal capacity."@en ;
                                                     rdfs:label "maximum part load ratio"@en .


###  https://saref.etsi.org/saref4bldg/partLoadRatioMin
<https://saref.etsi.org/saref4bldg/partLoadRatioMin> rdf:type owl:NamedIndividual ,
                                                              <https://saref.etsi.org/core/Property> ;
                                                     rdfs:comment "Minimum part load ratio as a fraction of nominal capacity."@en ;
                                                     rdfs:label "minimum part load ratio"@en .


###  https://saref.etsi.org/saref4bldg/powerOutputMax
<https://saref.etsi.org/saref4bldg/powerOutputMax> rdf:type owl:NamedIndividual ,
                                                            <https://saref.etsi.org/core/Property> ;
                                                   rdfs:comment "The maximum output power rating of the engine. Usually measured in Watts (W, J/s)."@en ;
                                                   rdfs:label "maximum power output"@en .


###  https://saref.etsi.org/saref4bldg/pressureRating
<https://saref.etsi.org/saref4bldg/pressureRating> rdf:type owl:NamedIndividual ,
                                                            <https://saref.etsi.org/core/Property> ;
                                                   rdfs:comment "Nominal pressure rating of the boiler as rated by the agency having jurisdiction. Usually measured in Pascals (Pa, N/m2)."@en ;
                                                   rdfs:label "pressure rating"@en .


###  https://saref.etsi.org/saref4bldg/primaryAirFlowRateMax
<https://saref.etsi.org/saref4bldg/primaryAirFlowRateMax> rdf:type owl:NamedIndividual ,
                                                                   <https://saref.etsi.org/core/Property> ;
                                                          rdfs:comment "Maximum primary airflow that can be delivered. Usually measured in m3/s."@en ;
                                                          rdfs:label "primary air flow rate range"@en .


###  https://saref.etsi.org/saref4bldg/primaryAirFlowRateMin
<https://saref.etsi.org/saref4bldg/primaryAirFlowRateMin> rdf:type owl:NamedIndividual ,
                                                                   <https://saref.etsi.org/core/Property> ;
                                                          rdfs:comment "Minimum primary airflow that can be delivered. Usually measured in m3/s."@en ;
                                                          rdfs:label "primary air flow rate range"@en .


###  https://saref.etsi.org/saref4bldg/primaryApparentPower
<https://saref.etsi.org/saref4bldg/primaryApparentPower> rdf:type owl:NamedIndividual ,
                                                                  <https://saref.etsi.org/core/Property> ;
                                                         rdfs:comment "The power in VA (volt ampere) that has been transformed and that runs into the transformer on the primary side. Usually measured in Watts (W, J/s)."@en ;
                                                         rdfs:label "primary apparent power"@en .


###  https://saref.etsi.org/saref4bldg/primaryCurrent
<https://saref.etsi.org/saref4bldg/primaryCurrent> rdf:type owl:NamedIndividual ,
                                                            <https://saref.etsi.org/core/Property> ;
                                                   rdfs:comment "The current that is going to be transformed and that runs into the transformer on the primary side. Usually measured in Ampere (A)."@en ;
                                                   rdfs:label "primary current"@en .


###  https://saref.etsi.org/saref4bldg/primaryFrequency
<https://saref.etsi.org/saref4bldg/primaryFrequency> rdf:type owl:NamedIndividual ,
                                                              <https://saref.etsi.org/core/Property> ;
                                                     rdfs:comment "The frequency that is going to be transformed and that runs into the transformer on the primary side. Usually measured in cycles/s or Hertz (Hz)."@en ;
                                                     rdfs:label "primary frequency"@en .


###  https://saref.etsi.org/saref4bldg/primaryVoltage
<https://saref.etsi.org/saref4bldg/primaryVoltage> rdf:type owl:NamedIndividual ,
                                                            <https://saref.etsi.org/core/Property> ;
                                                   rdfs:comment "The voltage that is going to be transformed and that runs into the transformer on the primary side. Usually measured in Volts (V, W/A)."@en ;
                                                   rdfs:label "primary voltage"@en .


###  https://saref.etsi.org/saref4bldg/pumpFlowRateMax
<https://saref.etsi.org/saref4bldg/pumpFlowRateMax> rdf:type owl:NamedIndividual ,
                                                             <https://saref.etsi.org/core/Property> ;
                                                    rdfs:comment "Allowable range of volume of fluid being pumped against the resistance specified. Usually measured in kg/s."@en ;
                                                    rdfs:label "pump flow rate range"@en .


###  https://saref.etsi.org/saref4bldg/pumpFlowRateMin
<https://saref.etsi.org/saref4bldg/pumpFlowRateMin> rdf:type owl:NamedIndividual ,
                                                             <https://saref.etsi.org/core/Property> ;
                                                    rdfs:comment "Allowable range of volume of fluid being pumped against the resistance specified. Usually measured in kg/s."@en ;
                                                    rdfs:label "pump flow rate range"@en .


###  https://saref.etsi.org/saref4bldg/realImpedanceRatio
<https://saref.etsi.org/saref4bldg/realImpedanceRatio> rdf:type owl:NamedIndividual ,
                                                                <https://saref.etsi.org/core/Property> ;
                                                       rdfs:comment "The ratio between the real part of the zero sequence impedance and the real part of the positive impedance (i.e. real part of the short-circuit voltage) of the transformer. Used for three-phase transformer which includes a N-conductor."@en ;
                                                       rdfs:label "real impedance ratio"@en .


###  https://saref.etsi.org/saref4bldg/secondCurvatureRadius
<https://saref.etsi.org/saref4bldg/secondCurvatureRadius> rdf:type owl:NamedIndividual ,
                                                                   <https://saref.etsi.org/core/Property> ;
                                                          rdfs:comment "SecondCurvatureRadius should be defined as the top or right side radius of curvature value. Usually measured in millimeters (mm)."@en ;
                                                          rdfs:label "second curvature radius"@en .


###  https://saref.etsi.org/saref4bldg/secondaryAirFlowRateMax
<https://saref.etsi.org/saref4bldg/secondaryAirFlowRateMax> rdf:type owl:NamedIndividual ,
                                                                     <https://saref.etsi.org/core/Property> ;
                                                            rdfs:comment "Maximum secondary airflow that can be delivered. Usually measured in Pascals (Pa, N/m2)."@en ;
                                                            rdfs:label "secondary air flow rate range"@en .


###  https://saref.etsi.org/saref4bldg/secondaryAirFlowRateMin
<https://saref.etsi.org/saref4bldg/secondaryAirFlowRateMin> rdf:type owl:NamedIndividual ,
                                                                     <https://saref.etsi.org/core/Property> ;
                                                            rdfs:comment "Maximum secondary airflow that can be delivered. Usually measured in Pascals (Pa, N/m2)."@en ;
                                                            rdfs:label "secondary air flow rate range"@en .


###  https://saref.etsi.org/saref4bldg/secondaryApparentPower
<https://saref.etsi.org/saref4bldg/secondaryApparentPower> rdf:type owl:NamedIndividual ,
                                                                    <https://saref.etsi.org/core/Property> ;
                                                           rdfs:comment "The power in VA (volt ampere) that has been transformed and is running out of the transformer on the secondary side. Usually measured in Watts (W, J/s)."@en ;
                                                           rdfs:label "secondary apparent power"@en .


###  https://saref.etsi.org/saref4bldg/secondaryCurrent
<https://saref.etsi.org/saref4bldg/secondaryCurrent> rdf:type owl:NamedIndividual ,
                                                              <https://saref.etsi.org/core/Property> ;
                                                     rdfs:comment "The current that has been transformed and is running out of the transformer on the secondary side. Usually measured in Ampere (A)."@en ;
                                                     rdfs:label "secondary current"@en .


###  https://saref.etsi.org/saref4bldg/secondaryFrequency
<https://saref.etsi.org/saref4bldg/secondaryFrequency> rdf:type owl:NamedIndividual ,
                                                                <https://saref.etsi.org/core/Property> ;
                                                       rdfs:comment "The frequency that has been transformed and is running out of the transformer on the secondary side. Usually measured in cycles/s or Hertz (Hz)."@en ;
                                                       rdfs:label "secondary frequency"@en .


###  https://saref.etsi.org/saref4bldg/secondaryVoltage
<https://saref.etsi.org/saref4bldg/secondaryVoltage> rdf:type owl:NamedIndividual ,
                                                              <https://saref.etsi.org/core/Property> ;
                                                     rdfs:comment "The voltage that has been transformed and is running out of the transformer on the secondary side. Usually measured in Volts (V, W/A)."@en ;
                                                     rdfs:label "secondary voltage"@en .


###  https://saref.etsi.org/saref4bldg/size
<https://saref.etsi.org/saref4bldg/size> rdf:type owl:NamedIndividual ,
                                                  <https://saref.etsi.org/core/Property> ;
                                         rdfs:comment "The size of the connection to the valve (or to each connection for faucets, mixing valves, etc.). Usually measured in millimeters (mm)."@en ;
                                         rdfs:label "size"@en .


###  https://saref.etsi.org/saref4bldg/solarReflectance
<https://saref.etsi.org/saref4bldg/solarReflectance> rdf:type owl:NamedIndividual ,
                                                              <https://saref.etsi.org/core/Property> ;
                                                     rdfs:comment "(Rsol): The ratio of incident solar radiation that is reflected by a shading system (also named _e). Note the following equation Asol + Rsol + Tsol = 1"@en ;
                                                     rdfs:label "solar reflectance"@en .


###  https://saref.etsi.org/saref4bldg/solarTransmittance
<https://saref.etsi.org/saref4bldg/solarTransmittance> rdf:type owl:NamedIndividual ,
                                                                <https://saref.etsi.org/core/Property> ;
                                                       rdfs:comment "(Tsol) The ratio of incident solar radiation that directly passes through a shading system (also named _e). Note the following equation Asol + Rsol + Tsol = 1"@en ;
                                                       rdfs:label "solar transmittance"@en .


###  https://saref.etsi.org/saref4bldg/spectrumMax
<https://saref.etsi.org/saref4bldg/spectrumMax> rdf:type owl:NamedIndividual ,
                                                         <https://saref.etsi.org/core/Property> ;
                                                rdfs:comment "The spectrum of radiation describes its composition with regard to wavelength. Light, for example, as the portion of electromagnetic radiation that is visible to the human eye, is radiation with wavelengths in the range of approx. 380 to 780 nm (1 nm = 10 m). The corresponding range of colours varies from violet to indigo, blue, green, yellow, orange, and red. These colours form a continuous spectrum, in which the various spectral sectors merge into each other."@en ;
                                                rdfs:label "maximum spectrum"@en .


###  https://saref.etsi.org/saref4bldg/spectrumMin
<https://saref.etsi.org/saref4bldg/spectrumMin> rdf:type owl:NamedIndividual ,
                                                         <https://saref.etsi.org/core/Property> ;
                                                rdfs:comment "The spectrum of radiation describes its composition with regard to wavelength. Light, for example, as the portion of electromagnetic radiation that is visible to the human eye, is radiation with wavelengths in the range of approx. 380 to 780 nm (1 nm = 10 m). The corresponding range of colours varies from violet to indigo, blue, green, yellow, orange, and red. These colours form a continuous spectrum, in which the various spectral sectors merge into each other."@en ;
                                                rdfs:label "minimum spectrum"@en .


###  https://saref.etsi.org/saref4bldg/staggeredRowSpacing
<https://saref.etsi.org/saref4bldg/staggeredRowSpacing> rdf:type owl:NamedIndividual ,
                                                                 <https://saref.etsi.org/core/Property> ;
                                                        rdfs:comment "Staggered tube row spacing. Usually measured in millimeters (mm)."@en ;
                                                        rdfs:label "staggered row spacing"@en .


###  https://saref.etsi.org/saref4bldg/startCurrentFactor
<https://saref.etsi.org/saref4bldg/startCurrentFactor> rdf:type owl:NamedIndividual ,
                                                                <https://saref.etsi.org/core/Property> ;
                                                       rdfs:comment "IEC. Start current factor defines how large the peek starting current will become on the engine. StartCurrentFactor is multiplied to NominalCurrent and we get the start current."@en ;
                                                       rdfs:label "start current factor"@en .


###  https://saref.etsi.org/saref4bldg/startingTime
<https://saref.etsi.org/saref4bldg/startingTime> rdf:type owl:NamedIndividual ,
                                                          <https://saref.etsi.org/core/Property> ;
                                                 rdfs:comment "The time (in s) needed for the motor to reach its rated speed with its driven equipment attached, starting from standstill and at the nominal voltage applied at its terminals."@en ;
                                                 rdfs:label "starting time"@en .


###  https://saref.etsi.org/saref4bldg/supportedWeightMax
<https://saref.etsi.org/saref4bldg/supportedWeightMax> rdf:type owl:NamedIndividual ,
                                                                <https://saref.etsi.org/core/Property> ;
                                                       rdfs:comment "The maximum weight that can be carried by the vibration isolator. Usually measured in kilograms (kg) or grams (g)."@en ;
                                                       rdfs:label "maximum supported weight"@en .


###  https://saref.etsi.org/saref4bldg/teTime
<https://saref.etsi.org/saref4bldg/teTime> rdf:type owl:NamedIndividual ,
                                                    <https://saref.etsi.org/core/Property> ;
                                           rdfs:comment "The maximum time (in s) at which the motor could run with locked rotor when the motor is used in an EX-environment. The time indicates that a protective device should trip before this time when the starting current of the motor is slowing through the device."@en ;
                                           rdfs:label "te time"@en .


###  https://saref.etsi.org/saref4bldg/temperatureRating
<https://saref.etsi.org/saref4bldg/temperatureRating> rdf:type owl:NamedIndividual ,
                                                               <https://saref.etsi.org/core/Property> ;
                                                      rdfs:comment "Temperature rating. Usually measured in degrees Kelvin (K)."@en ;
                                                      rdfs:label "temperature rating"@en .


###  https://saref.etsi.org/saref4bldg/testPressure
<https://saref.etsi.org/saref4bldg/testPressure> rdf:type owl:NamedIndividual ,
                                                          <https://saref.etsi.org/core/Property> ;
                                                 rdfs:comment "The maximum pressure to which the valve has been subjected under test. Usually measured in Pascals (Pa, N/m2)."@en ;
                                                 rdfs:label "test pressure"@en .


###  https://saref.etsi.org/saref4bldg/thermalConductivity
<https://saref.etsi.org/saref4bldg/thermalConductivity> rdf:type owl:NamedIndividual ,
                                                                 <https://saref.etsi.org/core/Property> ;
                                                        rdfs:comment "Fouling factor of the tubes in the tube bundle. Usually measured in m2 Kelvin/Watt."@en ;
                                                        rdfs:label "thermal conductivity"@en .


###  https://saref.etsi.org/saref4bldg/thermalEfficiency
<https://saref.etsi.org/saref4bldg/thermalEfficiency> rdf:type owl:NamedIndividual ,
                                                               <https://saref.etsi.org/core/Property> ;
                                                      rdfs:comment "Overall Thermal Efficiency is defined as gross energy output of the heat transfer device divided by the energy input."@en ;
                                                      rdfs:label "thermal efficiency"@en .


###  https://saref.etsi.org/saref4bldg/thermalMassHeatCapacity
<https://saref.etsi.org/saref4bldg/thermalMassHeatCapacity> rdf:type owl:NamedIndividual ,
                                                                     <https://saref.etsi.org/core/Property> ;
                                                            rdfs:comment "Product of component mass and specific heat."@en ;
                                                            rdfs:label "thermal mass heat capacity"@en .


###  https://saref.etsi.org/saref4bldg/thermalTransmittance
<https://saref.etsi.org/saref4bldg/thermalTransmittance> rdf:type owl:NamedIndividual ,
                                                                  <https://saref.etsi.org/core/Property> ;
                                                         rdfs:comment "Rate at which energy is transmitted through a body. Usually measured in Watts/m2 Kelvin."@en ;
                                                         rdfs:label "thermal transmittance"@en .


###  https://saref.etsi.org/saref4bldg/ventilatingPipeSize
<https://saref.etsi.org/saref4bldg/ventilatingPipeSize> rdf:type owl:NamedIndividual ,
                                                                 <https://saref.etsi.org/core/Property> ;
                                                        rdfs:comment "Size of the ventilating pipe(s). Usually measured in millimeters (mm)."@en ;
                                                        rdfs:label "ventilating pipe size"@en .


###  https://saref.etsi.org/saref4bldg/verticalSpacing
<https://saref.etsi.org/saref4bldg/verticalSpacing> rdf:type owl:NamedIndividual ,
                                                             <https://saref.etsi.org/core/Property> ;
                                                    rdfs:comment "Vertical spacing between tubes in the tube bundle.Usually measured in millimeters (mm)."@en ;
                                                    rdfs:label "vertical spacing"@en .


###  https://saref.etsi.org/saref4bldg/vibrationTransmissibility
<https://saref.etsi.org/saref4bldg/vibrationTransmissibility> rdf:type owl:NamedIndividual ,
                                                                       <https://saref.etsi.org/core/Property> ;
                                                              rdfs:comment "The vibration transmissibility percentage."@en ;
                                                              rdfs:label "vibration transmissibility"@en .


###  https://saref.etsi.org/saref4bldg/visibleLightReflectance
<https://saref.etsi.org/saref4bldg/visibleLightReflectance> rdf:type owl:NamedIndividual ,
                                                                     <https://saref.etsi.org/core/Property> ;
                                                            rdfs:comment "Fraction of the visible light that is reflected by the glazing at normal incidence. It is a value without unit."@en ;
                                                            rdfs:label "visible light reflectance"@en .


###  https://saref.etsi.org/saref4bldg/visibleLightTransmittance
<https://saref.etsi.org/saref4bldg/visibleLightTransmittance> rdf:type owl:NamedIndividual ,
                                                                       <https://saref.etsi.org/core/Property> ;
                                                              rdfs:comment "Fraction of the visible light that passes the shading system at normal incidence. It is a value without unit."@en ;
                                                              rdfs:label "visible light transmittance"@en .


###  https://saref.etsi.org/saref4bldg/volumen
<https://saref.etsi.org/saref4bldg/volumen> rdf:type owl:NamedIndividual ,
                                                     <https://saref.etsi.org/core/Property> ;
                                            rdfs:comment "Total volume of fluid in the tubes and their headers. Usually measured in cubic metre (m3)."@en ;
                                            rdfs:label "volumen"@en .


###  https://saref.etsi.org/saref4bldg/waterInletTemperatureMax
<https://saref.etsi.org/saref4bldg/waterInletTemperatureMax> rdf:type owl:NamedIndividual ,
                                                                      <https://saref.etsi.org/core/Property> ;
                                                             rdfs:comment "Allowable water inlet temperature range. Usually measured in degrees Kelvin (K)."@en ;
                                                             rdfs:label "water inlet temperature range"@en .


###  https://saref.etsi.org/saref4bldg/waterInletTemperatureMin
<https://saref.etsi.org/saref4bldg/waterInletTemperatureMin> rdf:type owl:NamedIndividual ,
                                                                      <https://saref.etsi.org/core/Property> ;
                                                             rdfs:comment "Allowable water inlet temperature range. Usually measured in degrees Kelvin (K)."@en ;
                                                             rdfs:label "water inlet temperature range"@en .


###  https://saref.etsi.org/saref4bldg/waterPressureMax
<https://saref.etsi.org/saref4bldg/waterPressureMax> rdf:type owl:NamedIndividual ,
                                                              <https://saref.etsi.org/core/Property> ;
                                                     rdfs:comment "Allowable water circuit working pressure range. Usually measured in Pascals (Pa, N/m2)."@en ;
                                                     rdfs:label "water pressure range"@en .


###  https://saref.etsi.org/saref4bldg/waterPressureMin
<https://saref.etsi.org/saref4bldg/waterPressureMin> rdf:type owl:NamedIndividual ,
                                                              <https://saref.etsi.org/core/Property> ;
                                                     rdfs:comment "Allowable water circuit working pressure range. Usually measured in Pascals (Pa, N/m2)."@en ;
                                                     rdfs:label "water pressure range"@en .


###  https://saref.etsi.org/saref4bldg/waterRequirement
<https://saref.etsi.org/saref4bldg/waterRequirement> rdf:type owl:NamedIndividual ,
                                                              <https://saref.etsi.org/core/Property> ;
                                                     rdfs:comment "Make-up water requirement. Usually measured in m3/s."@en ;
                                                     rdfs:label "water requirement"@en .


###  https://saref.etsi.org/saref4bldg/waterStorageCapacity
<https://saref.etsi.org/saref4bldg/waterStorageCapacity> rdf:type owl:NamedIndividual ,
                                                                  <https://saref.etsi.org/core/Property> ;
                                                         rdfs:comment "Water storage capacity. Usually measured in cubic metre (m3)."@en ;
                                                         rdfs:label "water storage capacity"@en .


###  https://saref.etsi.org/saref4bldg/weight
<https://saref.etsi.org/saref4bldg/weight> rdf:type owl:NamedIndividual ,
                                                    <https://saref.etsi.org/core/Property> ;
                                           rdfs:comment "The weight of the device. Usually measured in kilograms (kg) or grams (g)."@en ;
                                           rdfs:label "weight"@en .


###  https://saref.etsi.org/saref4bldg/workingPressure
<https://saref.etsi.org/saref4bldg/workingPressure> rdf:type owl:NamedIndividual ,
                                                             <https://saref.etsi.org/core/Property> ;
                                                    rdfs:comment "The normally expected maximum working pressure of the valve. Usually measured in Pascals (Pa, N/m2)."@en ;
                                                    rdfs:label "working pressure"@en .


###  https://saref.etsi.org/saref4bldg/workingPressureMax
<https://saref.etsi.org/saref4bldg/workingPressureMax> rdf:type owl:NamedIndividual ,
                                                                <https://saref.etsi.org/core/Property> ;
                                                       rdfs:comment "Maximum working pressure. Usually measured in Pascals (Pa, N/m2)."@en ;
                                                       rdfs:label "maximum working pressure"@en .


###  https://saref.etsi.org/saref4bldg/workingPressureMin
<https://saref.etsi.org/saref4bldg/workingPressureMin> rdf:type owl:NamedIndividual ,
                                                                <https://saref.etsi.org/core/Property> ;
                                                       rdfs:comment "Allowable minimum working pressure (relative to ambient pressure). Usually measured in Pascals (Pa, N/m2)."@en ;
                                                       rdfs:label "minimum working pressure"@en .


###  Generated by the OWL API (version 4.5.29.2024-05-13T12:11:03Z) https://github.com/owlcs/owlapi
